---
title: Applications of the quadratic formula in solving complex equations
videoId: i7idZfS8t8w
---

From: [[khanacademy]] <br/> 

The [[introduction_to_the_quadratic_formula | quadratic formula]] is considered one of the most useful formulas in mathematics <a class="yt-timestamp" data-t="00:00:04">[00:00:04]</a>. While memorization is generally not encouraged, it is recommended to memorize this particular formula, provided one also understands its derivation <a class="yt-timestamp" data-t="00:00:13">[00:00:13]</a>. The formula is used to [[solving_quadratic_equations | solve for the roots, or zeroes, of quadratic equations]] <a class="yt-timestamp" data-t="00:00:32">[00:00:32]</a>.

## The Quadratic Formula

For a general [[understanding_components_of_a_quadratic_equation | quadratic equation]] in the form:
`ax² + bx + c = 0` <a class="yt-timestamp" data-t="00:00:44">[00:00:44]</a>

Where:
*   `a` is the coefficient of the x² (second-degree) term <a class="yt-timestamp" data-t="00:00:58">[00:00:58]</a>
*   `b` is the coefficient of the x term <a class="yt-timestamp" data-t="00:01:02">[00:01:02]</a>
*   `c` is the constant term (or coefficient of the x⁰ term) <a class="yt-timestamp" data-t="00:01:05">[00:01:05]</a>

The [[solving_techniques_for_quadratic_equations | solutions]] for x are given by the [[introduction_to_the_quadratic_formula | quadratic formula]]:

`x = -b ± √(b² - 4ac) / 2a` <a class="yt-timestamp" data-t="00:01:16">[00:01:16]</a>

This formula is derived by [[quadratic_equations_transformation | completing the square]] on the general quadratic equation <a class="yt-timestamp" data-t="00:01:54">[00:01:54]</a>.

## Applications and Examples

The [[solving_quadratic_equations_using_the_quadratic_formula | quadratic formula]] is a versatile tool for [[solving_quadratic_equations | solving quadratic equations]], particularly useful for problems that are difficult or impossible to [[factoring_quadratic_equations | factor]] <a class="yt-timestamp" data-t="00:05:45">[00:05:45]</a>.

### Example 1: Verifying with Factoring

Let's solve `x² + 4x - 21 = 0` using the formula <a class="yt-timestamp" data-t="00:02:14">[00:02:14]</a>.

1.  **Identify coefficients**: For this equation, `a = 1`, `b = 4`, and `c = -21` <a class="yt-timestamp" data-t="00:02:30">[00:02:30]</a>.
2.  **Plug into the formula**:
    `x = -4 ± √(4² - 4(1)(-21)) / 2(1)` <a class="yt-timestamp" data-t="00:02:49">[00:02:49]</a>
3.  **Simplify**:
    `x = -4 ± √(16 - (-84)) / 2` <a class="yt-timestamp" data-t="00:03:05">[00:03:05]</a>
    `x = -4 ± √(16 + 84) / 2` <a class="yt-timestamp" data-t="00:03:50">[00:03:50]</a>
    `x = -4 ± √100 / 2` <a class="yt-timestamp" data-t="00:04:03">[00:04:03]</a>
    `x = -4 ± 10 / 2` <a class="yt-timestamp" data-t="00:04:09">[00:04:09]</a>
4.  **Find the solutions**:
    *   `x = (-4 + 10) / 2 = 6 / 2 = 3` <a class="yt-timestamp" data-t="00:04:32">[00:04:32]</a>
    *   `x = (-4 - 10) / 2 = -14 / 2 = -7` <a class="yt-timestamp" data-t="00:04:38">[00:04:38]</a>

The solutions are `x = 3` or `x = -7` <a class="yt-timestamp" data-t="00:04:47">[00:04:47]</a>. These results can be verified by [[factoring_quadratic_equations | factoring]] the original equation as `(x + 7)(x - 3) = 0`, which yields the same roots <a class="yt-timestamp" data-t="00:05:04">[00:05:04]</a>. This [[comparison_of_factoring_and_quadratic_formula | comparison of factoring and quadratic formula]] demonstrates that both [[methods_for_solving_quadratic_equations | methods]] yield the same answers when applicable <a class="yt-timestamp" data-t="00:05:36">[00:05:36]</a>.

### Example 2: Equations with No Real Solutions

Consider the equation `3x² + 6x = -10` <a class="yt-timestamp" data-t="00:06:17">[00:06:17]</a>.

1.  **Transform to standard form**: First, rearrange the equation to `ax² + bx + c = 0` by adding 10 to both sides: `3x² + 6x + 10 = 0` <a class="yt-timestamp" data-t="00:06:31">[00:06:31]</a>.
2.  **Identify coefficients**: Here, `a = 3`, `b = 6`, and `c = 10` <a class="yt-timestamp" data-t="00:06:51">[00:06:51]</a>.
3.  **Plug into the formula**:
    `x = -6 ± √(6² - 4(3)(10)) / 2(3)` <a class="yt-timestamp" data-t="00:07:10">[00:07:10]</a>
4.  **Simplify**:
    `x = -6 ± √(36 - 120) / 6` <a class="yt-timestamp" data-t="00:07:42">[00:07:42]</a>
    `x = -6 ± √(-84) / 6` <a class="yt-timestamp" data-t="00:08:19">[00:08:19]</a>

Since the term under the square root (`b² - 4ac`), known as the discriminant, is negative (`-84`), this equation has no real solutions <a class="yt-timestamp" data-t="00:09:06">[00:09:06]</a>. Graphing the function `y = 3x² + 6x + 10` confirms that it never intersects the x-axis, meaning y never equals 0 for any real x-value <a class="yt-timestamp" data-t="00:10:20">[00:10:20]</a>. This demonstrates the formula's ability to indicate when real solutions do not exist <a class="yt-timestamp" data-t="00:10:38">[00:10:38]</a>.

### Example 3: Equations with Irrational Solutions

Let's solve `negative 3x² + 12x + 1 = 0` <a class="yt-timestamp" data-t="00:10:52">[00:10:52]</a>.

1.  **Identify coefficients**: In this case, `a = -3`, `b = 12`, and `c = 1` <a class="yt-timestamp" data-t="00:11:07">[00:11:07]</a>.
2.  **Plug into the formula**:
    `x = -12 ± √(12² - 4(-3)(1)) / 2(-3)` <a class="yt-timestamp" data-t="00:11:13">[00:11:13]</a>
3.  **Simplify**:
    `x = -12 ± √(144 - (-12)) / -6` <a class="yt-timestamp" data-t="00:11:43">[00:11:43]</a>
    `x = -12 ± √(144 + 12) / -6` <a class="yt-timestamp" data-t="00:11:49">[00:11:49]</a>
    `x = -12 ± √156 / -6` <a class="yt-timestamp" data-t="00:12:01">[00:12:01]</a>
4.  **Simplify the radical**: To simplify `√156`, find its prime factorization: `156 = 2 * 78 = 2 * 2 * 39` <a class="yt-timestamp" data-t="00:12:17">[00:12:17]</a>.
    So, `√156 = √(4 * 39) = 2√39` <a class="yt-timestamp" data-t="00:12:48">[00:12:48]</a>.
5.  **Substitute and further simplify**:
    `x = -12 ± 2√39 / -6` <a class="yt-timestamp" data-t="00:13:10">[00:13:10]</a>
    Divide numerator and denominator by 2:
    `x = -6 ± √39 / -3` <a class="yt-timestamp" data-t="00:13:26">[00:13:26]</a>
    Separate the terms:
    `x = -6/-3 ± √39/-3` <a class="yt-timestamp" data-t="00:13:38">[00:13:38]</a>
    `x = 2 ± (-√39/3)` <a class="yt-timestamp" data-t="00:13:49">[00:13:49]</a>
    Since `±` already accounts for both positive and negative variations, the final simplified form is:
    `x = 2 ± √39 / 3` <a class="yt-timestamp" data-t="00:15:01">[00:15:01]</a>

These solutions are irrational, demonstrating the [[solving_quadratic_equations_using_the_quadratic_formula | quadratic formula's]] utility in finding exact solutions that [[factoring_quadratic_equations | factoring]] cannot provide <a class="yt-timestamp" data-t="00:10:46">[00:10:46]</a>. Graphing the function `y = -3x² + 12x + 1` shows two real roots that are consistent with these calculated values <a class="yt-timestamp" data-t="00:15:39">[00:15:39]</a>.