---
title: Canceling common factors in expressions
videoId: 7Uos1ED3KHI
---

From: [[khanacademy]] <br/> 

When working with rational numbers and expressions, a common practice is to reduce them to their lowest terms. This process involves identifying and canceling common factors found in both the numerator and the denominator <a class="yt-timestamp" data-t="00:00:00">[00:00:00]</a>.

## Review of Rational Numbers

The concept of putting fractions into "lowest terms" is fundamental <a class="yt-timestamp" data-t="00:00:07">[00:00:07]</a>.

*   **Example 1: 3/6**
    The numbers 3 and 6 share a common factor <a class="yt-timestamp" data-t="00:00:12">[00:00:12]</a>. The numerator is 3, and the denominator 6 can be written as 2 times 3 <a class="yt-timestamp" data-t="00:00:15">[00:00:15]</a>. Since 3 is a common factor, you can divide both the numerator and denominator by 3, resulting in 1/2 in lowest terms <a class="yt-timestamp" data-t="00:00:22">[00:00:22]</a>.
*   **Example 2: 8/24**
    Similarly, 8 and 24 share a common factor of 8 <a class="yt-timestamp" data-t="00:00:48">[00:00:48]</a>. The fraction 8/24 can be written as 8 over (3 times 8) <a class="yt-timestamp" data-t="00:00:48">[00:00:48]</a>. By canceling the common factor of 8, the fraction simplifies to 1/3 <a class="yt-timestamp" data-t="00:00:58">[00:00:58]</a>.

The process of [[finding_common_factors_in_fractions|finding common factors in fractions]] is directly applicable to rational expressions <a class="yt-timestamp" data-t="00:01:04">[00:01:04]</a>.

## Applying to Rational Expressions

Rational expressions are similar to rational numbers, but their numerators and denominators are expressions involving variables instead of just numbers <a class="yt-timestamp" data-t="00:01:10">[00:01:10]</a>. The same principle of canceling common factors applies <a class="yt-timestamp" data-t="00:01:04">[00:01:04]</a>.

### Example 1: `(9x + 3) / (12x + 4)`

To [[simplifying_expressions|simplify this expression]], first, [[factoring_polynomials|factor]] the numerator and the denominator <a class="yt-timestamp" data-t="00:01:37">[00:01:37]</a>:
*   **Numerator**: Factor out 3 from `9x + 3` to get `3(3x + 1)` <a class="yt-timestamp" data-t="00:01:39">[00:01:39]</a>.
*   **Denominator**: Factor out 4 from `12x + 4` to get `4(3x + 1)` <a class="yt-timestamp" data-t="00:01:49">[00:01:49]</a>.

The expression becomes `3(3x + 1) / 4(3x + 1)` <a class="yt-timestamp" data-t="00:02:04">[00:02:04]</a>.
Since `(3x + 1)` is a common factor in both the numerator and denominator, they cancel out <a class="yt-timestamp" data-t="00:02:09">[00:02:09]</a>. The simplified expression is `3/4` <a class="yt-timestamp" data-t="00:02:20">[00:02:20]</a>.

**Important Note on Equivalence**: When canceling variable expressions, it is crucial to state any values of the variable that would have made the original denominator zero <a class="yt-timestamp" data-t="00:03:21">[00:03:21]</a>. In this case, `3x + 1` would be zero if `x = -1/3` <a class="yt-timestamp" data-t="00:04:47">[00:04:47]</a>. Therefore, the simplified expression `3/4` is equivalent to the original `(9x + 3) / (12x + 4)` only if `x ≠ -1/3` <a class="yt-timestamp" data-t="00:05:00">[00:05:00]</a>.

### Example 2: `(x² - 9) / (5x + 15)`

*   **Numerator**: [[factoring_polynomials|Factor]] `x² - 9` as a difference of squares: `(x + 3)(x - 3)` <a class="yt-timestamp" data-t="00:02:58">[00:02:58]</a>.
*   **Denominator**: [[factoring_polynomials|Factor]] out 5 from `5x + 15`: `5(x + 3)` <a class="yt-timestamp" data-t="00:03:06">[00:03:06]</a>.

The expression becomes `(x + 3)(x - 3) / 5(x + 3)` <a class="yt-timestamp" data-t="00:03:12">[00:03:12]</a>.
Cancel the common factor `(x + 3)` <a class="yt-timestamp" data-t="00:03:12">[00:03:12]</a>. The result is `(x - 3) / 5` <a class="yt-timestamp" data-t="00:03:24">[00:03:24]</a>.

**Condition for Equivalence**: The original denominator `5(x + 3)` would be zero if `x = -3` <a class="yt-timestamp" data-t="00:03:33">[00:03:33]</a>. So, `(x - 3) / 5` is equivalent to the original expression only if `x ≠ -3` <a class="yt-timestamp" data-t="00:03:39">[00:03:39]</a>.

### Example 3: `(x² + 6x + 5) / (x² - x - 2)`

To [[simplifying_expressions|simplify this expression]], [[factoring_quadratic_polynomials|factor]] both quadratic expressions <a class="yt-timestamp" data-t="00:05:52">[00:05:52]</a>:
*   **Numerator (`x² + 6x + 5`)**: Find two numbers that multiply to 5 and add to 6 (which are 5 and 1) <a class="yt-timestamp" data-t="00:06:01">[00:06:01]</a>. So, `(x + 5)(x + 1)` <a class="yt-timestamp" data-t="00:06:09">[00:06:09]</a>.
*   **Denominator (`x² - x - 2`)**: Find two numbers that multiply to -2 and add to -1 (which are -2 and 1) <a class="yt-timestamp" data-t="00:06:17">[00:06:17]</a>. So, `(x - 2)(x + 1)` <a class="yt-timestamp" data-t="00:06:38">[00:06:38]</a>.

The expression becomes `(x + 5)(x + 1) / (x - 2)(x + 1)` <a class="yt-timestamp" data-t="00:06:46">[00:06:46]</a>.
Cancel the common factor `(x + 1)` <a class="yt-timestamp" data-t="00:06:46">[00:06:46]</a>. The simplified expression is `(x + 5) / (x - 2)` <a class="yt-timestamp" data-t="00:06:51">[00:06:51]</a>.

**Condition for Equivalence**: The original denominator `(x - 2)(x + 1)` would be zero if `x = 2` or `x = -1` <a class="yt-timestamp" data-t="00:07:00">[00:07:00]</a>. Therefore, `(x + 5) / (x - 2)` is equivalent to the original only if `x ≠ -1` <a class="yt-timestamp" data-t="00:07:00">[00:07:00]</a>. (Note: `x ≠ 2` is still implied by the simplified form, but `x ≠ -1` must be explicitly stated because the simplified form *is* defined at `x = -1`).

### Example 4: `(3x² + 3x - 18) / (2x² + 5x - 3)`

This example requires [[factoring_by_grouping|factoring by grouping]] for both the numerator and the denominator due to their leading coefficients not being 1 <a class="yt-timestamp" data-t="00:07:55">[00:07:55]</a>.

#### Factoring the Numerator: `3x² + 3x - 18`

1.  Find two numbers that multiply to `3 * -18 = -54` and add to `3` <a class="yt-timestamp" data-t="00:08:12">[00:08:12]</a>. These numbers are 9 and -6 <a class="yt-timestamp" data-t="00:08:41">[00:08:41]</a>.
2.  Rewrite the middle term (`3x`) using these numbers: `3x² + 9x - 6x - 18` <a class="yt-timestamp" data-t="00:08:54">[00:08:54]</a>.
3.  Group terms and factor:
    *   `3x(x + 3)` from `3x² + 9x` <a class="yt-timestamp" data-t="00:09:50">[00:09:50]</a>.
    *   `-6(x + 3)` from `-6x - 18` <a class="yt-timestamp" data-t="00:10:02">[00:10:02]</a>.
4.  [[factoring_polynomials|Factor]] out the common `(x + 3)`: `(3x - 6)(x + 3)` <a class="yt-timestamp" data-t="00:10:15">[00:10:15]</a>.

#### Factoring the Denominator: `2x² + 5x - 3`

1.  Find two numbers that multiply to `2 * -3 = -6` and add to `5` <a class="yt-timestamp" data-t="00:13:00">[00:13:00]</a>. These numbers are 6 and -1 <a class="yt-timestamp" data-t="00:13:12">[00:13:12]</a>.
2.  Rewrite the middle term (`5x`) using these numbers: `2x² + 6x - x - 3` <a class="yt-timestamp" data-t="00:13:28">[00:13:28]</a>.
3.  Group terms and factor:
    *   `2x(x + 3)` from `2x² + 6x` <a class="yt-timestamp" data-t="00:13:53">[00:13:53]</a>.
    *   `-1(x + 3)` from `-x - 3` <a class="yt-timestamp" data-t="00:14:02">[00:14:02]</a>.
4.  [[factoring_polynomials|Factor]] out the common `(x + 3)`: `(2x - 1)(x + 3)` <a class="yt-timestamp" data-t="00:14:11">[00:14:11]</a>.

#### Simplifying the Expression

The expression now becomes `(3x - 6)(x + 3) / (2x - 1)(x + 3)` <a class="yt-timestamp" data-t="00:14:28">[00:14:28]</a>.
Cancel the common factor `(x + 3)` <a class="yt-timestamp" data-t="00:14:40">[00:14:40]</a>. The simplified expression is `(3x - 6) / (2x - 1)` <a class="yt-timestamp" data-t="00:15:02">[00:15:02]</a>.

**Condition for Equivalence**: The original denominator `(2x - 1)(x + 3)` would be zero if `x = 1/2` or `x = -3` <a class="yt-timestamp" data-t="00:14:47">[00:14:47]</a>. Therefore, `(3x - 6) / (2x - 1)` is equivalent to the original only if `x ≠ -3` <a class="yt-timestamp" data-t="00:14:47">[00:14:47]</a>. (Note: `x ≠ 1/2` is still implied by the simplified form, but `x ≠ -3` must be explicitly stated).

By following these steps, you can [[simplifying_expressions|simplify rational expressions]] by canceling their common factors, always remembering to state any domain restrictions for the simplified expression to be truly equivalent to the original <a class="yt-timestamp" data-t="00:04:05">[00:04:05]</a>.