---
title: Combining like terms in equations
videoId: 9Ek61w1LxSc
---

From: [[khanacademy]] <br/> 

Algebraic equations often involve terms that can be grouped together to [[simplifying_expressions | simplify the expression]] <a class="yt-timestamp" data-t="00:09:45">[00:09:45]</a>. This process is known as combining like terms and is a crucial step in [[solving_equations_with_variables | solving equations with variables]] <a class="yt-timestamp" data-t="00:01:03">[00:01:03]</a>.

## Understanding the Basics of Equations

An equation states that two expressions are equal <a class="yt-timestamp" data-t="00:03:03">[00:03:03]</a>. For example, `7x = 14` means "7 times x is equal to 14" <a class="yt-timestamp" data-t="00:00:20">[00:00:20]</a>. In algebra, when a number (coefficient) is written next to a variable (like `x` or `y`), it signifies multiplication <a class="yt-timestamp" data-t="00:01:24">[00:01:24]</a>. This is a shorthand notation, as the traditional multiplication sign (`x`) can be confusing when `x` is also used as a variable <a class="yt-timestamp" data-t="00:01:33">[00:01:33]</a>.

While some simple equations, like `7x = 14`, can be solved by recalling times tables (e.g., `7 * 2 = 14`, so `x = 2`) <a class="yt-timestamp" data-t="00:00:41">[00:00:41]</a>, more complex equations require a systematic approach <a class="yt-timestamp" data-t="00:01:01">[00:01:01]</a>.

## The Concept of Combining Like Terms

[[combining_like_terms | Combining like terms]] involves grouping terms that contain the same variable raised to the same power. This can be visualized to understand the concept <a class="yt-timestamp" data-t="00:08:58">[00:08:58]</a>.

Consider the equation `2y + 4y = 18` <a class="yt-timestamp" data-t="00:08:16">[00:08:16]</a>.
*   `2y` literally means two `y`'s added together (`y + y`) <a class="yt-timestamp" data-t="00:09:04">[00:09:04]</a>.
*   `4y` means four `y`'s added together (`y + y + y + y`) <a class="yt-timestamp" data-t="00:09:15">[00:09:15]</a>.

So, `2y + 4y` can be seen as having "two y's plus four y's" <a class="yt-timestamp" data-t="00:09:50">[00:09:50]</a>. Just like "2 apples plus 4 apples equals 6 apples," "2 y's plus 4 y's equals 6 y's" <a class="yt-timestamp" data-t="00:10:00">[00:10:00]</a>.

Therefore, the expression `2y + 4y` simplifies to `6y` <a class="yt-timestamp" data-t="00:09:45">[00:09:45]</a>. This transforms the original equation into `6y = 18` <a class="yt-timestamp" data-t="00:10:07">[00:10:07]</a>.

## [[solving_linear_equations_with_additional_terms | Solving Equations]] After Combining Terms

Once like terms are combined, the equation often reduces to a simpler form, like `ax = b` (where 'a' is a coefficient, 'x' is the variable, and 'b' is a constant) <a class="yt-timestamp" data-t="00:03:55">[00:03:55]</a>. To solve for the variable, the standard step is to divide both sides of the equation by the coefficient of the variable <a class="yt-timestamp" data-t="00:04:01">[00:04:01]</a>. This is based on the principle that any [[operations_on_both_sides_of_an_equation | operation performed on one side of an equation]] must also be performed on the other side to maintain equality <a class="yt-timestamp" data-t="00:04:39">[00:04:39]</a>.

For `6y = 18`:
1.  Divide the left side by 6: `6y / 6 = y` <a class="yt-timestamp" data-t="00:10:18">[00:10:18]</a>.
2.  Divide the right side by 6: `18 / 6 = 3` <a class="yt-timestamp" data-t="00:10:29">[00:10:29]</a>.
3.  This yields `y = 3` <a class="yt-timestamp" data-t="00:10:31">[00:10:31]</a>.

Alternatively, dividing both sides by a number is [[reciprocal_multiplication_in_equations | equivalent to multiplying both sides by its reciprocal]] <a class="yt-timestamp" data-t="00:08:01">[00:08:01]</a>. So, for `6y = 18`, multiplying both sides by `1/6` would also result in `y = 3` <a class="yt-timestamp" data-t="00:07:28">[00:07:28]</a>.

## Checking Your Solution

A key advantage of [[understanding_equivalent_expressions_in_algebra | algebraic equations]] is the ability to check if your solution is correct <a class="yt-timestamp" data-t="00:10:40">[00:10:40]</a>. Substitute the found value of the variable back into the original equation.

For `2y + 4y = 18` with `y = 3`:
*   Substitute `y` with `3`: `2 * 3 + 4 * 3 = 18` <a class="yt-timestamp" data-t="00:10:45">[00:10:45]</a>
*   Calculate: `6 + 12 = 18` <a class="yt-timestamp" data-t="00:10:56">[00:10:56]</a>
*   Verify: `18 = 18` <a class="yt-timestamp" data-t="00:10:59">[00:10:59]</a>

Since both sides of the equation are equal, the solution `y = 3` is correct <a class="yt-timestamp" data-t="00:11:03">[00:11:03]</a>.