---
title: Common factors in rational expressions
videoId: 7Uos1ED3KHI
---

From: [[khanacademy]] <br/> 

Just as [[representations_of_rational_numbers | fractions]] or [[definition_of_rational_numbers | rational numbers]] can be put into lowest terms by finding common factors in the numerator and denominator, the same principle applies to rational expressions <a class="yt-timestamp" data-t="00:01:04">[00:01:04]</a>. Rational expressions are similar to rational numbers but involve variables in their numerators and/or denominators <a class="yt-timestamp" data-t="00:01:14">[00:01:14]</a>.

## How Common Factors Work

To [[simplifying_rational_expressions | simplify rational expressions]] by finding common factors:

1.  **Factor the Numerator and Denominator**: The first step is to completely [[factoring_quadratic_expressions | factor]] both the numerator and the denominator of the expression <a class="yt-timestamp" data-t="00:01:37">[00:01:37]</a>. This often involves techniques like factoring out a common monomial, recognizing a difference of squares, or [[factoring_quadratic_expressions | factoring quadratic expressions]] by grouping <a class="yt-timestamp" data-t="00:08:00">[00:08:00]</a>.
2.  **Identify Common Factors**: Look for any factors that are present in both the factored numerator and the factored denominator <a class="yt-timestamp" data-t="00:02:07">[00:02:07]</a>.
3.  **Cancel Common Factors**: Once identified, these common factors can be "cancelled out" by dividing both the numerator and the denominator by them <a class="yt-timestamp" data-t="00:02:26">[00:02:26]</a>. This is analogous to simplifying 3/6 to 1/2 by dividing both by 3 <a class="yt-timestamp" data-t="00:00:26">[00:00:26]</a>.

### Important Condition: Excluded Values

When simplifying rational expressions, it is crucial to remember that the original expression is undefined for any value of the variable that would make its denominator equal to zero <a class="yt-timestamp" data-t="00:03:33">[00:03:33]</a>. Even after cancelling common factors, the simplified expression is only equivalent to the original expression *if* these excluded values are explicitly stated <a class="yt-timestamp" data-t="00:03:52">[00:03:52]</a>. Failing to do so means the simplified expression might be defined at points where the original expression was not <a class="yt-timestamp" data-t="00:03:59">[00:03:59]</a>. This concept is important when [[graphing_rational_expressions | graphing rational expressions]], as excluded values due to cancelled factors often result in "holes" in the graph <a class="yt-timestamp" data-t="00:04:43">[00:04:43]</a>.

## Examples of Simplifying Rational Expressions

### Example 1: Linear Common Factors

Consider the expression:
```
(9x + 3) / (12x + 4)
```
1.  **Factor**:
    *   Numerator: Factor out 3 → `3(3x + 1)` <a class="yt-timestamp" data-t="00:01:40">[00:01:40]</a>
    *   Denominator: Factor out 4 → `4(3x + 1)` <a class="yt-timestamp" data-t="00:01:51">[00:01:51]</a>
    The expression becomes `3(3x + 1) / 4(3x + 1)` <a class="yt-timestamp" data-t="00:02:04">[00:02:04]</a>.
2.  **Identify Common Factor**: The common factor is `(3x + 1)` <a class="yt-timestamp" data-t="00:02:09">[00:02:09]</a>.
3.  **Cancel**:
    The expression simplifies to `3/4` <a class="yt-timestamp" data-t="00:02:23">[00:02:23]</a>.
4.  **Excluded Values**: The original denominator `12x + 4` would be zero if `3x + 1 = 0`, which means `x = -1/3`.
    Therefore, `(9x + 3) / (12x + 4) = 3/4`, where `x ≠ -1/3` <a class="yt-timestamp" data-t="00:05:00">[00:05:00]</a>.

### Example 2: Difference of Squares

Consider the expression:
```
(x² - 9) / (5x + 15)
```
1.  **Factor**:
    *   Numerator: This is a difference of squares → `(x + 3)(x - 3)` <a class="yt-timestamp" data-t="00:03:02">[00:03:02]</a>
    *   Denominator: Factor out 5 → `5(x + 3)` <a class="yt-timestamp" data-t="00:03:09">[00:03:09]</a>
    The expression becomes `(x + 3)(x - 3) / 5(x + 3)` <a class="yt-timestamp" data-t="00:03:12">[00:03:12]</a>.
2.  **Identify Common Factor**: The common factor is `(x + 3)` <a class="yt-timestamp" data-t="00:03:12">[00:03:12]</a>.
3.  **Cancel**:
    The expression simplifies to `(x - 3) / 5` <a class="yt-timestamp" data-t="00:03:24">[00:03:24]</a>.
4.  **Excluded Values**: The original denominator `5x + 15` would be zero if `x + 3 = 0`, which means `x = -3`.
    Therefore, `(x² - 9) / (5x + 15) = (x - 3) / 5`, where `x ≠ -3` <a class="yt-timestamp" data-t="00:03:42">[00:03:42]</a>.

### Example 3: Factoring Quadratic Expressions

Consider the expression:
```
(x² + 6x + 5) / (x² - x - 2)
```
1.  **Factor**:
    *   Numerator: For `x² + 6x + 5`, find two numbers that multiply to 5 and add to 6 (5 and 1). So, `(x + 5)(x + 1)` <a class="yt-timestamp" data-t="00:06:09">[00:06:09]</a>.
    *   Denominator: For `x² - x - 2`, find two numbers that multiply to -2 and add to -1 (-2 and 1). So, `(x - 2)(x + 1)` <a class="yt-timestamp" data-t="00:06:38">[00:06:38]</a>.
    The expression becomes `(x + 5)(x + 1) / (x - 2)(x + 1)` <a class="yt-timestamp" data-t="00:06:46">[00:06:46]</a>.
2.  **Identify Common Factor**: The common factor is `(x + 1)` <a class="yt-timestamp" data-t="00:06:46">[00:06:46]</a>.
3.  **Cancel**:
    The expression simplifies to `(x + 5) / (x - 2)` <a class="yt-timestamp" data-t="00:06:56">[00:06:56]</a>.
4.  **Excluded Values**: The original denominator `(x - 2)(x + 1)` would be zero if `x - 2 = 0` or `x + 1 = 0`. This means `x = 2` or `x = -1`.
    Therefore, `(x² + 6x + 5) / (x² - x - 2) = (x + 5) / (x - 2)`, where `x ≠ 2` and `x ≠ -1` <a class="yt-timestamp" data-t="00:07:00">[00:07:00]</a>.

### Example 4: Factoring Quadratics by Grouping

Consider the expression:
```
(3x² + 3x - 18) / (2x² + 5x - 3)
```
1.  **Factor Numerator** (`3x² + 3x - 18`):
    *   Find two numbers that multiply to `3 * -18 = -54` and add to `3` (9 and -6) <a class="yt-timestamp" data-t="00:08:14">[00:08:14]</a>.
    *   Rewrite `3x` as `9x - 6x` → `3x² + 9x - 6x - 18` <a class="yt-timestamp" data-t="00:09:03">[00:09:03]</a>.
    *   Group and factor: `3x(x + 3) - 6(x + 3)` <a class="yt-timestamp" data-t="00:09:56">[00:09:56]</a>.
    *   Factor out `(x + 3)` → `(3x - 6)(x + 3)` <a class="yt-timestamp" data-t="00:10:18">[00:10:18]</a>.
2.  **Factor Denominator** (`2x² + 5x - 3`):
    *   Find two numbers that multiply to `2 * -3 = -6` and add to `5` (6 and -1) <a class="yt-timestamp" data-t="00:13:00">[00:13:00]</a>.
    *   Rewrite `5x` as `6x - x` → `2x² + 6x - x - 3` <a class="yt-timestamp" data-t="00:13:34">[00:13:34]</a>.
    *   Group and factor: `2x(x + 3) - 1(x + 3)` <a class="yt-timestamp" data-t="00:13:57">[00:13:57]</a>.
    *   Factor out `(x + 3)` → `(2x - 1)(x + 3)` <a class="yt-timestamp" data-t="00:14:11">[00:14:11]</a>.
    The expression becomes `(3x - 6)(x + 3) / (2x - 1)(x + 3)` <a class="yt-timestamp" data-t="00:14:28">[00:14:28]</a>.
3.  **Identify Common Factor**: The common factor is `(x + 3)` <a class="yt-timestamp" data-t="00:14:40">[00:14:40]</a>.
4.  **Cancel**:
    The expression simplifies to `(3x - 6) / (2x - 1)` <a class="yt-timestamp" data-t="00:15:09">[00:15:09]</a>.
5.  **Excluded Values**: The original denominator `(2x - 1)(x + 3)` would be zero if `2x - 1 = 0` or `x + 3 = 0`. This means `x = 1/2` or `x = -3`.
    Therefore, `(3x² + 3x - 18) / (2x² + 5x - 3) = (3x - 6) / (2x - 1)`, where `x ≠ 1/2` and `x ≠ -3` <a class="yt-timestamp" data-t="00:15:14">[00:15:14]</a>.