---
title: Completing the square and derivation of the quadratic formula
videoId: i7idZfS8t8w
---

From: [[khanacademy]] <br/> 

The [[introduction_to_the_quadratic_formula | quadratic formula]] is considered one of the most useful formulas in mathematics <a class="yt-timestamp" data-t="00:00:04">[00:00:04]</a>. While memorization is recommended, it's also important to understand its proof and origin <a class="yt-timestamp" data-t="00:00:13">[00:00:13]</a>.

## Purpose of the Quadratic Formula
The [[introduction_to_the_quadratic_formula | quadratic formula]] is used to solve for the roots, or zeroes, of [[solving_quadratic_equations_using_the_quadratic_formula | quadratic equations]] <a class="yt-timestamp" data-t="00:00:32">[00:00:32]</a>.

## General Form of a Quadratic Equation
A general [[solving_quadratic_equations_using_the_quadratic_formula | quadratic equation]] is expressed in the form:
`ax² + bx + c = 0` <a class="yt-timestamp" data-t="00:00:44">[00:00:44]</a>

In this form:
*   `a` is the coefficient of the `x²` (or second-degree) term <a class="yt-timestamp" data-t="00:00:59">[00:00:59]</a>.
*   `b` is the coefficient of the `x` term <a class="yt-timestamp" data-t="00:01:02">[00:01:02]</a>.
*   `c` is the constant term (or coefficient on the `x` to the zero term) <a class="yt-timestamp" data-t="00:01:05">[00:01:05]</a>.

## The Quadratic Formula
Given a general [[solving_quadratic_equations_using_the_quadratic_formula | quadratic equation]] `ax² + bx + c = 0`, the [[introduction_to_the_quadratic_formula | quadratic formula]] provides its solutions for `x` as:
`x = (-b ± √(b² - 4ac)) / 2a` <a class="yt-timestamp" data-t="00:01:16">[00:01:16]</a>

Although it may appear complex initially, it becomes a more manageable formula with practice <a class="yt-timestamp" data-t="00:01:34">[00:01:34]</a>.

## Derivation of the Quadratic Formula
The [[introduction_to_the_quadratic_formula | quadratic formula]] is derived directly from applying the technique of [[completing_the_square_as_a_technique_for_solving_quadratic_equations | completing the square]] to the general [[solving_quadratic_equations_using_the_quadratic_formula | quadratic equation]] `ax² + bx + c = 0` <a class="yt-timestamp" data-t="00:01:54">[00:01:54]</a>. If one were to [[completing_the_square_as_a_technique_for_solving_quadratic_equations | complete the square]] on this equation, the result would be the [[introduction_to_the_quadratic_formula | quadratic formula]] itself <a class="yt-timestamp" data-t="00:01:58">[00:01:58]</a>. The full derivation is typically covered in subsequent lessons <a class="yt-timestamp" data-t="00:01:49">[00:01:49]</a>.

## Examples and Applications
The [[introduction_to_the_quadratic_formula | quadratic formula]] can be applied to solve [[solving_quadratic_equations_using_the_quadratic_formula | quadratic equations]], including those that are difficult to [[factoring_quadratic_expressions | factor]] <a class="yt-timestamp" data-t="00:05:45">[00:05:45]</a>.

### Example 1: `x² + 4x - 21 = 0`
To solve `x² + 4x - 21 = 0` using the [[introduction_to_the_quadratic_formula | quadratic formula]]:
1.  Identify coefficients: `a = 1` <a class="yt-timestamp" data-t="00:02:30">[00:02:30]</a>, `b = 4` <a class="yt-timestamp" data-t="00:02:37">[00:02:37]</a>, `c = -21` <a class="yt-timestamp" data-t="00:02:40">[00:02:40]</a>.
2.  Plug into the formula:
    `x = (-4 ± √(4² - 4 * 1 * -21)) / (2 * 1)` <a class="yt-timestamp" data-t="00:02:49">[00:02:49]</a>
3.  Simplify:
    `x = (-4 ± √(16 + 84)) / 2` <a class="yt-timestamp" data-t="00:03:45">[00:03:45]</a>
    `x = (-4 ± √100) / 2` <a class="yt-timestamp" data-t="00:04:03">[00:04:03]</a>
    `x = (-4 ± 10) / 2` <a class="yt-timestamp" data-t="00:04:09">[00:04:09]</a>
    `x = -2 ± 5` <a class="yt-timestamp" data-t="00:04:23">[00:04:23]</a>
4.  The solutions are:
    *   `x = -2 + 5 = 3` <a class="yt-timestamp" data-t="00:04:32">[00:04:32]</a>
    *   `x = -2 - 5 = -7` <a class="yt-timestamp" data-t="00:04:38">[00:04:38]</a>

This result is consistent with [[factoring_quadratic_expressions | factoring]] the equation `(x + 7)(x - 3) = 0`, which yields `x = -7` or `x = 3` <a class="yt-timestamp" data-t="00:05:04">[00:05:04]</a>.

### Example 2: `3x² + 6x = -10`
First, rearrange the equation to the standard form `ax² + bx + c = 0`:
`3x² + 6x + 10 = 0` <a class="yt-timestamp" data-t="00:06:31">[00:06:31]</a>

1.  Identify coefficients: `a = 3` <a class="yt-timestamp" data-t="00:06:51">[00:06:51]</a>, `b = 6` <a class="yt-timestamp" data-t="00:06:53">[00:06:53]</a>, `c = 10` <a class="yt-timestamp" data-t="00:06:57">[00:06:57]</a>.
2.  Plug into the formula:
    `x = (-6 ± √(6² - 4 * 3 * 10)) / (2 * 3)` <a class="yt-timestamp" data-t="00:07:10">[00:07:10]</a>
3.  Simplify:
    `x = (-6 ± √(36 - 120)) / 6` <a class="yt-timestamp" data-t="00:07:42">[00:07:42]</a>
    `x = (-6 ± √(-84)) / 6` <a class="yt-timestamp" data-t="00:08:36">[00:08:36]</a>

In this case, the expression under the square root (`b² - 4ac`), known as the discriminant, is negative (`-84`) <a class="yt-timestamp" data-t="00:08:46">[00:08:46]</a>. This indicates that the equation has no real solutions <a class="yt-timestamp" data-t="00:09:06">[00:09:06]</a>. Graphing the function `y = 3x² + 6x + 10` would show that it never intersects the x-axis, confirming no real roots <a class="yt-timestamp" data-t="00:10:27">[00:10:27]</a>. Solutions involving the square root of a negative number are called imaginary numbers <a class="yt-timestamp" data-t="00:09:17">[00:09:17]</a>.

### Example 3: `-3x² + 12x + 1 = 0`
1.  Identify coefficients: `a = -3` <a class="yt-timestamp" data-t="00:11:09">[00:11:09]</a>, `b = 12` <a class="yt-timestamp" data-t="00:11:12">[00:11:12]</a>, `c = 1` <a class="yt-timestamp" data-t="00:11:29">[00:11:29]</a>.
2.  Plug into the formula:
    `x = (-12 ± √(12² - 4 * -3 * 1)) / (2 * -3)` <a class="yt-timestamp" data-t="00:11:07">[00:11:07]</a>
3.  Simplify:
    `x = (-12 ± √(144 + 12)) / -6` <a class="yt-timestamp" data-t="00:11:43">[00:11:43]</a>
    `x = (-12 ± √156) / -6` <a class="yt-timestamp" data-t="00:11:51">[00:11:51]</a>
4.  Simplify the radical `√156`:
    `√156 = √(4 * 39) = 2√39` <a class="yt-timestamp" data-t="00:12:39">[00:12:39]</a>
5.  Substitute back and simplify:
    `x = (-12 ± 2√39) / -6` <a class="yt-timestamp" data-t="00:13:10">[00:13:10]</a>
    Divide numerator and denominator by 2:
    `x = (-6 ± √39) / -3` <a class="yt-timestamp" data-t="00:13:26">[00:13:26]</a>
    Separating terms:
    `x = (-6 / -3) ± (√39 / -3)` <a class="yt-timestamp" data-t="00:13:38">[00:13:38]</a>
    `x = 2 ± (√39 / -3)` <a class="yt-timestamp" data-t="00:13:49">[00:13:49]</a>
    Which simplifies to:
    `x = 2 ± (√39 / 3)` <a class="yt-timestamp" data-t="00:15:07">[00:15:07]</a>

The two solutions are `x = 2 + √39/3` and `x = 2 - √39/3` <a class="yt-timestamp" data-t="00:15:07">[00:15:07]</a>.