---
title: Elimination method in algebra
videoId: vA-55wZtLeE
---

From: [[khanacademy]] <br/> 

The [[algebraic_methods_in_algebra | elimination method]] is a technique used to solve [[algebraic_methods_in_algebra | systems of equations]] <a class="yt-timestamp" data-t="00:00:02">[00:00:02]</a>. The goal of this method is to [[substitution_vs_elimination_methods | eliminate]] one of the variables, allowing you to solve for the remaining variable in a single equation <a class="yt-timestamp" data-t="00:01:03">[00:01:03]</a>. Graphically, the solution represents the point of intersection of the lines defined by each equation <a class="yt-timestamp" data-t="00:00:31">[00:00:31]</a>.

## How the Elimination Method Works

The core principle of the elimination method is that you can add or subtract one entire equation from another, as long as you perform the same operation on both sides of the equation <a class="yt-timestamp" data-t="00:01:17">[00:01:17]</a>. This is permissible because if two quantities are equal, adding or subtracting one to both sides of another equation maintains the equality <a class="yt-timestamp" data-t="00:02:30">[00:02:30]</a>.

### Example 1: Adding Equations

Consider the following system of equations:
1.  `3x + 4y = 2.5` <a class="yt-timestamp" data-t="00:00:04">[00:00:04]</a>
2.  `5x - 4y = 25.5` <a class="yt-timestamp" data-t="00:00:12">[00:00:12]</a>

Notice that the `y` terms have coefficients that are opposites (`+4y` and `-4y`) <a class="yt-timestamp" data-t="00:03:08">[00:03:08]</a>. This makes them ideal for elimination by addition.

To solve this system using elimination:
1.  **Add the left-hand sides together and the right-hand sides together:**
    `(3x + 4y) + (5x - 4y) = 2.5 + 25.5` <a class="yt-timestamp" data-t="00:02:55">[00:02:55]</a>
2.  **Combine like terms:**
    `8x + 0y = 28` <a class="yt-timestamp" data-t="00:02:57">[00:02:57]</a>
    `8x = 28` <a class="yt-timestamp" data-t="00:03:26">[00:03:26]</a>
3.  **Solve for x:**
    `x = 28 / 8` <a class="yt-timestamp" data-t="00:03:30">[00:03:30]</a>
    `x = 7/2` (or 3.5) <a class="yt-timestamp" data-t="00:03:43">[00:03:43]</a>
4.  **Substitute the x-value back into either original equation to solve for y:**
    Using the first equation: `3(7/2) + 4y = 2.5` <a class="yt-timestamp" data-t="00:04:11">[00:04:11]</a>
    `21/2 + 4y = 5/2` (2.5 written as a fraction) <a class="yt-timestamp" data-t="00:04:21">[00:04:21]</a>
    `4y = 5/2 - 21/2` <a class="yt-timestamp" data-t="00:04:28">[00:04:28]</a>
    `4y = -16/2` <a class="yt-timestamp" data-t="00:04:47">[00:04:47]</a>
    `4y = -8` <a class="yt-timestamp" data-t="00:05:06">[00:05:06]</a>
    `y = -2` <a class="yt-timestamp" data-t="00:05:13">[00:05:13]</a>

Thus, the solution is `x = 7/2` and `y = -2` <a class="yt-timestamp" data-t="00:05:16">[00:05:16]</a>. You can [[checking_solutions_in_algebra | check solutions]] by substituting these values back into the other original equation <a class="yt-timestamp" data-t="00:05:29">[00:05:29]</a>.

## Application: Solving Word Problems

The elimination method is particularly useful for [[word_problems_in_algebra | word problems in algebra]] that translate into systems of equations <a class="yt-timestamp" data-t="00:06:02">[00:06:02]</a>.

### Example 2: Candy Store Purchase

**Problem:** Nadia buys 3 candy bars and 4 Fruit Roll-Ups for $2.84. Peter buys 3 candy bars and 1 Fruit Roll-Up for $1.79. What is the cost of each candy bar and each Fruit Roll-Up? <a class="yt-timestamp" data-t="00:06:07">[00:06:07]</a>

1.  **Define variables:**
    *   Let `x` = cost of a candy bar <a class="yt-timestamp" data-t="00:06:33">[00:06:33]</a>
    *   Let `y` = cost of a Fruit Roll-Up <a class="yt-timestamp" data-t="00:06:46">[00:06:46]</a>

2.  **Formulate equations:**
    *   Nadia's purchase: `3x + 4y = 2.84` <a class="yt-timestamp" data-t="00:07:00">[00:07:00]</a>
    *   Peter's purchase: `3x + 1y = 1.79` <a class="yt-timestamp" data-t="00:07:29">[00:07:29]</a>

3.  **Eliminate a variable using subtraction:**
    Notice that the `x` terms have the same coefficient (`3x`). To eliminate `x`, you can subtract the second equation from the first <a class="yt-timestamp" data-t="00:08:22">[00:08:22]</a>. This is equivalent to multiplying the second equation by -1 and then adding it to the first <a class="yt-timestamp" data-t="00:09:23">[00:09:23]</a>.

    Subtracting (or adding the negative of the second equation):
    `(3x + 4y) - (3x + y) = 2.84 - 1.79` <a class="yt-timestamp" data-t="00:09:45">[00:09:45]</a>
    `3x - 3x + 4y - y = 1.05`
    `0x + 3y = 1.05` <a class="yt-timestamp" data-t="00:09:50">[00:09:50]</a>
    `3y = 1.05` <a class="yt-timestamp" data-t="00:10:12">[00:10:12]</a>

4.  **Solve for y:**
    `y = 1.05 / 3` <a class="yt-timestamp" data-t="00:10:15">[00:10:15]</a>
    `y = 0.35` <a class="yt-timestamp" data-t="00:10:54">[00:10:54]</a>
    So, a Fruit Roll-Up costs $0.35 <a class="yt-timestamp" data-t="00:10:57">[00:10:57]</a>.

5.  **Substitute the y-value back into either original equation to solve for x:**
    Using Peter's equation (`3x + y = 1.79`): <a class="yt-timestamp" data-t="00:11:12">[00:11:12]</a>
    `3x + 0.35 = 1.79` <a class="yt-timestamp" data-t="00:11:22">[00:11:22]</a>
    `3x = 1.79 - 0.35` <a class="yt-timestamp" data-t="00:11:32">[00:11:32]</a>
    `3x = 1.44` <a class="yt-timestamp" data-t="00:11:45">[00:11:45]</a>
    `x = 1.44 / 3` <a class="yt-timestamp" data-t="00:11:52">[00:11:52]</a>
    `x = 0.48` <a class="yt-timestamp" data-t="00:12:26">[00:12:26]</a>
    So, a candy bar costs $0.48 <a class="yt-timestamp" data-t="00:12:34">[00:12:34]</a>.

### Key Takeaways

*   The elimination method is an efficient way to solve systems of linear equations <a class="yt-timestamp" data-t="00:00:02">[00:00:02]</a>.
*   It relies on adding or subtracting entire equations to eliminate one variable <a class="yt-timestamp" data-t="00:01:17">[00:01:17]</a>.
*   The fundamental rule is that you must add or subtract the same value to both sides of an equation to maintain its equality <a class="yt-timestamp" data-t="00:01:50">[00:01:50]</a>.
*   This method is particularly useful when variables already have opposing or identical coefficients, or can be easily manipulated to do so <a class="yt-timestamp" data-t="00:03:08">[00:03:08]</a>.
*   After finding one variable, substitute its value back into an original equation to find the other variable <a class="yt-timestamp" data-t="00:03:51">[00:03:51]</a>.