---
title: Evaluating expressions with different variable values
videoId: vDqOoI-4Z6M
---

From: [[khanacademy]] <br/> 

When performing basic arithmetic, we deal with concrete numbers like 23 + 5, which immediately yields 28. Similarly, 2 times 7 or 3 divided by 4 involve known numerical values <a class="yt-timestamp" data-t="00:00:00">[00:00:00]</a>.

As we transition into algebra, we begin working with variables <a class="yt-timestamp" data-t="00:00:20">[00:00:20]</a>. Variables represent values within [[understanding_algebraic_expressions | expressions]] that can change <a class="yt-timestamp" data-t="00:00:30">[00:00:30]</a>.

## Understanding Variables in Expressions

Consider the expression `x + 5` <a class="yt-timestamp" data-t="00:00:38">[00:00:38]</a>. The value of this expression depends on the value assigned to `x` <a class="yt-timestamp" data-t="00:00:46">[00:00:46]</a>.

*   If `x` is equal to 1, then `x + 5` becomes `1 + 5`, which evaluates to 6 <a class="yt-timestamp" data-t="00:00:51">[00:00:51]</a>.
*   If `x` is equal to -7, then `x + 5` becomes `-7 + 5`, which evaluates to -2 <a class="yt-timestamp" data-t="00:01:11">[00:01:11]</a>.

In this example, `x` is a variable, and its value can change depending on the specific context of the problem <a class="yt-timestamp" data-t="00:01:28">[00:01:28]</a>.

## [[difference_between_expressions_and_equations | Distinction Between Expressions and Equations]]

It's important to understand the [[difference_between_expressions_and_equations | distinction between an expression and an equation]] <a class="yt-timestamp" data-t="00:01:42">[00:01:42]</a>.

*   **Expression**: An [[understanding_algebraic_expressions | expression]] is a statement of value or quantity <a class="yt-timestamp" data-t="00:01:46">[00:01:46]</a>. Examples include `x + 5` or `y + z` <a class="yt-timestamp" data-t="00:02:09">[00:02:09]</a>. The value of an expression changes based on the values of its variables <a class="yt-timestamp" data-t="00:01:59">[00:01:59]</a>.
*   **Equation**: An equation sets two or more expressions equal to each other <a class="yt-timestamp" data-t="00:02:32">[00:02:32]</a>. For example, `x + 3 = 1` <a class="yt-timestamp" data-t="00:02:44">[00:02:44]</a>. In this case, if there's only one unknown, the equation can constrain the variable to a specific value (here, `x` must be -2) <a class="yt-timestamp" data-t="00:02:52">[00:02:52]</a>.

Equations do not always constrain variables to a single value. For instance, in the equation `x + y + z = 5`, if `y = 3` and `z = 2` are given, then the equation becomes `x + 3 + 2 = 5`, which simplifies to `x + 5 = 5`. This constrains `x` to be 0 <a class="yt-timestamp" data-t="00:03:17">[00:03:17]</a>.

The key takeaway is that a variable's value can vary depending on the context of the problem, whether it's within an expression or an equation <a class="yt-timestamp" data-t="00:04:20">[00:04:20]</a>.

## Evaluating Expressions with Different Variable Values

To further illustrate, let's evaluate various expressions by substituting different values for their variables <a class="yt-timestamp" data-t="00:04:31">[00:04:31]</a>.

### Example 1: `x` to the power of `y` (`x^y`)

*   **Expression**: `x^y` <a class="yt-timestamp" data-t="00:04:38">[00:04:38]</a>
    *   If `x = 5` and `y = 2`, the expression evaluates to `5^2`, which is 25 <a class="yt-timestamp" data-t="00:04:47">[00:04:47]</a>.
    *   If `x = -2` and `y = 3`, the expression evaluates to `(-2)^3`, which is `-2 * -2 * -2 = -8` <a class="yt-timestamp" data-t="00:05:16">[00:05:16]</a>.

### Example 2: Square root of (`x + y`) minus `x`

*   **Expression**: `√(x + y) - x` <a class="yt-timestamp" data-t="00:05:58">[00:05:58]</a>
    *   If `x = 1` and `y = 8` <a class="yt-timestamp" data-t="00:06:09">[00:06:09]</a>:
        *   Substitute `x` with 1 and `y` with 8 <a class="yt-timestamp" data-t="00:06:18">[00:06:18]</a>.
        *   `√(1 + 8) - 1` <a class="yt-timestamp" data-t="00:06:32">[00:06:32]</a>
        *   `√9 - 1` <a class="yt-timestamp" data-t="00:06:34">[00:06:34]</a>
        *   `3 - 1` <a class="yt-timestamp" data-t="00:06:48">[00:06:48]</a>
        *   The expression evaluates to 2 <a class="yt-timestamp" data-t="00:06:48">[00:06:48]</a>.