---
title: Example problems using substitution method
videoId: V7H1oUHXPkg
---

From: [[khanacademy]] <br/> 

This article demonstrates how to solve [[systematic_approach_to_solving_equations | systems of equations]] algebraically using the [[substitution_method_for_solving_linear_systems | substitution method]] <a class="yt-timestamp" data-t="00:00:06">[00:00:06]</a>. This technique provides an exact algebraic answer, unlike graphical methods which can make it hard to figure out exact intersection points <a class="yt-timestamp" data-t="00:00:13">[00:00:13]</a>.

## How the Substitution Method Works

The core idea of the [[substitution_method_for_solving_linear_systems | substitution method]] is to use one equation to [[using_algebraic_steps_to_solve_equations | solve for one of the variables]], and then [[using_substitution_to_verify_algebraic_solutions | substitute]] that expression back into the other equation <a class="yt-timestamp" data-t="00:00:59">[00:00:59]</a>. This results in one equation with one unknown, which can then be easily solved <a class="yt-timestamp" data-t="00:02:18">[00:02:18]</a>.

## Example 1: Solving a System of Linear Equations

Consider the following [[solving_systems_of_equations_using_elimination | system of equations]]:
1.  `x + 2y = 9` <a class="yt-timestamp" data-t="00:00:19">[00:00:19]</a>
2.  `3x + 5y = 20` <a class="yt-timestamp" data-t="00:00:27">[00:00:27]</a>

### Step 1: Isolate a Variable in One Equation
Choose one of the equations and [[using_algebraic_steps_to_solve_equations | solve for one variable]]. From the first equation (`x + 2y = 9`), we can [[using_algebraic_steps_to_solve_equations | solve for x]] by [[using_subtraction_in_equations | subtracting 2y]] from both sides <a class="yt-timestamp" data-t="00:01:16">[00:01:16]</a>:
`x = 9 - 2y` <a class="yt-timestamp" data-t="00:01:22">[00:01:22]</a>

### Step 2: Substitute the Expression into the Other Equation
Now, [[using_substitution_to_verify_algebraic_solutions | substitute]] `(9 - 2y)` for `x` in the second equation (`3x + 5y = 20`) <a class="yt-timestamp" data-t="00:01:52">[00:01:52]</a>:
`3 * (9 - 2y) + 5y = 20` <a class="yt-timestamp" data-t="00:02:07">[00:02:07]</a>

### Step 3: Solve the Resulting Equation
Distribute the 3 and combine like terms to [[using_algebraic_steps_to_solve_equations | solve for y]] <a class="yt-timestamp" data-t="00:02:20">[00:02:20]</a>:
`27 - 6y + 5y = 20` <a class="yt-timestamp" data-t="00:02:25">[00:02:25]</a>
`27 - y = 20` <a class="yt-timestamp" data-t="00:02:39">[00:02:39]</a>
[[using_subtraction_in_equations | Subtract 27]] from both sides <a class="yt-timestamp" data-t="00:02:45">[00:02:45]</a>:
`-y = -7` <a class="yt-timestamp" data-t="00:02:59">[00:02:59]</a>
Multiply by -1 to find `y` <a class="yt-timestamp" data-t="00:03:04">[00:03:04]</a>:
`y = 7` <a class="yt-timestamp" data-t="00:03:07">[00:03:07]</a>

### Step 4: Substitute Back to Find the Other Variable
Now that `y = 7` is known, [[using_substitution_to_verify_algebraic_solutions | substitute]] this value back into the expression for `x` (`x = 9 - 2y`) <a class="yt-timestamp" data-t="00:03:29">[00:03:29]</a>:
`x = 9 - 2 * (7)` <a class="yt-timestamp" data-t="00:03:36">[00:03:36]</a>
`x = 9 - 14` <a class="yt-timestamp" data-t="00:03:42">[00:03:42]</a>
`x = -5` <a class="yt-timestamp" data-t="00:03:42">[00:03:42]</a>

### Solution and Verification
The solution is `x = -5` and `y = 7` <a class="yt-timestamp" data-t="00:03:57">[00:03:57]</a>. This means if the two original equations were graphed as lines, they would intersect at the point `(-5, 7)` <a class="yt-timestamp" data-t="00:04:26">[00:04:26]</a>.

To [[using_substitution_to_verify_algebraic_solutions | verify]] this solution, [[using_substitution_to_verify_algebraic_solutions | substitute]] the values into both original equations <a class="yt-timestamp" data-t="00:04:02">[00:04:02]</a>:
*   For `x + 2y = 9`: `-5 + 2 * (7) = -5 + 14 = 9` (True) <a class="yt-timestamp" data-t="00:04:04">[00:04:04]</a>
*   For `3x + 5y = 20`: `3 * (-5) + 5 * (7) = -15 + 35 = 20` (True) <a class="yt-timestamp" data-t="00:04:12">[00:04:12]</a>
Since both equations are satisfied, the solution is correct <a class="yt-timestamp" data-t="00:04:24">[00:04:24]</a>.

## Example 2: Word Problem Application

The [[substitution_method_for_solving_linear_systems | substitution method]] is also useful for [[word_problems_involving_systems_of_equations | word problems involving systems of equations]] <a class="yt-timestamp" data-t="00:04:38">[00:04:38]</a>.

**Problem:** The sum of two numbers is 70, and they differ by 11. What are the numbers? <a class="yt-timestamp" data-t="00:04:40">[00:04:40]</a>

### Step 1: Define Variables and Formulate Equations
Let `x` be the larger number and `y` be the smaller number <a class="yt-timestamp" data-t="00:05:18">[00:05:18]</a>.
*   "The sum of two numbers is 70" translates to: `x + y = 70` <a class="yt-timestamp" data-t="00:05:39">[00:05:39]</a>
*   "They differ by 11" translates to: `x - y = 11` <a class="yt-timestamp" data-t="00:05:51">[00:05:51]</a>

This gives us the [[solving_systems_of_equations_using_elimination | system of equations]]:
1.  `x + y = 70`
2.  `x - y = 11`

### Step 2: Isolate a Variable
From the second equation (`x - y = 11`), [[using_algebraic_steps_to_solve_equations | solve for x]] by adding `y` to both sides <a class="yt-timestamp" data-t="00:06:15">[00:06:15]</a>:
`x = 11 + y` <a class="yt-timestamp" data-t="00:06:33">[00:06:33]</a>

### Step 3: Substitute and Solve
[[using_substitution_to_verify_algebraic_solutions | Substitute]] `(11 + y)` for `x` in the first equation (`x + y = 70`) <a class="yt-timestamp" data-t="00:06:40">[00:06:40]</a>:
`(11 + y) + y = 70` <a class="yt-timestamp" data-t="00:07:00">[00:07:00]</a>
`11 + 2y = 70` <a class="yt-timestamp" data-t="00:07:32">[00:07:32]</a>
[[using_subtraction_in_equations | Subtract 11]] from both sides <a class="yt-timestamp" data-t="00:07:36">[00:07:36]</a>:
`2y = 59` <a class="yt-timestamp" data-t="00:07:45">[00:07:45]</a>
`y = 59 / 2` <a class="yt-timestamp" data-t="00:07:51">[00:07:51]</a>
`y = 29.5` <a class="yt-timestamp" data-t="00:08:10">[00:08:10]</a>

### Step 4: Substitute Back
[[using_substitution_to_verify_algebraic_solutions | Substitute]] `y = 29.5` back into `x = 11 + y` <a class="yt-timestamp" data-t="00:08:17">[00:08:17]</a>:
`x = 11 + 29.5` <a class="yt-timestamp" data-t="00:08:21">[00:08:21]</a>
`x = 40.5` <a class="yt-timestamp" data-t="00:08:32">[00:08:32]</a>

### Solution and Verification
The two numbers are `40.5` and `29.5` <a class="yt-timestamp" data-t="00:08:36">[00:08:36]</a>.

To [[using_substitution_to_verify_algebraic_solutions | verify]]:
*   Sum: `40.5 + 29.5 = 70` (True) <a class="yt-timestamp" data-t="00:09:07">[00:09:07]</a>
*   Difference: `40.5 - 29.5 = 11` (True) <a class="yt-timestamp" data-t="00:09:11">[00:09:11]</a>
Both conditions are met <a class="yt-timestamp" data-t="00:09:15">[00:09:15]</a>.

### Key Takeaway
Regardless of which variable or equation you choose to start with, the important thing is to use both constraints provided by the [[solving_systems_of_equations_using_elimination | system of equations]] <a class="yt-timestamp" data-t="00:08:48">[00:08:48]</a>.