---
title: Factoring quadratics
videoId: eF6zYNzlZKQ
---

From: [[khanacademy]] <br/> 

[[factoring_quadratic_equations|Factoring a second degree polynomial]], often called a [[quadratic_polynomials|quadratic]] or [[quadratic_polynomials|quadratic expression]], involves breaking it down into a product of simpler terms, typically two binomials <a class="yt-timestamp" data-t="00:00:00">[00:00:00]</a>. A [[quadratic_polynomials|quadratic]] is any [[quadratic_polynomials|polynomial]] where the highest power of the variable (e.g., x) is the second power <a class="yt-timestamp" data-t="00:00:15">[00:00:15]</a>.

## The Basic Principle

To understand how to factor, consider the multiplication of two binomials: `(x + a)` and `(x + b)` <a class="yt-timestamp" data-t="00:00:44">[00:00:44]</a>.

Multiplying these gives:
`x * x` = `x²` <a class="yt-timestamp" data-t="00:00:57">[00:00:57]</a>
`x * b` = `bx` <a class="yt-timestamp" data-t="00:01:00">[00:01:00]</a>
`a * x` = `ax` <a class="yt-timestamp" data-t="00:01:03">[00:01:03]</a>
`a * b` = `ab` <a class="yt-timestamp" data-t="00:01:04">[00:01:04]</a>

Combining these terms results in: `x² + bx + ax + ab` <a class="yt-timestamp" data-t="00:01:00">[00:01:00]</a>
This can be rewritten as: `x² + (a + b)x + ab` <a class="yt-timestamp" data-t="00:01:22">[00:01:22]</a>

From this general form, we observe that for a [[quadratic_polynomials|quadratic]] in the form `x² + cx + d`:
*   The coefficient of the x term (the "first degree coefficient") is the sum of `a` and `b` (`c = a + b`) <a class="yt-timestamp" data-t="00:01:40">[00:01:40]</a>.
*   The constant term is the product of `a` and `b` (`d = ab`) <a class="yt-timestamp" data-t="00:01:49">[00:01:49]</a>.

Therefore, when [[factoring_quadratic_equations|factoring a quadratic]] where the [[understanding_components_of_a_quadratic_equation|coefficient on the x² term]] is 1, the goal is to find two numbers (`a` and `b`) that add up to the [[understanding_components_of_a_quadratic_equation|coefficient of the x term]] and multiply to the [[understanding_components_of_a_quadratic_equation|constant term]] <a class="yt-timestamp" data-t="00:03:31">[00:03:31]</a>.

## Examples of Factoring Quadratics

### Example 1: All Positive Terms

**Problem:** Factor `x² + 10x + 9` <a class="yt-timestamp" data-t="00:00:30">[00:00:30]</a>

**Solution:**
We need two numbers that:
*   Add up to 10 (`a + b = 10`) <a class="yt-timestamp" data-t="00:02:05">[00:02:05]</a>
*   Multiply to 9 (`a * b = 9`) <a class="yt-timestamp" data-t="00:02:14">[00:02:14]</a>

Consider factors of 9:
*   1 and 9 <a class="yt-timestamp" data-t="00:02:40">[00:02:40]</a>
*   3 and 3 <a class="yt-timestamp" data-t="00:02:40">[00:02:40]</a>

*   If `a = 3, b = 3`: `3 + 3 = 6` (not 10) <a class="yt-timestamp" data-t="00:02:45">[00:02:45]</a>
*   If `a = 1, b = 9`: `1 * 9 = 9` and `1 + 9 = 10` <a class="yt-timestamp" data-t="00:02:49">[00:02:49]</a>. This works!

**Factored form:** `(x + 1)(x + 9)` <a class="yt-timestamp" data-t="00:03:04">[00:03:04]</a>

---

### Example 2: Larger Coefficients

**Problem:** Factor `x² + 15x + 50` <a class="yt-timestamp" data-t="00:04:11">[00:04:11]</a>

**Solution:**
We need two numbers that:
*   Add up to 15 <a class="yt-timestamp" data-t="00:04:35">[00:04:35]</a>
*   Multiply to 50 <a class="yt-timestamp" data-t="00:04:35">[00:04:35]</a>

Consider factors of 50:
*   1 and 50 (sum = 51) <a class="yt-timestamp" data-t="00:04:48">[00:04:48]</a>
*   2 and 25 (sum = 27) <a class="yt-timestamp" data-t="00:04:52">[00:04:52]</a>
*   5 and 10 (sum = 15) <a class="yt-timestamp" data-t="00:04:57">[00:04:57]</a>. This works!

**Factored form:** `(x + 5)(x + 10)` <a class="yt-timestamp" data-t="00:05:24">[00:05:24]</a>

---

### Example 3: Negative Middle Term, Positive Constant Term

**Problem:** Factor `x² - 11x + 24` <a class="yt-timestamp" data-t="00:06:11">[00:06:11]</a>

**Solution:**
We need two numbers that:
*   Add up to -11 <a class="yt-timestamp" data-t="00:06:21">[00:06:21]</a>
*   Multiply to 24 <a class="yt-timestamp" data-t="00:06:30">[00:06:30]</a>

Since the product is positive (24) and the sum is negative (-11), both numbers must be negative <a class="yt-timestamp" data-t="00:07:03">[00:07:03]</a>.

Consider factors of 24:
*   1 and 24 (sum = 25)
*   2 and 12 (sum = 14) <a class="yt-timestamp" data-t="00:07:54">[00:07:54]</a>
*   3 and 8 (sum = 11) <a class="yt-timestamp" data-t="00:07:44">[00:07:44]</a>

If we use -3 and -8:
*   `-3 * -8 = 24` <a class="yt-timestamp" data-t="00:08:29">[00:08:29]</a>
*   `-3 + -8 = -11` <a class="yt-timestamp" data-t="00:08:37">[00:08:37]</a>. This works!

**Factored form:** `(x - 3)(x - 8)` <a class="yt-timestamp" data-t="00:08:46">[00:08:46]</a>

---

### Example 4: Negative Constant Term

**Problem:** Factor `x² + 5x - 14` <a class="yt-timestamp" data-t="00:09:08">[00:09:08]</a>

**Solution:**
We need two numbers that:
*   Add up to 5 <a class="yt-timestamp" data-t="00:09:33">[00:09:33]</a>
*   Multiply to -14 <a class="yt-timestamp" data-t="00:09:21">[00:09:21]</a>

Since the product is negative (-14), one number must be positive and the other negative <a class="yt-timestamp" data-t="00:09:29">[00:09:29]</a>.

Consider factors of 14:
*   1 and 14
*   2 and 7 <a class="yt-timestamp" data-t="00:10:22">[00:10:22]</a>

Let's test combinations to get a sum of 5:
*   `-1 + 14 = 13` <a class="yt-timestamp" data-t="00:09:53">[00:09:53]</a>
*   `1 + -14 = -13` <a class="yt-timestamp" data-t="00:10:16">[00:10:16]</a>
*   `-2 + 7 = 5` <a class="yt-timestamp" data-t="00:10:29">[00:10:29]</a>. This works! (`-2 * 7 = -14`)

**Factored form:** `(x - 2)(x + 7)` <a class="yt-timestamp" data-t="00:10:47">[00:10:47]</a>

---

### Example 5: Negative Middle Term, Negative Constant Term

**Problem:** Factor `x² - x - 56` <a class="yt-timestamp" data-t="00:11:09">[00:11:09]</a>

**Solution:**
We need two numbers that:
*   Add up to -1 (implied coefficient of -x) <a class="yt-timestamp" data-t="00:11:26">[00:11:26]</a>
*   Multiply to -56 <a class="yt-timestamp" data-t="00:11:16">[00:11:16]</a>

Since the product is negative, one number is positive, and the other is negative <a class="yt-timestamp" data-t="00:11:21">[00:11:21]</a>. Since the sum is negative, the larger absolute value number must be negative <a class="yt-timestamp" data-t="00:11:51">[00:11:51]</a>.

Consider factors of 56:
*   7 and 8 are close to each other <a class="yt-timestamp" data-t="00:11:33">[00:11:33]</a>.

If we use -8 and 7:
*   `-8 * 7 = -56` <a class="yt-timestamp" data-t="00:11:58">[00:11:58]</a>
*   `-8 + 7 = -1` <a class="yt-timestamp" data-t="00:12:03">[00:12:03]</a>. This works!

**Factored form:** `(x - 8)(x + 7)` <a class="yt-timestamp" data-t="00:12:12">[00:12:12]</a>

---

### Example 6: Negative Leading Coefficient

**Problem:** Factor `-x² - 5x + 24` <a class="yt-timestamp" data-t="00:12:50">[00:12:50]</a>

**Solution:**
When the [[understanding_components_of_a_quadratic_equation|coefficient on the x² term]] is negative, it's easiest to factor out a -1 first <a class="yt-timestamp" data-t="00:13:00">[00:13:00]</a>.
`-x² - 5x + 24 = -1(x² + 5x - 24)` <a class="yt-timestamp" data-t="00:13:07">[00:13:07]</a>

Now, factor the expression inside the parentheses: `x² + 5x - 24`.
We need two numbers that:
*   Add up to 5 <a class="yt-timestamp" data-t="00:13:41">[00:13:41]</a>
*   Multiply to -24 <a class="yt-timestamp" data-t="00:13:29">[00:13:29]</a>

Since the product is negative, one number is positive, one is negative <a class="yt-timestamp" data-t="00:13:34">[00:13:34]</a>. Since the sum is positive, the larger absolute value number must be positive.

Consider factors of 24:
*   3 and 8 <a class="yt-timestamp" data-t="00:14:11">[00:14:11]</a>

If we use -3 and 8:
*   `-3 * 8 = -24` <a class="yt-timestamp" data-t="00:14:26">[00:14:26]</a>
*   `-3 + 8 = 5` <a class="yt-timestamp" data-t="00:14:24">[00:14:24]</a>. This works!

**Factored form:** `-1(x - 3)(x + 8)` <a class="yt-timestamp" data-t="00:14:29">[00:14:29]</a>

---

### Example 7: Negative Leading Coefficient and Constant Term

**Problem:** Factor `-x² + 18x - 72` <a class="yt-timestamp" data-t="00:14:56">[00:14:56]</a>

**Solution:**
Factor out a -1:
`-x² + 18x - 72 = -1(x² - 18x + 72)` <a class="yt-timestamp" data-t="00:15:09">[00:15:09]</a>

Now, factor `x² - 18x + 72`.
We need two numbers that:
*   Add up to -18 <a class="yt-timestamp" data-t="00:15:29">[00:15:29]</a>
*   Multiply to 72 <a class="yt-timestamp" data-t="00:15:19">[00:15:19]</a>

Since the product is positive (72) and the sum is negative (-18), both numbers must be negative <a class="yt-timestamp" data-t="00:15:32">[00:15:32]</a>.

Consider factors of 72:
*   8 and 9 (sum of -8 and -9 is -17, close but not -18) <a class="yt-timestamp" data-t="00:15:43">[00:15:43]</a>
*   6 and 12 <a class="yt-timestamp" data-t="00:16:06">[00:16:06]</a>

If we use -6 and -12:
*   `-6 * -12 = 72`
*   `-6 + -12 = -18` <a class="yt-timestamp" data-t="00:16:09">[00:16:09]</a>. This works!

**Factored form:** `-1(x - 6)(x - 12)` <a class="yt-timestamp" data-t="00:16:18">[00:16:18]</a>

---

[[factoring_quadratic_equations|Factoring quadratics]] can feel like an "art" at first, requiring practice to quickly identify the correct factors and signs <a class="yt-timestamp" data-t="00:12:21">[00:12:21]</a>. With more experience, it becomes second nature <a class="yt-timestamp" data-t="00:12:33">[00:12:33]</a>.