---
title: Factoring quadratic expressions
videoId: eF6zYNzlZKQ
---

From: [[khanacademy]] <br/> 

A quadratic expression is a second-degree polynomial, meaning it contains a variable raised to the second power <a class="yt-timestamp" data-t="00:00:00">[00:00:00]</a>. These expressions often appear with 'x' as the variable, such as x² + 10x + 9 <a class="yt-timestamp" data-t="00:00:23">[00:00:23]</a>. [[Factoring in algebra | Factoring]] a quadratic expression means rewriting it as the product of two binomials <a class="yt-timestamp" data-t="00:00:35">[00:00:35]</a>.

## The General Principle of Factoring Quadratics

When a quadratic expression is in standard form (ax² + bx + c), and its leading coefficient (a) is 1, it can often be factored into the form (x + a)(x + b) <a class="yt-timestamp" data-t="00:00:44">[00:00:44]</a>.

To understand why, consider multiplying two binomials:
(x + a)(x + b) = x(x) + x(b) + a(x) + a(b) <a class="yt-timestamp" data-t="00:00:57">[00:00:57]</a>
= x² + bx + ax + ab <a class="yt-timestamp" data-t="00:01:03">[00:01:03]</a>
= x² + (a + b)x + ab <a class="yt-timestamp" data-t="00:01:18">[00:01:18]</a>

From this expansion, we can derive the key rules for [[factoring_quadratics_with_a_leading_coefficient_of_1 | factoring quadratics with a leading coefficient of 1]]:
*   The coefficient of the 'x' term (the first-degree coefficient) is the **sum** of 'a' and 'b' (a + b) <a class="yt-timestamp" data-t="00:01:34">[00:01:34]</a>.
*   The constant term is the **product** of 'a' and 'b' (ab) <a class="yt-timestamp" data-t="00:01:49">[00:01:49]</a>.

Therefore, to factor a quadratic like x² + cx + d, you need to find two numbers (a and b) that:
1.  Add up to the coefficient 'c' (a + b = c) <a class="yt-timestamp" data-t="00:02:05">[00:02:05]</a>
2.  Multiply to the constant term 'd' (a * b = d) <a class="yt-timestamp" data-t="00:02:14">[00:02:14]</a>

When first learning to factor, it's typical to deal with integer numbers for 'a' and 'b' <a class="yt-timestamp" data-t="00:02:27">[00:02:27]</a>.

## Examples of Factoring Quadratics

### Example 1: All Positive Terms

Consider the expression x² + 10x + 9 <a class="yt-timestamp" data-t="00:00:26">[00:00:26]</a>.
We need two numbers that:
*   Add up to 10
*   Multiply to 9

Let's list factors of 9:
*   1 and 9
*   3 and 3

Checking the sums:
*   1 + 9 = 10
*   3 + 3 = 6 (does not work)

Thus, the numbers are 1 and 9 <a class="yt-timestamp" data-t="00:02:57">[00:02:57]</a>.
So, the factored form is (x + 1)(x + 9) <a class="yt-timestamp" data-t="00:03:04">[00:03:04]</a>.

Another example: x² + 15x + 50 <a class="yt-timestamp" data-t="00:04:11">[00:04:11]</a>.
We need two numbers that:
*   Add up to 15
*   Multiply to 50

Let's list factors of 50:
*   1 and 50
*   2 and 25
*   5 and 10

Checking the sums:
*   1 + 50 = 51 (does not work)
*   2 + 25 = 27 (does not work)
*   5 + 10 = 15 (works!)

So, the numbers are 5 and 10 <a class="yt-timestamp" data-t="00:05:19">[00:05:19]</a>.
The factored form is (x + 5)(x + 10) <a class="yt-timestamp" data-t="00:05:24">[00:05:24]</a>.

### Example 2: Negative Middle Term, Positive Constant Term

Consider the expression x² - 11x + 24 <a class="yt-timestamp" data-t="00:06:11">[00:06:11]</a>.
We need two numbers that:
*   Add up to -11
*   Multiply to 24

Since the product (24) is positive, both numbers must have the same sign. Since the sum (-11) is negative, both numbers must be negative <a class="yt-timestamp" data-t="00:06:41">[00:06:41]</a>.

Let's list factors of 24 (and consider their negative counterparts):
*   -1 and -24 (sum = -25)
*   -2 and -12 (sum = -14)
*   -3 and -8 (sum = -11; works!) <a class="yt-timestamp" data-t="00:08:26">[00:08:26]</a>
*   -4 and -6 (sum = -10)

The numbers are -3 and -8 <a class="yt-timestamp" data-t="00:08:43">[00:08:43]</a>.
The factored form is (x - 3)(x - 8) <a class="yt-timestamp" data-t="00:08:53">[00:08:53]</a>.

### Example 3: Negative Constant Term

Consider the expression x² + 5x - 14 <a class="yt-timestamp" data-t="00:09:08">[00:09:08]</a>.
We need two numbers that:
*   Add up to 5
*   Multiply to -14

Since the product (-14) is negative, one number must be positive and the other negative <a class="yt-timestamp" data-t="00:09:21">[00:09:21]</a>.

Let's list factors of 14 and consider their signs:
*   -1 and 14 (sum = 13)
*   1 and -14 (sum = -13)
*   -2 and 7 (sum = 5; works!) <a class="yt-timestamp" data-t="00:10:24">[00:10:24]</a>
*   2 and -7 (sum = -5)

The numbers are -2 and 7 <a class="yt-timestamp" data-t="00:10:41">[00:10:41]</a>.
The factored form is (x - 2)(x + 7) <a class="yt-timestamp" data-t="00:10:47">[00:10:47]</a>.

Another example: x² - x - 56 <a class="yt-timestamp" data-t="00:11:09">[00:11:09]</a>.
We need two numbers that:
*   Add up to -1 (because -x is -1x)
*   Multiply to -56

Since the product (-56) is negative, one number is positive and one is negative. Since the sum (-1) is negative, the larger absolute value number must be negative <a class="yt-timestamp" data-t="00:11:51">[00:11:51]</a>.

Consider factors of 56 that are close together, like 7 and 8 <a class="yt-timestamp" data-t="00:11:33">[00:11:33]</a>:
*   -8 and 7 (sum = -1; works!) <a class="yt-timestamp" data-t="00:11:58">[00:11:58]</a>

The numbers are -8 and 7 <a class="yt-timestamp" data-t="00:12:08">[00:12:08]</a>.
The factored form is (x - 8)(x + 7) <a class="yt-timestamp" data-t="00:12:12">[00:12:12]</a>.

### Example 4: Negative Leading Coefficient

When the x² term has a negative coefficient, the easiest approach is to factor out a -1 from the entire expression first <a class="yt-timestamp" data-t="00:13:00">[00:13:00]</a>.

Consider the expression -x² - 5x + 24 <a class="yt-timestamp" data-t="00:12:42">[00:12:42]</a>.
Factor out -1:
= -1(x² + 5x - 24) <a class="yt-timestamp" data-t="00:13:07">[00:13:07]</a>

Now, factor the trinomial inside the parentheses (x² + 5x - 24):
We need two numbers that:
*   Add up to 5
*   Multiply to -24 (one positive, one negative)

Consider factors of 24:
*   -1 and 24 (sum = 23)
*   -2 and 12 (sum = 10)
*   -3 and 8 (sum = 5; works!) <a class="yt-timestamp" data-t="00:14:11">[00:14:11]</a>
*   -4 and 6 (sum = 2)

The numbers are -3 and 8 <a class="yt-timestamp" data-t="00:14:17">[00:14:17]</a>.
The factored form of the trinomial is (x - 3)(x + 8).
Remember to include the -1 factored out earlier:
= -1(x - 3)(x + 8) <a class="yt-timestamp" data-t="00:14:29">[00:14:29]</a>

Another example: -x² + 18x - 72 <a class="yt-timestamp" data-t="00:14:56">[00:14:56]</a>.
Factor out -1:
= -1(x² - 18x + 72) <a class="yt-timestamp" data-t="00:15:09">[00:15:09]</a>

Now, factor the trinomial inside (x² - 18x + 72):
We need two numbers that:
*   Add up to -18
*   Multiply to 72 (both must be negative)

Consider factors of 72:
*   -8 and -9 (sum = -17; close, but not quite) <a class="yt-timestamp" data-t="00:15:58">[00:15:58]</a>
*   -6 and -12 (sum = -18; works!) <a class="yt-timestamp" data-t="00:16:06">[00:16:06]</a>

The numbers are -6 and -12 <a class="yt-timestamp" data-t="00:16:15">[00:16:15]</a>.
The factored form of the trinomial is (x - 6)(x - 12).
Remember the -1:
= -1(x - 6)(x - 12) <a class="yt-timestamp" data-t="00:16:18">[00:16:18]</a>

Factoring quadratics often requires practice to develop an intuition for finding the correct factors quickly <a class="yt-timestamp" data-t="00:12:21">[00:12:21]</a>.