---
title: Factoring numerators and denominators
videoId: 7Uos1ED3KHI
---

From: [[khanacademy]] <br/> 

When working with fractions, or rational numbers, the concept of putting them in "lowest terms" involves identifying and cancelling out common factors between the numerator and the denominator <a class="yt-timestamp" data-t="00:00:07">[00:00:07]</a>. For example, in the fraction 3/6, both 3 and 6 share a common factor of 3 <a class="yt-timestamp" data-t="00:00:12">[00:00:12]</a>. Since 6 can be written as 2 times 3, the 3s can be cancelled out, resulting in 1/2 <a class="yt-timestamp" data-t="00:00:18">[00:00:18]</a>. Similarly, 8/24 simplifies to 1/3 because 24 is 3 times 8, allowing the 8s to cancel <a class="yt-timestamp" data-t="00:00:48">[00:00:48]</a>.

This same principle applies to rational expressions, which are similar to rational numbers but involve expressions with variables in the numerator and/or denominator <a class="yt-timestamp" data-t="00:01:04">[00:01:04]</a>.

## Simplifying Rational Expressions

To simplify rational expressions, the process involves [[factoring_quadratics | factoring]] both the numerator and the denominator to identify and cancel out any common factors <a class="yt-timestamp" data-t="00:01:37">[00:01:37]</a>.

### Example 1: Factoring out a Constant

Consider the expression: `(9x + 3) / (12x + 4)` <a class="yt-timestamp" data-t="00:01:23">[00:01:23]</a>

1.  **Factor the numerator:** `9x + 3` can be factored by pulling out a 3, resulting in `3(3x + 1)` <a class="yt-timestamp" data-t="00:01:39">[00:01:39]</a>.
2.  **Factor the denominator:** `12x + 4` can be factored by pulling out a 4, resulting in `4(3x + 1)` <a class="yt-timestamp" data-t="00:01:49">[00:01:49]</a>.
3.  **Identify common factors:** Both the numerator and the denominator now have a common factor of `(3x + 1)` <a class="yt-timestamp" data-t="00:02:07">[00:02:07]</a>.
4.  **Cancel common factors:** The `(3x + 1)` terms cancel out <a class="yt-timestamp" data-t="00:02:18">[00:02:18]</a>.

The simplified expression is `3/4` <a class="yt-timestamp" data-t="00:02:23">[00:02:23]</a>.

> [!CAUTION] Excluded Values
> When simplifying rational expressions, it is crucial to state any values of the variable that would make the original denominator zero, as these values would make the expression undefined <a class="yt-timestamp" data-t="00:03:33">[00:03:33]</a>. For the expression `(9x + 3) / (12x + 4)`, if `12x + 4 = 0`, then `x = -1/3` <a class="yt-timestamp" data-t="00:04:47">[00:04:47]</a>. Therefore, the simplified expression `3/4` is equivalent to the original *only if* `x` does not equal `-1/3` <a class="yt-timestamp" data-t="00:05:00">[00:05:00]</a>.

### Example 2: Factoring a Difference of Squares

Consider the expression: `(x^2 - 9) / (5x + 15)` <a class="yt-timestamp" data-t="00:02:40">[00:02:40]</a>

1.  **Factor the numerator:** `x^2 - 9` is a difference of squares, which factors into `(x + 3)(x - 3)` <a class="yt-timestamp" data-t="00:03:00">[00:03:00]</a>.
2.  **Factor the denominator:** `5x + 15` can be factored by pulling out a 5, resulting in `5(x + 3)` <a class="yt-timestamp" data-t="00:03:06">[00:03:06]</a>.
3.  **Identify and cancel common factors:** The common factor is `(x + 3)` <a class="yt-timestamp" data-t="00:03:12">[00:03:12]</a>.

The simplified expression is `(x - 3) / 5`, with the condition that `x` cannot be equal to `-3` (because `-3` would make the original denominator zero) <a class="yt-timestamp" data-t="00:03:39">[00:03:39]</a>.

### Example 3: Factoring Quadratic Trinomials

Consider the expression: `(x^2 + 6x + 5) / (x^2 - x - 2)` <a class="yt-timestamp" data-t="00:05:40">[00:05:40]</a>

1.  **Factor the numerator:** For `x^2 + 6x + 5`, find two numbers that multiply to 5 and add to 6. These are 5 and 1 <a class="yt-timestamp" data-t="00:06:01">[00:06:01]</a>. So, the numerator factors to `(x + 5)(x + 1)` <a class="yt-timestamp" data-t="00:06:09">[00:06:09]</a>.
2.  **Factor the denominator:** For `x^2 - x - 2`, find two numbers that multiply to -2 and add to -1. These are -2 and 1 <a class="yt-timestamp" data-t="00:06:17">[00:06:17]</a>. So, the denominator factors to `(x - 2)(x + 1)` <a class="yt-timestamp" data-t="00:06:38">[00:06:38]</a>.
3.  **Identify and cancel common factors:** The common factor is `(x + 1)` <a class="yt-timestamp" data-t="00:06:46">[00:06:46]</a>.

The simplified expression is `(x + 5) / (x - 2)`, with the condition that `x` cannot be equal to `-1` (because `-1` would make the original denominator zero) <a class="yt-timestamp" data-t="00:06:59">[00:06:59]</a>.

### Example 4: Factoring by Grouping (for Quadratics with leading coefficient â‰  1)

Consider the expression: `(3x^2 + 3x - 18) / (2x^2 + 5x - 3)` <a class="yt-timestamp" data-t="00:07:30">[00:07:30]</a>

#### Factoring the Numerator: `3x^2 + 3x - 18`

To [[factoring_by_grouping | factor by grouping]]:
1.  Find two numbers that multiply to `(3 * -18) = -54` and add to `3` <a class="yt-timestamp" data-t="00:08:09">[00:08:09]</a>. These numbers are 9 and -6 <a class="yt-timestamp" data-t="00:08:41">[00:08:41]</a>.
2.  Rewrite the middle term (`3x`) as `9x - 6x` <a class="yt-timestamp" data-t="00:09:03">[00:09:03]</a>.
    Expression becomes: `3x^2 + 9x - 6x - 18` <a class="yt-timestamp" data-t="00:09:03">[00:09:03]</a>.
3.  Group the terms: `(3x^2 + 9x) + (-6x - 18)` <a class="yt-timestamp" data-t="00:09:31">[00:09:31]</a>.
4.  Factor out common terms from each group:
    *   `3x(x + 3)` from the first group <a class="yt-timestamp" data-t="00:09:53">[00:09:53]</a>.
    *   `-6(x + 3)` from the second group <a class="yt-timestamp" data-t="00:10:02">[00:10:02]</a>.
5.  Factor out the common binomial `(x + 3)`: `(3x - 6)(x + 3)` <a class="yt-timestamp" data-t="00:10:15">[00:10:15]</a>.

#### Factoring the Denominator: `2x^2 + 5x - 3`

To [[factoring_by_grouping | factor by grouping]]:
1.  Find two numbers that multiply to `(2 * -3) = -6` and add to `5` <a class="yt-timestamp" data-t="00:13:00">[00:13:00]</a>. These numbers are 6 and -1 <a class="yt-timestamp" data-t="00:13:12">[00:13:12]</a>.
2.  Rewrite the middle term (`5x`) as `6x - x` <a class="yt-timestamp" data-t="00:13:37">[00:13:37]</a>.
    Expression becomes: `2x^2 + 6x - x - 3` <a class="yt-timestamp" data-t="00:13:37">[00:13:37]</a>.
3.  Group the terms: `(2x^2 + 6x) + (-x - 3)` <a class="yt-timestamp" data-t="00:13:53">[00:13:53]</a>.
4.  Factor out common terms from each group:
    *   `2x(x + 3)` from the first group <a class="yt-timestamp" data-t="00:13:57">[00:13:57]</a>.
    *   `-1(x + 3)` from the second group <a class="yt-timestamp" data-t="00:14:02">[00:14:02]</a>.
5.  Factor out the common binomial `(x + 3)`: `(2x - 1)(x + 3)` <a class="yt-timestamp" data-t="00:14:11">[00:14:11]</a>.

#### Simplifying the Full Expression

The original expression can now be rewritten with its factored numerator and denominator:
`(3x - 6)(x + 3) / (2x - 1)(x + 3)` <a class="yt-timestamp" data-t="00:14:28">[00:14:28]</a>

1.  **Identify and cancel common factors:** The common factor is `(x + 3)` <a class="yt-timestamp" data-t="00:14:40">[00:14:40]</a>.

The simplified expression is `(3x - 6) / (2x - 1)`, with the crucial condition that `x` cannot be equal to `-3` (because `-3` would make the original denominator zero, making the expression undefined) <a class="yt-timestamp" data-t="00:14:47">[00:14:47]</a>.