---
title: Factoring by grouping
videoId: 2ZzuZvz33X0
---

From: [[khanacademy]] <br/> 

[[factoring_polynomials | Factoring polynomials]], especially [[factoring_quadratic_equations | quadratic equations]], is a common method for solving them, particularly when the equation is explicitly set to zero <a class="yt-timestamp" data-t="00:00:17">[00:00:17]</a>. One standard technique for [[factoring_polynomials | factoring]] is called **factoring by grouping** <a class="yt-timestamp" data-t="00:00:33">[00:00:33]</a>.

## When to Use Factoring by Grouping

Factoring by grouping is a versatile method for [[factoring_quadratic_polynomials | factoring quadratic polynomials]] of the form `ax² + bx + c` <a class="yt-timestamp" data-t="00:00:02">[00:00:02]</a>. While a [[shortcut_methods_for_factoring | shortcut method]] exists for quadratics where the leading coefficient `a` is 1 <a class="yt-timestamp" data-t="00:00:38">[00:00:38]</a>, factoring by grouping remains a completely appropriate and general approach <a class="yt-timestamp" data-t="00:13:14">[00:13:14]</a>.

## Steps for Factoring by Grouping

The process of factoring by grouping involves splitting the middle term of the quadratic expression into two terms <a class="yt-timestamp" data-t="00:01:16">[00:01:16]</a>.

Consider the example: `s² - 2s - 35 = 0` <a class="yt-timestamp" data-t="00:00:02">[00:00:02]</a>.

1.  **Identify Coefficients**: For a quadratic `as² + bs + c`, identify `b` and `c`. In this example, `b = -2` and `c = -35` <a class="yt-timestamp" data-t="00:00:02">[00:00:02]</a>.
2.  **Find Two Numbers**: Find two numbers, let's call them `a` and `b` (not to be confused with the coefficients of the quadratic), such that their sum equals the middle coefficient (`a + b = -2`) and their product equals the constant term (`a * b = -35`) <a class="yt-timestamp" data-t="00:00:40">[00:00:40]</a>, <a class="yt-timestamp" data-t="00:00:49">[00:00:49]</a>.
    *   Since the product is a negative number (`-35`), one of the numbers must be positive and the other negative <a class="yt-timestamp" data-t="00:00:59">[00:00:59]</a>.
    *   In this case, the numbers are `5` and `-7` <a class="yt-timestamp" data-t="00:01:08">[00:01:08]</a>.
        *   `5 + (-7) = -2` <a class="yt-timestamp" data-t="00:01:11">[00:01:11]</a>
        *   `5 * (-7) = -35` <a class="yt-timestamp" data-t="00:00:56">[00:00:56]</a>
3.  **Split the Middle Term**: Rewrite the middle term (`-2s`) using the two numbers found (`+5s - 7s`) <a class="yt-timestamp" data-t="00:01:16">[00:01:16]</a>.
    *   `s² + 5s - 7s - 35 = 0` <a class="yt-timestamp" data-t="00:01:23">[00:01:23]</a>
4.  **Group Terms**: Group the first two terms and the last two terms together <a class="yt-timestamp" data-t="00:01:42">[00:01:42]</a>.
    *   `(s² + 5s) + (-7s - 35) = 0` <a class="yt-timestamp" data-t="00:01:42">[00:01:42]</a>
5.  **Factor Out Common Factors**: Factor out the greatest common factor from each group <a class="yt-timestamp" data-t="00:01:49">[00:01:49]</a>.
    *   From `(s² + 5s)`, factor out `s`: `s(s + 5)` <a class="yt-timestamp" data-t="00:01:51">[00:01:51]</a>
    *   From `(-7s - 35)`, factor out `-7`: `-7(s + 5)` <a class="yt-timestamp" data-t="00:02:02">[00:02:02]</a>, <a class="yt-timestamp" data-t="00:02:06">[00:02:06]</a>
    *   The expression becomes: `s(s + 5) - 7(s + 5) = 0` <a class="yt-timestamp" data-t="00:02:12">[00:02:12]</a>
6.  **Factor Out the Common Binomial**: Notice that `(s + 5)` is a common factor in both terms <a class="yt-timestamp" data-t="00:02:15">[00:02:15]</a>. Factor it out.
    *   `(s + 5)(s - 7) = 0` <a class="yt-timestamp" data-t="00:02:26">[00:02:26]</a>

## Solving the Equation Using the Zero Product Property

Once the quadratic equation is factored into the product of two binomials equal to zero, the [[Factoring_quadratic_equations | zero product property]] can be applied <a class="yt-timestamp" data-t="00:02:51">[00:02:51]</a>. This property states that if the product of two numbers (`A` and `B`) is zero (`A * B = 0`), then at least one of the numbers must be zero (`A = 0` or `B = 0` or both) <a class="yt-timestamp" data-t="00:03:02">[00:03:02]</a>.

Applying this to `(s + 5)(s - 7) = 0`:

1.  Set each binomial equal to zero <a class="yt-timestamp" data-t="00:03:22">[00:03:22]</a>.
    *   `s + 5 = 0` <a class="yt-timestamp" data-t="00:03:22">[00:03:22]</a>
    *   `s - 7 = 0` <a class="yt-timestamp" data-t="00:03:30">[00:03:30]</a>
2.  Solve each linear equation for `s` <a class="yt-timestamp" data-t="00:03:48">[00:03:48]</a>.
    *   For `s + 5 = 0`: Subtract `5` from both sides: `s = -5` <a class="yt-timestamp" data-t="00:03:52">[00:03:52]</a>, <a class="yt-timestamp" data-t="00:04:00">[00:04:00]</a>
    *   For `s - 7 = 0`: Add `7` to both sides: `s = 7` <a class="yt-timestamp" data-t="00:04:01">[00:04:01]</a>, <a class="yt-timestamp" data-t="00:04:07">[00:04:07]</a>
3.  The solutions for `s` are `-5` and `7` <a class="yt-timestamp" data-t="00:04:13">[00:04:13]</a>. These can be verified by substituting them back into the original equation <a class="yt-timestamp" data-t="00:04:21">[00:04:21]</a>.

## Comparison to Shortcut Method

While factoring by grouping involves splitting the middle term, a [[shortcut_methods_for_factoring | shortcut method]] exists when the leading coefficient of the quadratic is 1 <a class="yt-timestamp" data-t="00:04:40">[00:04:40]</a>. For an expression like `x² + (a+b)x + ab`, it can be directly factored into `(x + a)(x + b)` <a class="yt-timestamp" data-t="00:05:08">[00:05:08]</a>. Once the two numbers (e.g., `5` and `-7`) that sum to the middle coefficient and multiply to the constant term are found, the expression `s² - 2s - 35` could be directly factored as `(s + 5)(s - 7)` <a class="yt-timestamp" data-t="00:05:54">[00:05:54]</a>, <a class="yt-timestamp" data-t="00:06:00">[00:06:00]</a>. This shortcut skips the intermediate steps of grouping <a class="yt-timestamp" data-t="00:04:47">[00:04:47]</a>.