---
title: Factoring by grouping technique
videoId: 2ZzuZvz33X0
---

From: [[khanacademy]] <br/> 

[[factoring_in_algebra | Factoring in algebra]], particularly the "factoring by grouping" technique, is a method used to solve quadratic equations, especially when they are explicitly set equal to zero <a class="yt-timestamp" data-t="00:00:19">[00:00:19]</a>. This method involves transforming a quadratic expression into a product of two binomials <a class="yt-timestamp" data-t="00:00:23">[00:00:23]</a>.

## How to Factor by Grouping

When a quadratic equation is in the form `ax² + bx + c = 0`, the factoring by grouping method proceeds as follows:

### 1. Identify Product and Sum Relationship
Find two numbers, let's call them 'a' and 'b', such that:
*   Their sum (`a + b`) is equal to the coefficient of the middle term (`b` in `ax² + bx + c`) <a class="yt-timestamp" data-t="00:00:44">[00:00:44]</a><a class="yt-timestamp" data-t="00:00:49">[00:00:49]</a>.
*   Their product (`a * b`) is equal to the constant term (`c` in `ax² + bx + c`) <a class="yt-timestamp" data-t="00:00:52">[00:00:52]</a><a class="yt-timestamp" data-t="00:00:56">[00:00:56]</a>.
    *   If the product is a negative number, one of the two numbers must be positive and the other negative <a class="yt-timestamp" data-t="00:00:59">[00:00:59]</a>.
This relationship is a key aspect of [[product_and_sum_relationships_in_factoring | product and sum relationships in factoring]].

### 2. Split the Middle Term
Once the two numbers are identified, rewrite the middle term (`bx`) of the quadratic expression as the sum of two terms using these numbers. For example, `bx` becomes `ax + bx` (where 'a' and 'b' are the numbers found in step 1) <a class="yt-timestamp" data-t="00:01:16">[00:01:16]</a><a class="yt-timestamp" data-t="00:01:27">[00:01:27]</a>.

### 3. Group and Factor Common Terms
Group the first two terms and the last two terms of the new four-term expression <a class="yt-timestamp" data-t="00:01:42">[00:01:42]</a><a class="yt-timestamp" data-t="00:01:45">[00:01:45]</a>. Factor out the greatest common factor from each pair of grouped terms <a class="yt-timestamp" data-t="00:01:49">[00:01:49]</a>.

### 4. Factor Out the Common Binomial
After factoring, there should be a common binomial factor in both resulting terms. Factor out this common binomial <a class="yt-timestamp" data-t="00:02:15">[00:02:15]</a><a class="yt-timestamp" data-t="00:02:23">[00:02:23]</a><a class="yt-timestamp" data-t="00:02:26">[00:02:26]</a>. The expression will now be in the form of `(binomial 1) * (binomial 2)` <a class="yt-timestamp" data-t="00:02:46">[00:02:46]</a>.

## Example: Solving s² - 2s - 35 = 0

Let's apply the factoring by grouping technique to solve the equation `s² - 2s - 35 = 0` <a class="yt-timestamp" data-t="00:00:02">[00:00:02]</a>.

### Step-by-Step Solution:

1.  **Identify Numbers:** We need two numbers whose sum is -2 and whose product is -35 <a class="yt-timestamp" data-t="00:00:44">[00:00:44]</a><a class="yt-timestamp" data-t="00:00:52">[00:00:52]</a>.
    *   Since the product is negative, one number is positive, and the other is negative <a class="yt-timestamp" data-t="00:00:59">[00:00:59]</a>.
    *   The numbers are 5 and -7 (5 + (-7) = -2; 5 * -7 = -35) <a class="yt-timestamp" data-t="00:01:08">[00:01:08]</a><a class="yt-timestamp" data-t="00:01:11">[00:01:11]</a>.

2.  **Split the Middle Term:** Rewrite `-2s` as `+5s - 7s` <a class="yt-timestamp" data-t="00:01:16">[00:01:16]</a><a class="yt-timestamp" data-t="00:01:27">[00:01:27]</a>.
    *   `s² + 5s - 7s - 35 = 0` <a class="yt-timestamp" data-t="00:01:34">[00:01:34]</a>

3.  **Group and Factor Common Terms:**
    *   Group the first two terms: `(s² + 5s)` <a class="yt-timestamp" data-t="00:01:45">[00:01:45]</a>.
        *   Factor out `s`: `s(s + 5)` <a class="yt-timestamp" data-t="00:01:50">[00:01:50]</a><a class="yt-timestamp" data-t="00:01:51">[00:01:51]</a>.
    *   Group the last two terms: `(-7s - 35)` <a class="yt-timestamp" data-t="00:01:59">[00:01:59]</a>.
        *   Factor out `-7`: `-7(s + 5)` <a class="yt-timestamp" data-t="00:02:02">[00:02:02]</a><a class="yt-timestamp" data-t="00:02:06">[00:02:06]</a>.
    *   The equation becomes: `s(s + 5) - 7(s + 5) = 0` <a class="yt-timestamp" data-t="00:02:12">[00:02:12]</a>.

4.  **Factor Out the Common Binomial:**
    *   Both terms now share the `(s + 5)` factor <a class="yt-timestamp" data-t="00:02:15">[00:02:15]</a>.
    *   Factor it out: `(s + 5)(s - 7) = 0` <a class="yt-timestamp" data-t="00:02:26">[00:02:26]</a>.

## Solving the Factored Equation

Once the quadratic equation is factored into the product of two binomials equal to zero, you can find the solutions for `s`.
If the product of two numbers is zero, then at least one of the numbers must be zero <a class="yt-timestamp" data-t="00:03:00">[00:03:00]</a><a class="yt-timestamp" data-t="00:03:13">[00:03:13]</a>.
Therefore, either:
*   `s + 5 = 0` (which means `s = -5` after subtracting 5 from both sides) <a class="yt-timestamp" data-t="00:03:22">[00:03:22]</a><a class="yt-timestamp" data-t="00:03:52">[00:03:52]</a><a class="yt-timestamp" data-t="00:03:57">[00:03:57]</a>.
*   OR `s - 7 = 0` (which means `s = 7` after adding 7 to both sides) <a class="yt-timestamp" data-t="00:03:30">[00:03:30]</a><a class="yt-timestamp" data-t="00:04:01">[00:04:01]</a><a class="yt-timestamp" data-t="00:04:07">[00:04:07]</a>.

The solutions for `s` are -5 and 7 <a class="yt-timestamp" data-t="00:04:13">[00:04:13]</a>. These solutions can be verified by substituting them back into the original equation <a class="yt-timestamp" data-t="00:04:21">[00:04:21]</a>.

## Comparison to Shortcut Method

While factoring by grouping is a robust method, a [[shortcut_methods_for_factoring_quadratics | shortcut method]] exists when the leading coefficient (the coefficient of the `x²` term) is 1 <a class="yt-timestamp" data-t="00:00:36">[00:00:36]</a><a class="yt-timestamp" data-t="00:00:38">[00:00:38]</a><a class="yt-timestamp" data-t="00:04:40">[00:04:40]</a>.
When expanding binomials like `(x + a)(x + b)`, the result is `x² + (a + b)x + ab` <a class="yt-timestamp" data-t="00:04:50">[00:04:50]</a><a class="yt-timestamp" data-t="00:05:08">[00:05:08]</a>. This reveals a pattern where the constant term is the product of 'a' and 'b', and the coefficient of the middle term is their sum <a class="yt-timestamp" data-t="00:05:17">[00:05:17]</a>.
Therefore, for `s² - 2s - 35 = 0`, once the numbers 5 and -7 are found (whose sum is -2 and product is -35), one can directly write the factored form as `(s + 5)(s - 7) = 0` <a class="yt-timestamp" data-t="00:05:33">[00:05:33]</a><a class="yt-timestamp" data-t="00:05:54">[00:05:54]</a><a class="yt-timestamp" data-t="00:06:00">[00:06:00]</a>. This is a quicker way to factor [[factoring_quadratics_with_a_leading_coefficient_of_1 | quadratics with a leading coefficient of 1]], but factoring by grouping is still a completely appropriate method <a class="yt-timestamp" data-t="00:06:13">[00:06:13]</a>.