---
title: Factoring quadratics with a leading coefficient of 1
videoId: eF6zYNzlZKQ
---

From: [[khanacademy]] <br/> 

A **quadratic expression** is a second-degree polynomial, meaning it has a variable (often 'x') raised to the second power as its highest degree term <a class="yt-timestamp" data-t="00:00:00">[00:00:00]</a>. This article focuses on [[factoring_quadratic_expressions | factoring quadratic expressions]] where the coefficient of the x² term is 1 <a class="yt-timestamp" data-t="00:03:22">[00:03:22]</a>.

## The General Principle of Factoring Quadratics

To factor a quadratic expression like x² + bx + c into the product of two binomials, we utilize the distributive property (often called FOIL) in reverse <a class="yt-timestamp" data-t="00:00:35">[00:00:35]</a>.

Consider the product of two binomials: (x + a)(x + b) <a class="yt-timestamp" data-t="00:00:44">[00:00:44]</a>.
When expanded, this becomes <a class="yt-timestamp" data-t="00:00:57">[00:00:57]</a>:
x * x = x² <a class="yt-timestamp" data-t="00:00:57">[00:00:57]</a>
x * b = bx <a class="yt-timestamp" data-t="00:01:01">[00:01:01]</a>
a * x = ax <a class="yt-timestamp" data-t="00:01:03">[00:01:03]</a>
a * b = ab <a class="yt-timestamp" data-t="00:01:06">[00:01:06]</a>

Combining the 'x' terms, we get:
x² + bx + ax + ab <a class="yt-timestamp" data-t="00:01:12">[00:01:12]</a>
x² + (a + b)x + ab <a class="yt-timestamp" data-t="00:01:22">[00:01:22]</a>

From this general form, we can observe the following relationships <a class="yt-timestamp" data-t="00:01:29">[00:01:29]</a>:
*   The coefficient of the 'x' term (the first-degree coefficient) is the sum of 'a' and 'b' (a + b) <a class="yt-timestamp" data-t="00:01:34">[00:01:34]</a>.
*   The constant term is the product of 'a' and 'b' (ab) <a class="yt-timestamp" data-t="00:01:49">[00:01:49]</a>.

Therefore, to factor a quadratic expression of the form x² + bx + c (where b is the coefficient of x, and c is the constant term), you need to find two numbers, 'a' and 'b', such that <a class="yt-timestamp" data-t="00:02:05">[00:02:05]</a>:
1.  Their sum (a + b) equals the coefficient of the x term (b).
2.  Their product (a * b) equals the constant term (c).

It is important that the quadratic expression is in standard form before applying this method <a class="yt-timestamp" data-t="00:03:41">[00:03:41]</a>.

## Examples of Factoring Quadratics

### Example 1: All Positive Terms
Factor: x² + 10x + 9 <a class="yt-timestamp" data-t="00:00:26">[00:00:26]</a>

We need two numbers that:
*   Add up to 10 (coefficient of x) <a class="yt-timestamp" data-t="00:02:14">[00:02:14]</a>
*   Multiply to 9 (constant term) <a class="yt-timestamp" data-t="00:02:14">[00:02:14]</a>

Considering factors of 9 that are integers <a class="yt-timestamp" data-t="00:02:27">[00:02:27]</a>:
*   1 and 9: 1 * 9 = 9; 1 + 9 = 10. (This works) <a class="yt-timestamp" data-t="00:02:49">[00:02:49]</a>
*   3 and 3: 3 * 3 = 9; 3 + 3 = 6. (Does not work) <a class="yt-timestamp" data-t="00:02:45">[00:02:45]</a>

So, the numbers are 1 and 9.
Factored form: (x + 1)(x + 9) <a class="yt-timestamp" data-t="00:03:04">[00:03:04]</a>

### Example 2: All Positive Terms (continued)
Factor: x² + 15x + 50 <a class="yt-timestamp" data-t="00:04:11">[00:04:11]</a>

We need two numbers that:
*   Add up to 15 <a class="yt-timestamp" data-t="00:04:35">[00:04:35]</a>
*   Multiply to 50 <a class="yt-timestamp" data-t="00:04:35">[00:04:35]</a>

Consider factors of 50 <a class="yt-timestamp" data-t="00:04:47">[00:04:47]</a>:
*   1 and 50: 1 + 50 = 51 (No) <a class="yt-timestamp" data-t="00:05:07">[00:05:07]</a>
*   2 and 25: 2 + 25 = 27 (No) <a class="yt-timestamp" data-t="00:05:12">[00:05:12]</a>
*   5 and 10: 5 + 10 = 15 (Yes!) <a class="yt-timestamp" data-t="00:05:16">[00:05:16]</a>

So, the numbers are 5 and 10.
Factored form: (x + 5)(x + 10) <a class="yt-timestamp" data-t="00:05:24">[00:05:24]</a>

### Example 3: Negative Middle Term, Positive Constant Term
Factor: x² - 11x + 24 <a class="yt-timestamp" data-t="00:06:11">[00:06:11]</a>

We need two numbers that:
*   Add up to -11 <a class="yt-timestamp" data-t="00:06:26">[00:06:26]</a>
*   Multiply to 24 <a class="yt-timestamp" data-t="00:06:30">[00:06:30]</a>

Since the product is positive (24) and the sum is negative (-11), both numbers must be negative <a class="yt-timestamp" data-t="00:07:03">[00:07:03]</a>.
Consider factors of 24 (and make them negative) <a class="yt-timestamp" data-t="00:07:28">[00:07:28]</a>:
*   -1 and -24: -1 + (-24) = -25 (No)
*   -2 and -12: -2 + (-12) = -14 (No)
*   -3 and -8: -3 + (-8) = -11 (Yes!) <a class="yt-timestamp" data-t="00:08:37">[00:08:37]</a>
*   -4 and -6: -4 + (-6) = -10 (No)

So, the numbers are -3 and -8.
Factored form: (x - 3)(x - 8) <a class="yt-timestamp" data-t="00:08:53">[00:08:53]</a>

### Example 4: Positive Middle Term, Negative Constant Term
Factor: x² + 5x - 14 <a class="yt-timestamp" data-t="00:09:08">[00:09:08]</a>

We need two numbers that:
*   Add up to 5 <a class="yt-timestamp" data-t="00:09:39">[00:09:39]</a>
*   Multiply to -14 <a class="yt-timestamp" data-t="00:09:26">[00:09:26]</a>

Since the product is negative (-14), one number must be positive and the other must be negative <a class="yt-timestamp" data-t="00:09:29">[00:09:29]</a>.
Consider factors of 14, where one is negative <a class="yt-timestamp" data-t="00:09:41">[00:09:41]</a>:
*   -1 and 14: -1 + 14 = 13 (No) <a class="yt-timestamp" data-t="00:10:01">[00:10:01]</a>
*   1 and -14: 1 + (-14) = -13 (No) <a class="yt-timestamp" data-t="00:10:16">[00:10:16]</a>
*   -2 and 7: -2 + 7 = 5 (Yes!) <a class="yt-timestamp" data-t="00:10:29">[00:10:29]</a>
*   2 and -7: 2 + (-7) = -5 (No) <a class="yt-timestamp" data-t="00:10:36">[00:10:36]</a>

So, the numbers are -2 and 7.
Factored form: (x - 2)(x + 7) <a class="yt-timestamp" data-t="00:10:47">[00:10:47]</a>

### Example 5: Negative Middle and Constant Terms
Factor: x² - x - 56 <a class="yt-timestamp" data-t="00:11:09">[00:11:09]</a>

We need two numbers that:
*   Add up to -1 (coefficient of x) <a class="yt-timestamp" data-t="00:11:26">[00:11:26]</a>
*   Multiply to -56 (constant term) <a class="yt-timestamp" data-t="00:11:16">[00:11:16]</a>

Since the product is negative, one number is positive and one is negative <a class="yt-timestamp" data-t="00:11:24">[00:11:24]</a>. Since the sum is negative, the number with the larger absolute value must be negative <a class="yt-timestamp" data-t="00:11:51">[00:11:51]</a>.
Consider factors of 56:
*   Knowing 8 * 7 = 56 <a class="yt-timestamp" data-t="00:11:33">[00:11:33]</a>.
*   To get a sum of -1, we try -8 and 7.
*   -8 * 7 = -56 (Yes) <a class="yt-timestamp" data-t="00:11:58">[00:11:58]</a>
*   -8 + 7 = -1 (Yes!) <a class="yt-timestamp" data-t="00:12:03">[00:12:03]</a>

So, the numbers are -8 and 7.
Factored form: (x - 8)(x + 7) <a class="yt-timestamp" data-t="00:12:12">[00:12:12]</a>

### Example 6: Factoring out a Negative Leading Coefficient
Factor: -x² - 5x + 24 <a class="yt-timestamp" data-t="00:12:50">[00:12:50]</a>

When the leading coefficient is negative, it's often easiest to factor out -1 first <a class="yt-timestamp" data-t="00:13:00">[00:13:00]</a>.
-x² - 5x + 24 = -1(x² + 5x - 24) <a class="yt-timestamp" data-t="00:13:07">[00:13:07]</a>

Now, we need to factor the quadratic inside the parenthesis: x² + 5x - 24.
We need two numbers that:
*   Add up to 5 <a class="yt-timestamp" data-t="00:13:41">[00:13:41]</a>
*   Multiply to -24 <a class="yt-timestamp" data-t="00:13:29">[00:13:29]</a>

Since the product is negative, one number is positive and one is negative <a class="yt-timestamp" data-t="00:13:34">[00:13:34]</a>.
Consider factors of 24:
*   3 and 8: If 3 is negative (-3) and 8 is positive, then -3 + 8 = 5 (Yes!) <a class="yt-timestamp" data-t="00:14:13">[00:14:13]</a>
*   -3 * 8 = -24 (Yes!) <a class="yt-timestamp" data-t="00:14:26">[00:14:26]</a>

So, the numbers are -3 and 8.
Factored form: -1(x - 3)(x + 8) <a class="yt-timestamp" data-t="00:14:31">[00:14:31]</a>

### Example 7: Factoring out a Negative Leading Coefficient (continued)
Factor: -x² + 18x - 72 <a class="yt-timestamp" data-t="00:14:56">[00:14:56]</a>

First, factor out -1:
-x² + 18x - 72 = -1(x² - 18x + 72) <a class="yt-timestamp" data-t="00:15:09">[00:15:09]</a>

Now, factor x² - 18x + 72:
We need two numbers that:
*   Add up to -18 <a class="yt-timestamp" data-t="00:15:29">[00:15:29]</a>
*   Multiply to 72 <a class="yt-timestamp" data-t="00:15:19">[00:15:19]</a>

Since the product is positive (72) and the sum is negative (-18), both numbers must be negative <a class="yt-timestamp" data-t="00:15:32">[00:15:32]</a>.
Consider negative factors of 72:
*   -8 and -9: -8 + (-9) = -17 (Close, but no) <a class="yt-timestamp" data-t="00:15:53">[00:15:53]</a>
*   -6 and -12: -6 + (-12) = -18 (Yes!) <a class="yt-timestamp" data-t="00:16:06">[00:16:06]</a>
*   -6 * -12 = 72 (Yes!)

So, the numbers are -6 and -12.
Factored form: -1(x - 6)(x - 12) <a class="yt-timestamp" data-t="00:16:18">[00:16:18]</a>

This method, while sometimes feeling like an "art," becomes second nature with practice <a class="yt-timestamp" data-t="00:12:21">[00:12:21]</a>.