---
title: Introduction to the quadratic formula
videoId: i7idZfS8t8w
---

From: [[khanacademy]] <br/> 

The quadratic formula is considered one of the top five most useful formulas in mathematics <a class="yt-timestamp" data-t="00:00:04">[00:00:04]</a>. While memorization is recommended, it is also important to understand its derivation to know where it came from <a class="yt-timestamp" data-t="00:00:17">[00:00:17]</a>.

The primary purpose of the quadratic formula is to [[solving_quadratic_equations_using_the_quadratic_formula | solve for the roots, or zeroes, of quadratic equations]] <a class="yt-timestamp" data-t="00:00:32">[00:00:32]</a>. It is particularly useful for problems that are difficult to factor <a class="yt-timestamp" data-t="00:05:45">[00:05:45]</a>.

## General Form of a Quadratic Equation

A quadratic equation is typically expressed in the form:
`ax² + bx + c = 0` <a class="yt-timestamp" data-t="00:00:44">[00:00:44]</a>.

In this general form:
*   `a` is the coefficient of the x² term (the second-degree term) <a class="yt-timestamp" data-t="00:00:59">[00:00:59]</a>.
*   `b` is the coefficient of the x term <a class="yt-timestamp" data-t="00:01:02">[00:01:02]</a>.
*   `c` is the constant term (or the coefficient on the x to the zero term) <a class="yt-timestamp" data-t="00:01:05">[00:01:05]</a>.

## The Formula

Given a general quadratic equation `ax² + bx + c = 0`, the quadratic formula states that the solutions for `x` are:

```
x = (-b ± √(b² - 4ac)) / 2a
```
<a class="yt-timestamp" data-t="00:01:13">[00:01:13]</a>

Although it may appear complex initially, the formula becomes more manageable with practice <a class="yt-timestamp" data-t="00:01:34">[00:01:34]</a>.

### Derivation

The quadratic formula is derived by [[completing_the_square_and_derivation_of_the_quadratic_formula | completing the square]] on the general quadratic equation `ax² + bx + c = 0` <a class="yt-timestamp" data-t="00:01:54">[00:01:54]</a>.

## [[examples_and_applications_of_the_quadratic_formula | Examples of Application]]

### Example 1: Factorable Quadratic

Let's solve `x² + 4x - 21 = 0` using the quadratic formula <a class="yt-timestamp" data-t="00:02:14">[00:02:14]</a>.

1.  **Identify coefficients**:
    *   `a = 1` <a class="yt-timestamp" data-t="00:02:30">[00:02:30]</a>
    *   `b = 4` <a class="yt-timestamp" data-t="00:02:37">[00:02:37]</a>
    *   `c = -21` <a class="yt-timestamp" data-t="00:02:40">[00:02:40]</a>

2.  **Plug into the formula**:
    `x = (-4 ± √(4² - 4*1*-21)) / (2*1)` <a class="yt-timestamp" data-t="00:02:49">[00:02:49]</a>
    `x = (-4 ± √(16 - (-84))) / 2` <a class="yt-timestamp" data-t="00:03:08">[00:03:08]</a>
    `x = (-4 ± √(16 + 84)) / 2` <a class="yt-timestamp" data-t="00:03:55">[00:03:55]</a>
    `x = (-4 ± √100) / 2` <a class="yt-timestamp" data-t="00:04:03">[00:04:03]</a>
    `x = (-4 ± 10) / 2` <a class="yt-timestamp" data-t="00:04:09">[00:04:09]</a>

3.  **Calculate the two solutions**:
    *   `x₁ = (-4 + 10) / 2 = 6 / 2 = 3` <a class="yt-timestamp" data-t="00:04:32">[00:04:32]</a>
    *   `x₂ = (-4 - 10) / 2 = -14 / 2 = -7` <a class="yt-timestamp" data-t="00:04:38">[00:04:38]</a>

These solutions (3 and -7) match the results obtained by factoring the equation `(x+7)(x-3) = 0` <a class="yt-timestamp" data-t="00:05:04">[00:05:04]</a>.

### Example 2: Quadratic with No Real Solutions

Consider the equation `3x² + 6x = -10` <a class="yt-timestamp" data-t="00:06:17">[00:06:17]</a>.

1.  **Rewrite in standard form**: Add 10 to both sides to get `3x² + 6x + 10 = 0` <a class="yt-timestamp" data-t="00:06:31">[00:06:31]</a>.

2.  **Identify coefficients**:
    *   `a = 3` <a class="yt-timestamp" data-t="00:06:51">[00:06:51]</a>
    *   `b = 6` <a class="yt-timestamp" data-t="00:06:53">[00:06:53]</a>
    *   `c = 10` <a class="yt-timestamp" data-t="00:06:53">[00:06:53]</a>

3.  **Plug into the formula**:
    `x = (-6 ± √(6² - 4*3*10)) / (2*3)` <a class="yt-timestamp" data-t="00:07:10">[00:07:10]</a>
    `x = (-6 ± √(36 - 120)) / 6` <a class="yt-timestamp" data-t="00:07:42">[00:07:42]</a>
    `x = (-6 ± √-84) / 6` <a class="yt-timestamp" data-t="00:08:46">[00:08:46]</a>

When the term under the square root (`b² - 4ac`), known as the discriminant, is negative, there are no real solutions <a class="yt-timestamp" data-t="00:09:06">[00:09:06]</a>. This means the parabola represented by the quadratic function does not intersect the x-axis <a class="yt-timestamp" data-t="00:10:27">[00:10:27]</a>. Solutions involving the square root of a negative number require the use of [[understanding_the_domain_of_a_quadratic_function | imaginary numbers]] <a class="yt-timestamp" data-t="00:09:17">[00:09:17]</a>.

### Example 3: Non-Factorable Quadratic with Real Solutions

Let's solve `negative 3x² + 12x + 1 = 0` <a class="yt-timestamp" data-t="00:10:52">[00:10:52]</a>.

1.  **Identify coefficients**:
    *   `a = -3` <a class="yt-timestamp" data-t="00:10:52">[00:10:52]</a>
    *   `b = 12` <a class="yt-timestamp" data-t="00:11:13">[00:11:13]</a>
    *   `c = 1` <a class="yt-timestamp" data-t="00:11:27">[00:11:27]</a>

2.  **Plug into the formula**:
    `x = (-12 ± √(12² - 4*-3*1)) / (2*-3)` <a class="yt-timestamp" data-t="00:11:13">[00:11:13]</a>
    `x = (-12 ± √(144 - (-12))) / -6` <a class="yt-timestamp" data-t="00:11:27">[00:11:27]</a>
    `x = (-12 ± √(144 + 12)) / -6` <a class="yt-timestamp" data-t="00:11:49">[00:11:49]</a>
    `x = (-12 ± √156) / -6` <a class="yt-timestamp" data-t="00:12:01">[00:12:01]</a>

3.  **Simplify the radical**:
    The prime factorization of 156 is `2 × 2 × 3 × 13`, so `√156 = √(4 × 39) = 2√39` <a class="yt-timestamp" data-t="00:12:17">[00:12:17]</a>.

4.  **Substitute back and simplify**:
    `x = (-12 ± 2√39) / -6` <a class="yt-timestamp" data-t="00:13:10">[00:13:10]</a>
    Divide numerator and denominator by 2:
    `x = (-6 ± √39) / -3` <a class="yt-timestamp" data-t="00:13:26">[00:13:26]</a>
    Separate the terms and simplify further:
    `x = (-6 / -3) ± (√39 / -3)` <a class="yt-timestamp" data-t="00:13:38">[00:13:38]</a>
    `x = 2 ± (-√39 / 3)` <a class="yt-timestamp" data-t="00:13:51">[00:13:51]</a>

The solutions are `x = 2 + (√39 / 3)` and `x = 2 - (√39 / 3)` <a class="yt-timestamp" data-t="00:15:07">[00:15:07]</a>. The `±` sign handles the positive/negative of the radical being divided by a negative number <a class="yt-timestamp" data-t="00:14:16">[00:14:16]</a>.