---
title: Mathematical expressions
videoId: 3NHSwiv_pSE
---

From: [[khanacademy]] <br/> 

[[simplifying_expressions | Simplifying expressions]] involves applying known mathematical ideas to rewrite them in a simpler form <a class="yt-timestamp" data-t="00:00:09">[00:00:09]</a>. This process often utilizes fundamental [[arithmetic_operations | arithmetic operations]] and properties.

## The Distributive Property

The distributive property is a key concept when [[simplifying_expressions | simplifying expressions]] <a class="yt-timestamp" data-t="00:00:53">[00:00:53]</a>. It states that multiplying a sum or difference by a number is the same as multiplying each term in the sum or difference by that number and then adding or subtracting the products <a class="yt-timestamp" data-t="00:01:09">[00:01:09]</a>.

### Example 1: Simplifying 2(3x + 5)

To [[simplifying_expressions | simplify]] the expression 2(3x + 5), one can interpret it literally as two sets of "(3x + 5)" <a class="yt-timestamp" data-t="00:00:21">[00:00:21]</a>:
*   (3x + 5) + (3x + 5) <a class="yt-timestamp" data-t="00:00:25">[00:00:25]</a>
*   This means there are two "3x" terms and two "5" terms <a class="yt-timestamp" data-t="00:00:37">[00:00:37]</a>.
*   So, 2(3x + 5) can be rewritten as 2(3x) + 2(5) <a class="yt-timestamp" data-t="00:00:40">[00:00:40]</a>.
*   Applying the multiplication: 2 * 3x = 6x <a class="yt-timestamp" data-t="00:01:15">[00:01:15]</a>.
*   And 2 * 5 = 10 <a class="yt-timestamp" data-t="00:01:21">[00:01:21]</a>.
*   Therefore, 2(3x + 5) simplifies to 6x + 10 <a class="yt-timestamp" data-t="00:01:24">[00:01:24]</a>.

### Example 2: Simplifying 7(3y - 5) - 2(10 + 4y)

More complex expressions also use the same principles <a class="yt-timestamp" data-t="00:01:30">[00:01:30]</a>. To [[simplifying_expressions | simplify]] 7(3y - 5) - 2(10 + 4y):

1.  **Distribute the 7 to the first part:**
    *   7 * 3y = 21y <a class="yt-timestamp" data-t="00:02:03">[00:02:03]</a>
    *   7 * (-5) = -35 <a class="yt-timestamp" data-t="00:02:16">[00:02:16]</a>
    *   So, 7(3y - 5) becomes 21y - 35 <a class="yt-timestamp" data-t="00:02:22">[00:02:22]</a>.

2.  **Distribute the -2 to the second part (being careful with the sign):**
    *   Think of it as distributing "-2" instead of "2" and then subtracting <a class="yt-timestamp" data-t="00:02:35">[00:02:35]</a>.
    *   -2 * 10 = -20 <a class="yt-timestamp" data-t="00:02:46">[00:02:46]</a>
    *   -2 * 4y = -8y <a class="yt-timestamp" data-t="00:02:56">[00:02:56]</a>
    *   So, -2(10 + 4y) becomes -20 - 8y <a class="yt-timestamp" data-t="00:03:03">[00:03:03]</a>.

3.  **Combine the simplified parts:**
    *   The expression is now 21y - 35 - 20 - 8y <a class="yt-timestamp" data-t="00:03:06">[00:03:06]</a>.

4.  **Combine like terms:**
    *   Terms with 'y': 21y - 8y = 13y <a class="yt-timestamp" data-t="00:03:17">[00:03:17]</a>.
    *   Constant terms: -35 - 20 = -55 <a class="yt-timestamp" data-t="00:03:42">[00:03:42]</a>.

5.  **Final simplified expression:** 13y - 55 <a class="yt-timestamp" data-t="00:03:56">[00:03:56]</a>.

This process demonstrates common [[strategies_for_dealing_with_complex_arithmetic_expressions | strategies for dealing with complex arithmetic expressions]] and helps in [[understanding_algebraic_expressions | understanding algebraic expressions]].