---
title: Product and sum relationships in factoring
videoId: eF6zYNzlZKQ
---

From: [[khanacademy]] <br/> 

[[Factoring quadratic expressions | Factoring a second-degree polynomial]], often called a quadratic expression, involves rewriting it as the product of two binomials <a class="yt-timestamp" data-t="00:00:06">[00:00:06]</a>. This method is particularly useful when the leading coefficient (the coefficient of the x² term) is 1 <a class="yt-timestamp" data-t="00:03:22">[00:03:22]</a>.

## The Core Relationship

To understand [[factoring in algebra | factoring]] a quadratic expression of the form x² + Bx + C, consider the [[stepbystep_process_of_expanding_binomials | expansion of two binomials]] in the form (x + a)(x + b) <a class="yt-timestamp" data-t="00:00:41">[00:00:41]</a>:

(x + a)(x + b) = x(x) + x(b) + a(x) + a(b) <a class="yt-timestamp" data-t="00:00:57">[00:00:57]</a>
= x² + bx + ax + ab <a class="yt-timestamp" data-t="00:01:03">[00:01:03]</a>
= x² + (a + b)x + ab <a class="yt-timestamp" data-t="00:01:22">[00:01:22]</a>

By comparing this expanded form with the standard quadratic x² + Bx + C, we can derive a key relationship:
*   The coefficient of the x term (B) is the sum of `a` and `b` (a + b) <a class="yt-timestamp" data-t="00:01:40">[00:01:40]</a>.
*   The constant term (C) is the product of `a` and `b` (ab) <a class="yt-timestamp" data-t="00:01:49">[00:01:49]</a>.

Therefore, when [[solving_quadratic_equations_by_factoring | factoring]] a quadratic expression of the form x² + Bx + C, the goal is to find two numbers, `a` and `b`, such that their sum equals B and their product equals C <a class="yt-timestamp" data-t="00:02:05">[00:02:05]</a>. It is assumed that these numbers are integers, especially when beginning to learn factoring <a class="yt-timestamp" data-t="00:02:27">[00:02:27]</a>.

## Examples

### Positive Sum and Positive Product

**Example 1: Factor x² + 10x + 9** <a class="yt-timestamp" data-t="00:00:26">[00:00:26]</a>

1.  Identify the sum (B) and product (C): We need two numbers that add up to 10 (a + b = 10) and multiply to 9 (ab = 9) <a class="yt-timestamp" data-t="00:02:05">[00:02:05]</a>.
2.  List factors of C: The factors of 9 are (1, 9) and (3, 3) <a class="yt-timestamp" data-t="00:02:37">[00:02:37]</a>.
3.  Test sums:
    *   3 + 3 = 6 (Does not equal 10) <a class="yt-timestamp" data-t="00:02:45">[00:02:45]</a>
    *   1 + 9 = 10 (Equals 10) <a class="yt-timestamp" data-t="00:02:53">[00:02:53]</a>
4.  The numbers are 1 and 9 <a class="yt-timestamp" data-t="00:02:57">[00:02:57]</a>.
5.  Factored form: (x + 1)(x + 9) <a class="yt-timestamp" data-t="00:03:04">[00:03:04]</a>

**Example 2: Factor x² + 15x + 50** <a class="yt-timestamp" data-t="00:04:11">[00:04:11]</a>

1.  Identify the sum (B) and product (C): a + b = 15, ab = 50 <a class="yt-timestamp" data-t="00:04:25">[00:04:25]</a>.
2.  List factors of C: Factors of 50 are (1, 50), (2, 25), (5, 10) <a class="yt-timestamp" data-t="00:04:47">[00:04:47]</a>.
3.  Test sums:
    *   1 + 50 = 51 (Does not equal 15) <a class="yt-timestamp" data-t="00:05:07">[00:05:07]</a>
    *   2 + 25 = 27 (Does not equal 15) <a class="yt-timestamp" data-t="00:05:12">[00:05:12]</a>
    *   5 + 10 = 15 (Equals 15) <a class="yt-timestamp" data-t="00:05:16">[00:05:16]</a>
4.  The numbers are 5 and 10 <a class="yt-timestamp" data-t="00:05:19">[00:05:19]</a>.
5.  Factored form: (x + 5)(x + 10) <a class="yt-timestamp" data-t="00:05:24">[00:05:24]</a>

### Negative Sum and Positive Product

**Example 3: Factor x² - 11x + 24** <a class="yt-timestamp" data-t="00:06:11">[00:06:11]</a>

1.  Identify the sum (B) and product (C): a + b = -11, ab = 24 <a class="yt-timestamp" data-t="00:06:21">[00:06:21]</a>.
2.  Analyze signs: Since the product is positive (24), both `a` and `b` must have the same sign. Since the sum is negative (-11), both `a` and `b` must be negative <a class="yt-timestamp" data-t="00:06:41">[00:06:41]</a>.
3.  List factors of 24 (considering negatives): (-1, -24), (-2, -12), (-3, -8), (-4, -6) <a class="yt-timestamp" data-t="00:07:28">[00:07:28]</a>.
4.  Test sums:
    *   (-1) + (-24) = -25
    *   (-2) + (-12) = -14
    *   (-3) + (-8) = -11 (Equals -11) <a class="yt-timestamp" data-t="00:08:29">[00:08:29]</a>
5.  The numbers are -3 and -8 <a class="yt-timestamp" data-t="00:08:43">[00:08:43]</a>.
6.  Factored form: (x - 3)(x - 8) <a class="yt-timestamp" data-t="00:08:46">[00:08:46]</a>

### Positive Sum and Negative Product

**Example 4: Factor x² + 5x - 14** <a class="yt-timestamp" data-t="00:09:08">[00:09:08]</a>

1.  Identify the sum (B) and product (C): a + b = 5, ab = -14 <a class="yt-timestamp" data-t="00:09:19">[00:09:19]</a>.
2.  Analyze signs: Since the product is negative (-14), one number must be positive and the other negative <a class="yt-timestamp" data-t="00:09:29">[00:09:29]</a>.
3.  List factors of 14 (considering opposite signs): (1, -14), (-1, 14), (2, -7), (-2, 7) <a class="yt-timestamp" data-t="00:09:49">[00:09:49]</a>.
4.  Test sums:
    *   1 + (-14) = -13
    *   (-1) + 14 = 13
    *   2 + (-7) = -5
    *   (-2) + 7 = 5 (Equals 5) <a class="yt-timestamp" data-t="00:10:29">[00:10:29]</a>
5.  The numbers are -2 and 7 <a class="yt-timestamp" data-t="00:10:41">[00:10:41]</a>.
6.  Factored form: (x - 2)(x + 7) <a class="yt-timestamp" data-t="00:10:47">[00:10:47]</a>

### Negative Sum and Negative Product

**Example 5: Factor x² - x - 56** <a class="yt-timestamp" data-t="00:11:09">[00:11:09]</a>

1.  Identify the sum (B) and product (C): a + b = -1, ab = -56 <a class="yt-timestamp" data-t="00:11:16">[00:11:16]</a>.
2.  Analyze signs: Product is negative, so one positive and one negative. Sum is negative, so the larger absolute value factor must be negative <a class="yt-timestamp" data-t="00:11:51">[00:11:51]</a>.
3.  List factors of 56 (considering opposite signs, larger negative): (1, -56), (2, -28), (4, -14), (7, -8) <a class="yt-timestamp" data-t="00:11:33">[00:11:33]</a>. The pair (7, -8) is often recognized due to their proximity to each other <a class="yt-timestamp" data-t="00:11:44">[00:11:44]</a>.
4.  Test sums:
    *   7 + (-8) = -1 (Equals -1) <a class="yt-timestamp" data-t="00:12:03">[00:12:03]</a>
5.  The numbers are 7 and -8 <a class="yt-timestamp" data-t="00:12:08">[00:12:08]</a>.
6.  Factored form: (x - 8)(x + 7) <a class="yt-timestamp" data-t="00:12:12">[00:12:12]</a>

### Leading Negative Coefficient

When the x² term has a negative coefficient, the easiest approach is to factor out a -1 first <a class="yt-timestamp" data-t="00:13:00">[00:13:00]</a>.

**Example 6: Factor -x² - 5x + 24** <a class="yt-timestamp" data-t="00:12:50">[00:12:50]</a>

1.  Factor out -1: -1(x² + 5x - 24) <a class="yt-timestamp" data-t="00:13:07">[00:13:07]</a>.
2.  Now factor the inner quadratic (x² + 5x - 24): We need a + b = 5 and ab = -24 <a class="yt-timestamp" data-t="00:13:29">[00:13:29]</a>.
    *   Analyze signs: Product is negative, so one positive and one negative. Sum is positive, so the larger absolute value factor must be positive.
    *   Factors of 24 (considering opposite signs, larger positive): (-1, 24), (-2, 12), (-3, 8), (-4, 6).
    *   Test sums:
        *   (-3) + 8 = 5 (Equals 5) <a class="yt-timestamp" data-t="00:14:13">[00:14:13]</a>
3.  The numbers are -3 and 8 <a class="yt-timestamp" data-t="00:14:17">[00:14:17]</a>.
4.  Factored form: -1(x - 3)(x + 8) <a class="yt-timestamp" data-t="00:14:29">[00:14:29]</a>

**Example 7: Factor -x² + 18x - 72** <a class="yt-timestamp" data-t="00:14:56">[00:14:56]</a>

1.  Factor out -1: -1(x² - 18x + 72) <a class="yt-timestamp" data-t="00:15:06">[00:15:06]</a>.
2.  Now factor the inner quadratic (x² - 18x + 72): We need a + b = -18 and ab = 72 <a class="yt-timestamp" data-t="00:15:16">[00:15:16]</a>.
    *   Analyze signs: Product is positive, so both have the same sign. Sum is negative, so both must be negative <a class="yt-timestamp" data-t="00:15:32">[00:15:32]</a>.
    *   Factors of 72 (considering negatives): (-1, -72), (-2, -36), (-3, -24), (-4, -18), (-6, -12), (-8, -9).
    *   Test sums:
        *   (-9) + (-8) = -17 (Close, but not -18) <a class="yt-timestamp" data-t="00:15:58">[00:15:58]</a>
        *   (-6) + (-12) = -18 (Equals -18) <a class="yt-timestamp" data-t="00:16:09">[00:16:09]</a>
3.  The numbers are -6 and -12 <a class="yt-timestamp" data-t="00:16:15">[00:16:15]</a>.
4.  Factored form: -1(x - 6)(x - 12) <a class="yt-timestamp" data-t="00:16:18">[00:16:18]</a>

## Practice and Tips

Factoring quadratics using the product and sum relationship is an important skill in [[factoring in algebra | algebra]] <a class="yt-timestamp" data-t="00:12:21">[00:12:21]</a>. It can feel like an "art" initially, requiring you to consider various factors and their positive/negative signs <a class="yt-timestamp" data-t="00:12:23">[00:12:23]</a>. However, with consistent practice, this process will become second nature <a class="yt-timestamp" data-t="00:12:33">[00:12:33]</a>.

### Tips for success:
*   Always ensure the quadratic is in standard form (Ax² + Bx + C) before attempting to factor <a class="yt-timestamp" data-t="00:03:41">[00:03:41]</a>.
*   If the leading coefficient is negative, factor out -1 first <a class="yt-timestamp" data-t="00:13:00">[00:13:00]</a>.
*   Start by listing all integer factors of the constant term (C) <a class="yt-timestamp" data-t="00:02:23">[00:02:23]</a>.
*   Pay close attention to the signs of B and C:
    *   If C is positive, both factors have the same sign as B.
    *   If C is negative, the factors have opposite signs. The factor with the larger absolute value will have the same sign as B.
*   Test the sums of the factor pairs until you find the one that matches B <a class="yt-timestamp" data-t="00:02:40">[00:02:40]</a>.