---
title: Properties of zeros in equations
videoId: 2ZzuZvz33X0
---

From: [[khanacademy]] <br/> 

When solving a quadratic equation, such as `s² - 2s - 35 = 0` <a class="yt-timestamp" data-t="00:00:02">[00:00:02]</a>, particularly when it is explicitly set to zero, factoring the expression is the most effective approach <a class="yt-timestamp" data-t="00:00:17">[00:00:17]</a>. The principle behind this method relies on the unique [[effects_of_multiplying_by_zero_and_one | properties of zero in multiplication]] <a class="yt-timestamp" data-t="00:02:51">[00:02:51]</a>.

## Factoring Quadratic Equations

To factor a quadratic equation like `s² - 2s - 35 = 0`, one common method is factoring by grouping <a class="yt-timestamp" data-t="00:00:40">[00:00:40]</a>. This involves finding two numbers whose sum equals the coefficient of the middle term (in this case, -2) and whose product equals the constant term (here, -35) <a class="yt-timestamp" data-t="00:00:40">[00:00:40]</a>.

For the equation `s² - 2s - 35 = 0`:
*   We look for two numbers `a` and `b` such that `a + b = -2` <a class="yt-timestamp" data-t="00:00:49">[00:00:49]</a> and `a × b = -35` <a class="yt-timestamp" data-t="00:00:52">[00:00:52]</a>.
*   Since the product is a negative number, one factor must be positive and the other negative <a class="yt-timestamp" data-t="00:00:59">[00:00:59]</a>.
*   The numbers that fit these conditions are 5 and -7 <a class="yt-timestamp" data-t="00:01:08">[00:01:08]</a>, because `5 + (-7) = -2` <a class="yt-timestamp" data-t="00:01:11">[00:01:11]</a> and `5 × (-7) = -35` <a class="yt-timestamp" data-t="00:00:56">[00:00:56]</a>.

### Factoring by Grouping Steps

1.  Split the middle term (`-2s`) using the identified numbers: `s² + 5s - 7s - 35 = 0` <a class="yt-timestamp" data-t="00:01:16">[00:01:16]</a>.
2.  Group the terms: `(s² + 5s) + (-7s - 35) = 0` <a class="yt-timestamp" data-t="00:01:42">[00:01:42]</a>.
3.  Factor out common terms from each group:
    *   `s(s + 5)` <a class="yt-timestamp" data-t="00:01:49">[00:01:49]</a>
    *   `-7(s + 5)` <a class="yt-timestamp" data-t="00:02:02">[00:02:02]</a>
4.  Combine the factored terms: `s(s + 5) - 7(s + 5) = 0` <a class="yt-timestamp" data-t="00:02:06">[00:02:06]</a>.
5.  Factor out the common binomial `(s + 5)`: `(s + 5)(s - 7) = 0` <a class="yt-timestamp" data-t="00:02:26">[00:02:26]</a>.

## The Zero Product Property

Once the equation is factored into the form `(s + 5)(s - 7) = 0`, we apply the [[effects_of_multiplying_by_zero_and_one | Zero Product Property]] <a class="yt-timestamp" data-t="00:02:51">[00:02:51]</a>. This property states that if the product of two or more numbers is zero, then at least one of those numbers must be zero <a class="yt-timestamp" data-t="00:03:13">[00:03:13]</a>.

In our case, `(s + 5)` is one number and `(s - 7)` is another <a class="yt-timestamp" data-t="00:02:56">[00:02:56]</a>. Since their product is zero, either `(s + 5) = 0` or `(s - 7) = 0` (or both) <a class="yt-timestamp" data-t="00:03:22">[00:03:22]</a>.

## Solving for the Variable

This leads to two separate [[understanding_linear_equations | linear equations]]:

1.  **s + 5 = 0**
    *   Subtract 5 from both sides: `s = -5` <a class="yt-timestamp" data-t="00:03:52">[00:03:52]</a>.
2.  **s - 7 = 0**
    *   Add 7 to both sides: `s = 7` <a class="yt-timestamp" data-t="00:04:07">[00:04:07]</a>.

Thus, the solutions for `s` are -5 or 7 <a class="yt-timestamp" data-t="00:04:13">[00:04:13]</a>. These solutions can be verified by substituting them back into the original equation <a class="yt-timestamp" data-t="00:04:21">[00:04:21]</a>.

## Shortcut Method

When the leading coefficient of a quadratic equation is 1 (e.g., `s²` instead of `2s²`), a shortcut to factoring exists <a class="yt-timestamp" data-t="00:04:40">[00:04:40]</a>. If we have `x² + (a + b)x + ab`, it can be directly factored into `(x + a)(x + b)` <a class="yt-timestamp" data-t="00:05:08">[00:05:08]</a>.
Since we found that 5 and -7 satisfy the sum and product conditions for `s² - 2s - 35 = 0`, we could have directly factored it as `(s + 5)(s - 7) = 0` <a class="yt-timestamp" data-t="00:06:00">[00:06:00]</a>, bypassing the intermediate grouping steps <a class="yt-timestamp" data-t="00:06:07">[00:06:07]</a>. However, factoring by grouping remains a valid and appropriate method <a class="yt-timestamp" data-t="00:06:14">[00:06:14]</a>.