---
title: Quadratic equations transformation
videoId: bNQY0z76M5A
---

From: [[khanacademy]] <br/> 

## Completing the Square

**Completing the Square** is a technique used to transform and solve [[solving_quadratic_equations | quadratic equations]] <a class="yt-timestamp" data-t="00:00:02">[00:00:02]</a>. This method is universally applicable to any [[quadratic_polynomials | quadratic equation]] <a class="yt-timestamp" data-t="00:00:14">[00:00:14]</a> and serves as the fundamental basis for the [[introduction_to_the_quadratic_formula | quadratic formula]] <a class="yt-timestamp" data-t="00:00:14">[00:00:14]</a>. The [[introduction_to_the_quadratic_formula | quadratic formula]] itself can be derived using the completing the square method <a class="yt-timestamp" data-t="00:00:21">[00:00:21]</a>.

The core idea behind completing the square is to manipulate a [[quadratic_polynomials | quadratic equation]] so that one side becomes a perfect square binomial, resembling the form (x + a)² or (x - a)² <a class="yt-timestamp" data-t="00:00:56">[00:00:56]</a>. This transformation is achieved by strategically adding and subtracting values from both sides of the equation <a class="yt-timestamp" data-t="00:01:01">[00:01:01]</a>.

### Why Use Completing the Square?

While other [[solving_techniques_for_quadratic_equations | solving techniques for quadratic equations]], such as [[factoring_quadratic_equations | factoring]], can be faster in certain cases <a class="yt-timestamp" data-t="00:05:10">[00:05:10]</a>, completing the square offers a significant advantage: it **always works** <a class="yt-timestamp" data-t="00:05:16">[00:05:16]</a>. This method is particularly useful for [[quadratic_polynomials | quadratic equations]] that are difficult or impossible to [[factoring_quadratic_equations | factor]] using traditional methods, especially when coefficients are fractions or lead to irrational solutions <a class="yt-timestamp" data-t="00:07:14">[00:07:14]</a>, <a class="yt-timestamp" data-t="00:07:26">[00:07:26]</a>, <a class="yt-timestamp" data-t="00:11:07">[00:11:07]</a>.

### Steps to Complete the Square

Let's illustrate the process with an example: `x² - 4x = 5` <a class="yt-timestamp" data-t="00:00:36">[00:00:36]</a>.

1.  **Isolate the x² and x terms**: Ensure the constant term is on the opposite side of the equation from the x² and x terms. In the given example, this is already done <a class="yt-timestamp" data-t="00:07:50">[00:07:50]</a>.
2.  **Ensure a leading coefficient of 1**: If the x² term has a coefficient other than 1, divide the entire equation by that coefficient <a class="yt-timestamp" data-t="00:06:23">[00:06:23]</a>, <a class="yt-timestamp" data-t="00:06:41">[00:06:41]</a>.
    *   *Example:* For `10x² - 30x - 8 = 0` <a class="yt-timestamp" data-t="00:05:37">[00:05:37]</a>, first divide by 2 to get `5x² - 15x - 4 = 0` <a class="yt-timestamp" data-t="00:06:02">[00:06:02]</a>. Then, divide by 5 to get `x² - 3x - 4/5 = 0` <a class="yt-timestamp" data-t="00:06:43">[00:06:43]</a>. You can then move the constant to the right: `x² - 3x = 4/5` <a class="yt-timestamp" data-t="00:08:13">[00:08:13]</a>.
3.  **Find the term to complete the square**:
    *   Take the coefficient of the x term (let's call it `b`). For `x² - 4x = 5`, `b = -4` <a class="yt-timestamp" data-t="00:02:25">[00:02:25]</a>.
    *   Divide this coefficient by 2: `b/2` <a class="yt-timestamp" data-t="00:02:29">[00:02:29]</a>. For our example, `-4 / 2 = -2` <a class="yt-timestamp" data-t="00:02:32">[00:02:32]</a>.
    *   Square the result: `(b/2)²` <a class="yt-timestamp" data-t="00:02:40">[00:02:40]</a>. For our example, `(-2)² = 4` <a class="yt-timestamp" data-t="00:02:41">[00:02:41]</a>.
4.  **Add this term to both sides**: Add the calculated `(b/2)²` value to both sides of the equation to maintain balance <a class="yt-timestamp" data-t="00:02:44">[00:02:44]</a>, <a class="yt-timestamp" data-t="00:03:12">[00:03:12]</a>.
    *   `x² - 4x + 4 = 5 + 4` <a class="yt-timestamp" data-t="00:02:46">[00:02:46]</a>, <a class="yt-timestamp" data-t="00:03:07">[00:03:07]</a>.
    *   This simplifies to `x² - 4x + 4 = 9` <a class="yt-timestamp" data-t="00:03:27">[00:03:27]</a>.
5.  **Factor the perfect square**: The left-hand side can now be factored into a perfect square binomial. The term in the parentheses will always be `(x + b/2)` or `(x - b/2)` <a class="yt-timestamp" data-t="00:03:39">[00:03:39]</a>.
    *   `x² - 4x + 4` becomes `(x - 2)²` <a class="yt-timestamp" data-t="00:03:59">[00:03:59]</a>.
    *   So, the equation is now `(x - 2)² = 9` <a class="yt-timestamp" data-t="00:03:59">[00:03:59]</a>.
6.  **Solve by taking the square root**: Take the square root of both sides of the equation. Remember to include both the positive and negative roots <a class="yt-timestamp" data-t="00:04:02">[00:04:02]</a>.
    *   `√(x - 2)² = ±√9` <a class="yt-timestamp" data-t="00:04:02">[00:04:02]</a>.
    *   `x - 2 = ±3` <a class="yt-timestamp" data-t="00:04:07">[00:04:07]</a>.
7.  **Isolate x**: Solve for `x` by adding or subtracting the constant term <a class="yt-timestamp" data-t="00:04:10">[00:04:10]</a>.
    *   `x = 2 ± 3` <a class="yt-timestamp" data-t="00:04:10">[00:04:10]</a>.
    *   This yields two solutions:
        *   `x = 2 + 3 = 5` <a class="yt-timestamp" data-t="00:04:16">[00:04:16]</a>
        *   `x = 2 - 3 = -1` <a class="yt-timestamp" data-t="00:04:22">[00:04:22]</a>

<br/>
---

> [!info] Understanding Components of a Quadratic Equation
> When transforming a [[quadratic_polynomials | quadratic equation]] `ax² + bx + c = 0` using completing the square, the key is to recognize the pattern of a perfect square trinomial `(x + k)² = x² + 2kx + k²`. By matching the `x` term's coefficient, `b`, with `2k`, we find `k = b/2`. Then, the constant term needed to complete the square is `k² = (b/2)²`.