---
title: Simplifying expressions
videoId: 3NHSwiv_pSE
---

From: [[khanacademy]] <br/> 

Simplifying expressions involves applying fundamental algebraic properties to rewrite an expression in a more concise or manageable form <a class="yt-timestamp" data-t="00:00:09">[00:00:09]</a>. This process often utilizes the [[understanding_equivalent_expressions_in_algebra | distributive property]] and combining like terms <a class="yt-timestamp" data-t="00:03:57">[00:03:57]</a>.

## Using the Distributive Property

The [[understanding_equivalent_expressions_in_algebra | distributive property]] states that `a(b + c) = ab + ac` <a class="yt-timestamp" data-t="00:00:53">[00:00:53]</a>. This property is key for [[expression_simplification_techniques | simplifying expressions]] where a number or variable is multiplied by a sum or difference inside parentheses.

### Example 1: Basic Distribution

To simplify `2(3x + 5)` <a class="yt-timestamp" data-t="00:00:15">[00:00:15]</a>:
*   The expression `2(3x + 5)` literally means two instances of `(3x + 5)` <a class="yt-timestamp" data-t="00:00:21">[00:00:21]</a>.
*   This can be written as `(3x + 5) + (3x + 5)` <a class="yt-timestamp" data-t="00:00:25">[00:00:25]</a>.
*   Applying the [[understanding_equivalent_expressions_in_algebra | distributive property]], multiply `2` by each term inside the parentheses:
    *   `2 * 3x = 6x` <a class="yt-timestamp" data-t="00:01:15">[00:01:15]</a>
    *   `2 * 5 = 10` <a class="yt-timestamp" data-t="00:01:21">[00:01:21]</a>
*   The simplified expression is `6x + 10` <a class="yt-timestamp" data-t="00:01:24">[00:01:24]</a>.

## Combining Like Terms

After distributing, the next step in [[expression_simplification_techniques | simplifying expressions]] often involves combining "like terms." Like terms are terms that have the same variables raised to the same powers.

### Example 2: More Involved Simplification

Consider the expression `7(3y - 5) - 2(10 + 4y)` <a class="yt-timestamp" data-t="00:01:34">[00:01:34]</a>.

1.  **Distribute on the left side** (`7(3y - 5)`) <a class="yt-timestamp" data-t="00:01:59">[00:01:59]</a>:
    *   `7 * 3y = 21y` <a class="yt-timestamp" data-t="00:02:03">[00:02:03]</a>
    *   `7 * -5 = -35` <a class="yt-timestamp" data-t="00:02:16">[00:02:16]</a>
    *   This part becomes `21y - 35` <a class="yt-timestamp" data-t="00:02:22">[00:02:22]</a>.

2.  **Distribute on the right side** (`-2(10 + 4y)`) <a class="yt-timestamp" data-t="00:02:24">[00:02:24]</a>:
    *   It's crucial to distribute the `-2` (including the negative sign) <a class="yt-timestamp" data-t="00:02:35">[00:02:35]</a>.
    *   `-2 * 10 = -20` <a class="yt-timestamp" data-t="00:02:39">[00:02:39]</a>
    *   `-2 * 4y = -8y` <a class="yt-timestamp" data-t="00:02:56">[00:02:56]</a>
    *   This part becomes `-20 - 8y` <a class="yt-timestamp" data-t="00:03:00">[00:03:00]</a>.

3.  **Combine the results**:
    *   The expression is now `21y - 35 - 20 - 8y` <a class="yt-timestamp" data-t="00:03:03">[00:03:03]</a>.

4.  **Combine like terms** <a class="yt-timestamp" data-t="00:03:10">[00:03:10]</a>:
    *   **Y-terms**: `21y - 8y = 13y` <a class="yt-timestamp" data-t="00:03:33">[00:03:33]</a>
    *   **Constant terms**: `-35 - 20 = -55` <a class="yt-timestamp" data-t="00:03:51">[00:03:51]</a>

5.  **Final simplified expression**: `13y - 55` <a class="yt-timestamp" data-t="00:03:56">[00:03:56]</a>.