---
title: Simplifying fractions
videoId: 7Uos1ED3KHI
---

From: [[khanacademy]] <br/> 

[[Methods for simplifying fractions | Simplifying fractions]], whether rational numbers or algebraic expressions, involves reducing them to their lowest terms by identifying and canceling out common factors from the numerator and denominator <a class="yt-timestamp" data-t="00:01:04">[00:01:04]</a>.

## Basic Principles of Simplifying Fractions

When learning about fractions (rational numbers), the concept of "lowest terms" is introduced <a class="yt-timestamp" data-t="00:00:07">[00:00:07]</a>. This means expressing a fraction where the numerator and denominator share no common factors other than 1.

For example:
*   To simplify 3/6:
    *   Identify that 3 and 6 share a common factor of 3 <a class="yt-timestamp" data-t="00:00:12">[00:00:12]</a>.
    *   Rewrite the denominator: 6 = 2 × 3 <a class="yt-timestamp" data-t="00:00:18">[00:00:18]</a>.
    *   Divide both the numerator and denominator by 3, or conceptualize it as cancelling out 3/3 <a class="yt-timestamp" data-t="00:00:26">[00:00:26]</a>.
    *   The fraction in lowest terms becomes 1/2 <a class="yt-timestamp" data-t="00:00:35">[00:00:35]</a>.
*   To simplify 8/24:
    *   Recognize that 24 can be written as 3 × 8 <a class="yt-timestamp" data-t="00:00:48">[00:00:48]</a>.
    *   Cancel out the common factor of 8 (as 8/8) <a class="yt-timestamp" data-t="00:00:56">[00:00:56]</a>.
    *   The simplified fraction is 1/3 <a class="yt-timestamp" data-t="00:00:58">[00:00:58]</a>.

## Simplifying Rational Expressions

The same principles apply to rational expressions, which are essentially fractions where the numerator and/or denominator are algebraic expressions involving variables instead of just numbers <a class="yt-timestamp" data-t="00:01:10">[00:01:10]</a>.

The key steps are:
1.  Factorize both the numerator and the denominator.
2.  Identify any common factors.
3.  Cancel out the common factors.
4.  **Crucially**, identify and exclude any values of the variable that would have made the *original* denominator equal to zero, as these values would make the original expression undefined <a class="yt-timestamp" data-t="00:03:21">[00:03:21]</a>.

### Example 1: Simplifying (9x + 3) / (12x + 4)

1.  **Factor the numerator:** 9x + 3 = 3(3x + 1) <a class="yt-timestamp" data-t="00:01:37">[00:01:37]</a>
2.  **Factor the denominator:** 12x + 4 = 4(3x + 1) <a class="yt-timestamp" data-t="00:01:49">[00:01:49]</a>
3.  **Identify common factor:** (3x + 1) <a class="yt-timestamp" data-t="00:02:09">[00:02:09]</a>
4.  **Cancel common factor:**
    (3(3x + 1)) / (4(3x + 1)) = 3/4 <a class="yt-timestamp" data-t="00:02:20">[00:02:20]</a>
5.  **Identify excluded values:** The original denominator (12x + 4) would be zero if 3x + 1 = 0, which means x = -1/3 <a class="yt-timestamp" data-t="00:04:51">[00:04:51]</a>.
    Therefore, the simplified expression is 3/4, where x ≠ -1/3 <a class="yt-timestamp" data-t="00:05:00">[00:05:00]</a>.

### Example 2: Simplifying (x² - 9) / (5x + 15)

1.  **Factor the numerator:** This is a difference of squares: x² - 9 = (x + 3)(x - 3) <a class="yt-timestamp" data-t="00:03:00">[00:03:00]</a>
2.  **Factor the denominator:** 5x + 15 = 5(x + 3) <a class="yt-timestamp" data-t="00:03:06">[00:03:06]</a>
3.  **Identify common factor:** (x + 3) <a class="yt-timestamp" data-t="00:03:12">[00:03:12]</a>
4.  **Cancel common factor:**
    ((x + 3)(x - 3)) / (5(x + 3)) = (x - 3) / 5 <a class="yt-timestamp" data-t="00:03:24">[00:03:24]</a>
5.  **Identify excluded values:** The original denominator (5x + 15) would be zero if x + 3 = 0, which means x = -3 <a class="yt-timestamp" data-t="00:03:47">[00:03:47]</a>.
    Therefore, the simplified expression is (x - 3) / 5, where x ≠ -3 <a class="yt-timestamp" data-t="00:03:42">[00:03:42]</a>.

### Example 3: Simplifying (x² + 6x + 5) / (x² - x - 2)

1.  **Factor the numerator:** Find two numbers that multiply to 5 and add to 6 (5 and 1).
    x² + 6x + 5 = (x + 5)(x + 1) <a class="yt-timestamp" data-t="00:06:01">[00:06:01]</a>
2.  **Factor the denominator:** Find two numbers that multiply to -2 and add to -1 (-2 and 1).
    x² - x - 2 = (x - 2)(x + 1) <a class="yt-timestamp" data-t="00:06:14">[00:06:14]</a>
3.  **Identify common factor:** (x + 1) <a class="yt-timestamp" data-t="00:06:46">[00:06:46]</a>
4.  **Cancel common factor:**
    ((x + 5)(x + 1)) / ((x - 2)(x + 1)) = (x + 5) / (x - 2) <a class="yt-timestamp" data-t="00:06:51">[00:06:51]</a>
5.  **Identify excluded values:** The original denominator (x² - x - 2) would be zero if x + 1 = 0, which means x = -1 <a class="yt-timestamp" data-t="00:07:00">[00:07:00]</a>.
    Therefore, the simplified expression is (x + 5) / (x - 2), where x ≠ -1 <a class="yt-timestamp" data-t="00:07:20">[00:07:20]</a>.

### Example 4: Simplifying (3x² + 3x - 18) / (2x² + 5x - 3)

This example requires factoring quadratic expressions with a leading coefficient other than 1, often done by grouping.

#### Factoring the Numerator: 3x² + 3x - 18

1.  **Find two numbers:** Multiply to 3 * (-18) = -54, and add to 3. These numbers are 9 and -6 <a class="yt-timestamp" data-t="00:08:09">[00:08:09]</a>.
2.  **Rewrite the middle term:** 3x² + 9x - 6x - 18 <a class="yt-timestamp" data-t="00:09:03">[00:09:03]</a>
3.  **Group and factor:**
    *   (3x² + 9x) + (-6x - 18) <a class="yt-timestamp" data-t="00:09:35">[00:09:35]</a>
    *   3x(x + 3) - 6(x + 3) <a class="yt-timestamp" data-t="00:09:56">[00:09:56]</a>
    *   (3x - 6)(x + 3) <a class="yt-timestamp" data-t="00:10:15">[00:10:15]</a>
    *   The numerator is (3x - 6)(x + 3) <a class="yt-timestamp" data-t="00:10:45">[00:10:45]</a>.

#### Factoring the Denominator: 2x² + 5x - 3

1.  **Find two numbers:** Multiply to 2 * (-3) = -6, and add to 5. These numbers are 6 and -1 <a class="yt-timestamp" data-t="00:13:00">[00:13:00]</a>.
2.  **Rewrite the middle term:** 2x² + 6x - x - 3 <a class="yt-timestamp" data-t="00:13:34">[00:13:34]</a>
3.  **Group and factor:**
    *   (2x² + 6x) + (-x - 3) <a class="yt-timestamp" data-t="00:13:53">[00:13:53]</a>
    *   2x(x + 3) - 1(x + 3) <a class="yt-timestamp" data-t="00:13:57">[00:13:57]</a>
    *   (2x - 1)(x + 3) <a class="yt-timestamp" data-t="00:14:11">[00:14:11]</a>
    *   The denominator is (2x - 1)(x + 3) <a class="yt-timestamp" data-t="00:14:28">[00:14:28]</a>.

#### Final Simplification

1.  **Set up the factored expression:**
    ((3x - 6)(x + 3)) / ((2x - 1)(x + 3)) <a class="yt-timestamp" data-t="00:14:37">[00:14:37]</a>
2.  **Identify common factor:** (x + 3) <a class="yt-timestamp" data-t="00:14:40">[00:14:40]</a>
3.  **Cancel common factor:** (3x - 6) / (2x - 1) <a class="yt-timestamp" data-t="00:15:09">[00:15:09]</a>
4.  **Identify excluded values:** The original denominator would be zero if x + 3 = 0, which means x = -3 <a class="yt-timestamp" data-t="00:14:47">[00:14:47]</a>.
    Therefore, the simplified expression is (3x - 6) / (2x - 1), where x ≠ -3 <a class="yt-timestamp" data-t="00:15:14">[00:15:14]</a>.