---
title: Solving quadratic equations using the quadratic formula
videoId: i7idZfS8t8w
---

From: [[khanacademy]] <br/> 

The quadratic formula is considered one of the most useful formulas in mathematics <a class="yt-timestamp" data-t="00:00:00">[00:00:00]</a>. While memorization is generally not recommended, this formula is an exception, with the caveat that one should also understand its proof <a class="yt-timestamp" data-t="00:00:11">[00:00:11]</a>. Its primary purpose is to [[solving_algebraic_equations | solve for the roots]] or zeroes of [[introduction_to_the_quadratic_formula | quadratic equations]] <a class="yt-timestamp" data-t="00:00:32">[00:00:32]</a>.

## The Quadratic Formula

A general [[introduction_to_the_quadratic_formula | quadratic equation]] is expressed in the form:
`ax^2 + bx + c = 0` <a class="yt-timestamp" data-t="00:00:44">[00:00:44]</a>.

In this standard form:
*   `a` is the coefficient of the `x^2` (second-degree) term <a class="yt-timestamp" data-t="00:01:00">[00:01:00]</a>.
*   `b` is the coefficient of the `x` term <a class="yt-timestamp" data-t="00:01:02">[00:01:02]</a>.
*   `c` is the constant term (or coefficient of `x^0`) <a class="yt-timestamp" data-t="00:01:05">[00:01:05]</a>.

The quadratic formula provides the solutions for `x`:

> [!Formula] The Quadratic Formula
> `x = (-b ± √(b^2 - 4ac)) / 2a` <a class="yt-timestamp" data-t="00:01:13">[00:01:13]</a>

This formula can seem complex, but with practice, it becomes more manageable <a class="yt-timestamp" data-t="00:01:34">[00:01:34]</a>. It is derived by [[completing_the_square_and_derivation_of_the_quadratic_formula | completing the square]] on the general quadratic equation `ax^2 + bx + c = 0` <a class="yt-timestamp" data-t="00:01:49">[00:01:49]</a>. For more on its derivation, refer to [[relation_between_completing_the_square_and_the_quadratic_formula | Completing the Square and Derivation of the Quadratic Formula]].

## Applying the Quadratic Formula

The quadratic formula is useful for [[examples_and_applications_of_the_quadratic_formula | solving quadratic equations]], especially those that are difficult or impossible to factor <a class="yt-timestamp" data-t="00:05:42">[00:05:42]</a>.

### Example 1: Factorable Equation

Let's solve `x^2 + 4x - 21 = 0` <a class="yt-timestamp" data-t="00:02:14">[00:02:14]</a>.
1.  **Identify a, b, c**:
    *   `a = 1` (coefficient of `x^2`) <a class="yt-timestamp" data-t="00:02:30">[00:02:30]</a>
    *   `b = 4` (coefficient of `x`) <a class="yt-timestamp" data-t="00:02:37">[00:02:37]</a>
    *   `c = -21` (constant term) <a class="yt-timestamp" data-t="00:02:40">[00:02:40]</a>

2.  **Plug into the formula**:
    `x = (-4 ± √(4^2 - 4 * 1 * -21)) / (2 * 1)` <a class="yt-timestamp" data-t="00:02:49">[00:02:49]</a>

3.  **Simplify**:
    `x = (-4 ± √(16 - (-84))) / 2` <a class="yt-timestamp" data-t="00:03:08">[00:03:08]</a>
    `x = (-4 ± √(16 + 84)) / 2` <a class="yt-timestamp" data-t="00:03:50">[00:03:50]</a>
    `x = (-4 ± √100) / 2` <a class="yt-timestamp" data-t="00:04:03">[00:04:03]</a>
    `x = (-4 ± 10) / 2` <a class="yt-timestamp" data-t="00:04:09">[00:04:09]</a>
    `x = -2 ± 5` <a class="yt-timestamp" data-t="00:04:23">[00:04:23]</a>

4.  **Find the two solutions**:
    *   `x_1 = -2 + 5 = 3` <a class="yt-timestamp" data-t="00:04:32">[00:04:32]</a>
    *   `x_2 = -2 - 5 = -7` <a class="yt-timestamp" data-t="00:04:38">[00:04:38]</a>

This result matches the solutions obtained by [[solving_quadratic_equations_by_factoring | factoring]] the equation `(x + 7)(x - 3) = 0`, which yields `x = -7` or `x = 3` <a class="yt-timestamp" data-t="00:05:04">[00:05:04]</a>.

### Example 2: No Real Solutions

Let's solve `3x^2 + 6x = -10` <a class="yt-timestamp" data-t="00:06:17">[00:06:17]</a>.
1.  **Rearrange to standard form (equal to 0)**:
    Add 10 to both sides: `3x^2 + 6x + 10 = 0` <a class="yt-timestamp" data-t="00:06:31">[00:06:31]</a>.

2.  **Identify a, b, c**:
    *   `a = 3` <a class="yt-timestamp" data-t="00:06:51">[00:06:51]</a>
    *   `b = 6` <a class="yt-timestamp" data-t="00:06:53">[00:06:53]</a>
    *   `c = 10` <a class="yt-timestamp" data-t="00:06:56">[00:06:56]</a>

3.  **Plug into the formula**:
    `x = (-6 ± √(6^2 - 4 * 3 * 10)) / (2 * 3)` <a class="yt-timestamp" data-t="00:07:10">[00:07:10]</a>

4.  **Simplify**:
    `x = (-6 ± √(36 - 120)) / 6` <a class="yt-timestamp" data-t="00:07:42">[00:07:42]</a>
    `x = (-6 ± √(-84)) / 6` <a class="yt-timestamp" data-t="00:08:18">[00:08:18]</a>

> [!Note] No Real Solutions
> When the term under the square root (`b^2 - 4ac`, known as the discriminant) is negative, there are no real solutions to the equation <a class="yt-timestamp" data-t="00:09:06">[00:09:06]</a>. This means the graph of the quadratic equation will not intersect the x-axis <a class="yt-timestamp" data-t="00:10:27">[00:10:27]</a>. Solutions for such cases involve [[imaginary numbers]], which are typically introduced in more advanced topics <a class="yt-timestamp" data-t="00:09:17">[00:09:17]</a>.

### Example 3: Non-Obvious Solution

Let's solve `-3x^2 + 12x + 1 = 0` <a class="yt-timestamp" data-t="00:10:52">[00:10:52]</a>.
1.  **Identify a, b, c**:
    *   `a = -3` <a class="yt-timestamp" data-t="00:11:07">[00:11:07]</a>
    *   `b = 12` <a class="yt-timestamp" data-t="00:11:13">[00:11:13]</a>
    *   `c = 1` <a class="yt-timestamp" data-t="00:11:29">[00:11:29]</a>

2.  **Plug into the formula**:
    `x = (-12 ± √(12^2 - 4 * -3 * 1)) / (2 * -3)` <a class="yt-timestamp" data-t="00:11:07">[00:11:07]</a>

3.  **Simplify**:
    `x = (-12 ± √(144 - (-12))) / -6` <a class="yt-timestamp" data-t="00:11:39">[00:11:39]</a>
    `x = (-12 ± √(144 + 12)) / -6` <a class="yt-timestamp" data-t="00:11:49">[00:11:49]</a>
    `x = (-12 ± √156) / -6` <a class="yt-timestamp" data-t="00:11:51">[00:11:51]</a>

4.  **Simplify the radical (√156)**:
    Prime factorization of 156: `156 = 2 * 78 = 2 * 2 * 39` <a class="yt-timestamp" data-t="00:12:17">[00:12:17]</a>.
    So, `√156 = √(2^2 * 39) = 2√39` <a class="yt-timestamp" data-t="00:12:48">[00:12:48]</a>.

5.  **Substitute back and simplify the expression**:
    `x = (-12 ± 2√39) / -6` <a class="yt-timestamp" data-t="00:13:10">[00:13:10]</a>
    Divide numerator and denominator by 2:
    `x = (-6 ± √39) / -3` <a class="yt-timestamp" data-t="00:13:23">[00:13:23]</a>

6.  **Separate terms for final solutions**:
    `x = -6 / -3 ± √39 / -3` <a class="yt-timestamp" data-t="00:13:38">[00:13:38]</a>
    `x = 2 ± (-√39 / 3)` <a class="yt-timestamp" data-t="00:13:49">[00:13:49]</a>

The "plus or minus" sign already accounts for the sign change when dividing by a negative number. So, the solutions can be written as:
`x = 2 ± (√39 / 3)` <a class="yt-timestamp" data-t="00:15:01">[00:15:01]</a>.

These solutions are:
*   `x_1 = 2 + (√39 / 3)`
*   `x_2 = 2 - (√39 / 3)`