---
title: Understanding equivalent expressions
videoId: f15zA0PhSek
---

From: [[khanacademy]] <br/> 

Solving equations involves finding the value of an unknown variable, often denoted as 'x'. The primary goal is to [[equivalent_transformations_in_algebra | isolate the variable]] on one side of the equation, resulting in a form like "x equals something" <a class="yt-timestamp" data-t="00:00:33">[00:00:33]</a>. This is achieved by performing a series of [[equivalent_transformations_in_algebra | operations]] on both sides of the equation <a class="yt-timestamp" data-t="00:00:46">[00:00:46]</a>.

Visualizing these operations can make the process intuitive, clarifying which steps are permissible and why <a class="yt-timestamp" data-t="00:00:58">[00:00:58]</a>. As long as [[equivalent_transformations_in_algebra | legitimate operations]] are performed, the correct answer will eventually be obtained <a class="yt-timestamp" data-t="00:02:26">[00:02:26]</a>.

## Solving an Involved Equation Example

Let's consider the equation `2x + 3 = 5x - 2` <a class="yt-timestamp" data-t="00:00:03">[00:00:03]</a> <a class="yt-timestamp" data-t="00:00:15">[00:00:15]</a>.

### Step 1: Consolidate Variables

The first step is to bring all the 'x' terms to one side of the equation <a class="yt-timestamp" data-t="00:02:04">[00:02:04]</a>. A reasonable approach is to subtract `2x` from both sides to keep a positive number of 'x's on the right-hand side <a class="yt-timestamp" data-t="00:02:12">[00:02:12]</a> <a class="yt-timestamp" data-t="00:02:30">[00:02:30]</a>:

*   **Original Equation:** `2x + 3 = 5x - 2`
*   **Subtract `2x` from both sides:**
    `2x + 3 - 2x = 5x - 2 - 2x` <a class="yt-timestamp" data-t="00:02:47">[00:02:47]</a> <a class="yt-timestamp" data-t="00:02:50">[00:02:50]</a>
*   **Simplify:**
    *   On the left, `2x - 2x` cancels out, leaving `3` <a class="yt-timestamp" data-t="00:02:59">[00:02:59]</a>.
    *   On the right, `5x - 2x` simplifies to `3x` <a class="yt-timestamp" data-t="00:03:10">[00:03:10]</a>.
*   **Resulting Equation:** `3 = 3x - 2` <a class="yt-timestamp" data-t="00:03:21">[00:03:21]</a>

### Step 2: Isolate the Variable Term

Next, we need to isolate the term with 'x' (in this case, `3x`) by eliminating the constant term from that side. We can achieve this by adding `2` to both sides of the equation <a class="yt-timestamp" data-t="00:03:49">[00:03:49]</a>:

*   **Current Equation:** `3 = 3x - 2`
*   **Add `2` to both sides:**
    `3 + 2 = 3x - 2 + 2` <a class="yt-timestamp" data-t="00:04:07">[00:04:07]</a> <a class="yt-timestamp" data-t="00:04:09">[00:04:09]</a>
*   **Simplify:**
    *   On the left, `3 + 2` equals `5` <a class="yt-timestamp" data-t="00:04:13">[00:04:13]</a>.
    *   On the right, `-2 + 2` cancels out, leaving `3x` <a class="yt-timestamp" data-t="00:04:22">[00:04:22]</a>.
*   **Resulting Equation:** `5 = 3x` <a class="yt-timestamp" data-t="00:04:44">[00:04:44]</a>

### Step 3: Solve for the Variable

Finally, to solve for 'x', divide both sides by the coefficient of 'x', which is `3` <a class="yt-timestamp" data-t="00:05:31">[00:05:31]</a> <a class="yt-timestamp" data-t="00:05:51">[00:05:51]</a>:

*   **Current Equation:** `5 = 3x`
*   **Divide both sides by `3`:**
    `5 / 3 = 3x / 3` <a class="yt-timestamp" data-t="00:05:43">[00:05:43]</a> <a class="yt-timestamp" data-t="00:05:44">[00:05:44]</a>
*   **Simplify:**
    *   On the left, `5 / 3` remains `5/3` <a class="yt-timestamp" data-t="00:06:05">[00:06:05]</a>.
    *   On the right, `3x / 3` simplifies to `x` <a class="yt-timestamp" data-t="00:06:00">[00:06:00]</a>.
*   **Solution:** `5/3 = x` <a class="yt-timestamp" data-t="00:06:08">[00:06:08]</a>

It is perfectly acceptable to have the variable on the right-hand side; `5/3 = x` is completely [[equivalent_transformations_in_algebra | equivalent]] to `x = 5/3` <a class="yt-timestamp" data-t="00:06:17">[00:06:17]</a>.

### Expressing the Solution

The solution can also be expressed as a mixed number: `3` goes into `5` one time with a remainder of `2`, so `5/3` is equivalent to `1 2/3` <a class="yt-timestamp" data-t="00:06:31">[00:06:31]</a>.

Therefore, `x = 1 2/3` <a class="yt-timestamp" data-t="00:06:44">[00:06:44]</a>.
To verify the solution, substitute `1 2/3` back into the original equation to ensure both sides are equal <a class="yt-timestamp" data-t="00:06:49">[00:06:49]</a>.