---
title: Understanding components of a quadratic equation
videoId: i7idZfS8t8w
---

From: [[khanacademy]] <br/> 

The [[introduction_to_the_quadratic_formula | quadratic formula]] is considered one of the most useful formulas in mathematics for [[solving_quadratic_equations | solving quadratic equations]] <a class="yt-timestamp" data-t="00:00:04">[00:00:04]</a>. While memorizing it is recommended, understanding its derivation through [[quadratic_equations_transformation | completing the square]] is also crucial <a class="yt-timestamp" data-t="00:00:17">[00:00:17]</a>.

## Standard Form of a Quadratic Equation

A [[quadratic_polynomials | quadratic equation]] is typically expressed in the form:
`ax² + bx + c = 0` <a class="yt-timestamp" data-t="00:00:44">[00:00:44]</a>

In this general form:
*   `a` is the coefficient of the x-squared (second-degree) term <a class="yt-timestamp" data-t="00:01:00">[00:01:00]</a>.
*   `b` is the coefficient of the x-term <a class="yt-timestamp" data-t="00:01:02">[00:01:02]</a>.
*   `c` is the constant term, which can be thought of as the coefficient of the x-to-the-zero term <a class="yt-timestamp" data-t="00:01:05">[00:01:05]</a>.

The quadratic formula is used to solve for the roots, or zeroes, of these equations <a class="yt-timestamp" data-t="00:00:32">[00:00:32]</a>.

## The Quadratic Formula

For a general quadratic equation `ax² + bx + c = 0`, the [[methods_for_solving_quadratic_equations | solutions]] for x are given by the quadratic formula:

```
x = [-b ± sqrt(b² - 4ac)] / 2a
```
This formula provides the values of x for which the equation equals zero <a class="yt-timestamp" data-t="00:01:13">[00:01:13]</a>.

## Origin of the Formula

The [[quadratic_formula | quadratic formula]] is derived by [[quadratic_equations_transformation | completing the square]] on the general quadratic equation `ax² + bx + c = 0` <a class="yt-timestamp" data-t="00:01:54">[00:01:54]</a>.

## [[applications_of_the_quadratic_formula_in_solving_complex_equations | Applying the Quadratic Formula]]

### Example 1: Verifying with a Factorable Equation

Consider the equation `x² + 4x - 21 = 0` <a class="yt-timestamp" data-t="00:02:14">[00:02:14]</a>.
Here, `a = 1`, `b = 4`, and `c = -21` <a class="yt-timestamp" data-t="00:02:30">[00:02:30]</a>.

Plugging these values into the formula:
`x = [-4 ± sqrt(4² - 4 * 1 * -21)] / (2 * 1)` <a class="yt-timestamp" data-t="00:02:56">[00:02:56]</a>
`x = [-4 ± sqrt(16 + 84)] / 2` <a class="yt-timestamp" data-t="00:03:55">[00:03:55]</a>
`x = [-4 ± sqrt(100)] / 2` <a class="yt-timestamp" data-t="00:04:03">[00:04:03]</a>
`x = [-4 ± 10] / 2` <a class="yt-timestamp" data-t="00:04:13">[00:04:13]</a>

This yields two solutions:
*   `x = (-4 + 10) / 2 = 6 / 2 = 3` <a class="yt-timestamp" data-t="00:04:32">[00:04:32]</a>
*   `x = (-4 - 10) / 2 = -14 / 2 = -7` <a class="yt-timestamp" data-t="00:04:38">[00:04:38]</a>

These results match those obtained by [[factoring_quadratic_equations | factoring the quadratic equation]] into `(x + 7)(x - 3) = 0` <a class="yt-timestamp" data-t="00:05:04">[00:05:04]</a>.

### Example 2: Equations with No Real Solutions

Consider `3x² + 6x = -10` <a class="yt-timestamp" data-t="00:06:17">[00:06:17]</a>.
First, transform it to the standard form: `3x² + 6x + 10 = 0` <a class="yt-timestamp" data-t="00:06:31">[00:06:31]</a>.
Here, `a = 3`, `b = 6`, and `c = 10` <a class="yt-timestamp" data-t="00:06:51">[00:06:51]</a>.

Applying the formula:
`x = [-6 ± sqrt(6² - 4 * 3 * 10)] / (2 * 3)` <a class="yt-timestamp" data-t="00:07:13">[00:07:13]</a>
`x = [-6 ± sqrt(36 - 120)] / 6` <a class="yt-timestamp" data-t="00:07:46">[00:07:46]</a>
`x = [-6 ± sqrt(-84)] / 6` <a class="yt-timestamp" data-t="00:08:46">[00:08:46]</a>

Since the discriminant (`b² - 4ac`) is negative, `sqrt(-84)` is not a real number <a class="yt-timestamp" data-t="00:08:58">[00:08:58]</a>. This means the equation has no real solutions <a class="yt-timestamp" data-t="00:09:15">[00:09:15]</a>. Graphically, the parabola represented by `y = 3x² + 6x + 10` does not intersect the x-axis, confirming no real roots <a class="yt-timestamp" data-t="00:10:20">[00:10:20]</a>. Solutions involving the square root of a negative number are called imaginary numbers <a class="yt-timestamp" data-t="00:09:17">[00:09:17]</a>.

### Example 3: Finding Complex Solutions

Consider ` -3x² + 12x + 1 = 0` <a class="yt-timestamp" data-t="00:10:52">[00:10:52]</a>.
Here, `a = -3`, `b = 12`, and `c = 1` <a class="yt-timestamp" data-t="00:11:07">[00:11:07]</a>.

Applying the formula:
`x = [-12 ± sqrt(12² - 4 * -3 * 1)] / (2 * -3)` <a class="yt-timestamp" data-t="00:11:13">[00:11:13]</a>
`x = [-12 ± sqrt(144 + 12)] / -6` <a class="yt-timestamp" data-t="00:11:43">[00:11:43]</a>
`x = [-12 ± sqrt(156)] / -6` <a class="yt-timestamp" data-t="00:12:01">[00:12:01]</a>

To simplify `sqrt(156)`:
`sqrt(156) = sqrt(4 * 39) = 2 * sqrt(39)` <a class="yt-timestamp" data-t="00:12:48">[00:12:48]</a>

Substitute back into the equation:
`x = [-12 ± 2 * sqrt(39)] / -6` <a class="yt-timestamp" data-t="00:13:10">[00:13:10]</a>
Divide all terms by 2:
`x = [-6 ± sqrt(39)] / -3` <a class="yt-timestamp" data-t="00:13:26">[00:13:26]</a>

This can be further simplified:
`x = (-6 / -3) ± (sqrt(39) / -3)` <a class="yt-timestamp" data-t="00:13:38">[00:13:38]</a>
`x = 2 ± (-sqrt(39) / 3)` <a class="yt-timestamp" data-t="00:13:51">[00:13:51]</a>

Since `±` already accounts for both positive and negative variations, the final solutions are:
`x = 2 ± [sqrt(39) / 3]` <a class="yt-timestamp" data-t="00:15:01">[00:15:01]</a>.