---
title: Understanding algebraic expressions
videoId: vDqOoI-4Z6M
---

From: [[khanacademy]] <br/> 

When dealing with basic arithmetic, one works with concrete numbers like `23 + 5` or `2 * 7`, where the exact numbers are known and can be calculated directly <a class="yt-timestamp" data-t="00:00:02">[00:00:02]</a>. As one enters the algebraic world, the concept of variables is introduced <a class="yt-timestamp" data-t="00:00:20">[00:00:20]</a>.

## What Are Variables?

Variables are values within expressions that can change <a class="yt-timestamp" data-t="00:00:33">[00:00:33]</a>. Their specific value depends on the context of the problem <a class="yt-timestamp" data-t="00:01:34">[00:01:34]</a>.

For instance, consider the expression `x + 5` <a class="yt-timestamp" data-t="00:00:38">[00:00:38]</a>:
*   If `x` is equal to `1`, then `x + 5` becomes `1 + 5`, which evaluates to `6` <a class="yt-timestamp" data-t="00:01:00">[00:01:00]</a>.
*   If `x` is equal to `-7`, then `x + 5` becomes `-7 + 5`, which evaluates to `-2` <a class="yt-timestamp" data-t="00:01:11">[00:01:11]</a>.

In both cases, `x` acts as a variable, and its value changes based on the context provided <a class="yt-timestamp" data-t="00:01:34">[00:01:34]</a>.

## Expressions vs. Equations

It's important to understand the distinction between an expression and an equation <a class="yt-timestamp" data-t="00:01:42">[00:01:42]</a>.

### Algebraic Expressions
An expression is essentially a statement of value or a quantity <a class="yt-timestamp" data-t="00:01:46">[00:01:46]</a>.
*   **Examples:** `x + 5` <a class="yt-timestamp" data-t="00:01:56">[00:01:56]</a> or `y + z` <a class="yt-timestamp" data-t="00:02:11">[00:02:11]</a>.
*   The value of an expression changes depending on the values of the variables within it <a class="yt-timestamp" data-t="00:01:59">[00:01:59]</a>. These can be evaluated for different variable values <a class="yt-timestamp" data-t="00:02:05">[00:02:05]</a>.
*   For `y + z`, if `y = 1` and `z = 2`, the expression evaluates to `3` <a class="yt-timestamp" data-t="00:02:14">[00:02:14]</a>. If `y = 0` and `z = -1`, it evaluates to `-1` <a class="yt-timestamp" data-t="00:02:18">[00:02:18]</a>.

### Algebraic Equations
An equation involves setting two expressions equal to each other <a class="yt-timestamp" data-t="00:02:32">[00:02:32]</a>, hence the term "equating" <a class="yt-timestamp" data-t="00:02:38">[00:02:38]</a>.
*   **Example:** `x + 3 = 1` <a class="yt-timestamp" data-t="00:02:44">[00:02:44]</a>.
*   In an equation with a single unknown, the variable's value can be constrained <a class="yt-timestamp" data-t="00:02:52">[00:02:52]</a>. For `x + 3 = 1`, `x` must be `-2` <a class="yt-timestamp" data-t="00:03:06">[00:03:06]</a>.
*   Equations can also have multiple variables, like `x + y + z = 5` <a class="yt-timestamp" data-t="00:03:17">[00:03:17]</a>.
    *   If `y = 3` and `z = 2`, the equation becomes `x + 3 + 2 = 5`, which simplifies to `x + 5 = 5` <a class="yt-timestamp" data-t="00:03:42">[00:03:42]</a>. In this specific scenario, `x` is constrained to be `0` <a class="yt-timestamp" data-t="00:04:07">[00:04:07]</a>.

### Key Distinction
The crucial takeaway is that in an equation, two expressions are equated <a class="yt-timestamp" data-t="00:04:20">[00:04:20]</a>, and a variable can take on different values depending on the specific problem's context <a class="yt-timestamp" data-t="00:04:25">[00:04:25]</a>. This concept is fundamental to [[understanding_relationships_and_equations_in_algebra | understanding relationships and equations in algebra]].

## Evaluating Expressions with Variables

To solidify the understanding of variables, consider evaluating expressions by substituting different values for the variables.

### Example 1: `x` to the `y` power (`x^y`) <a class="yt-timestamp" data-t="00:04:38">[00:04:38]</a>
*   If `x = 5` and `y = 2`, the expression evaluates to `5^2`, which is `25` <a class="yt-timestamp" data-t="00:04:47">[00:04:47]</a>.
*   If `x = -2` and `y = 3`, the expression evaluates to `(-2)^3`, which is `-2 * -2 * -2 = -8` <a class="yt-timestamp" data-t="00:05:16">[00:05:16]</a>.

### Example 2: Square root of `x + y` minus `x` (`√(x + y) - x`) <a class="yt-timestamp" data-t="00:05:58">[00:05:58]</a>
*   If `x = 1` and `y = 8`, the expression evaluates to `√(1 + 8) - 1` <a class="yt-timestamp" data-t="00:06:09">[00:06:09]</a>.
    *   First, calculate `1 + 8 = 9` <a class="yt-timestamp" data-t="00:06:32">[00:06:32]</a>.
    *   Then, find the principal root of `9`, which is `3` <a class="yt-timestamp" data-t="00:06:34">[00:06:34]</a>.
    *   Finally, subtract `x` (which is `1`): `3 - 1 = 2` <a class="yt-timestamp" data-t="00:06:48">[00:06:48]</a>.

This demonstrates how expressions can be simplified and evaluated once specific values are assigned to their variables.