---
title: Understanding equivalent expressions in algebra
videoId: f15zA0PhSek
---

From: [[khanacademy]] <br/> 

Equivalent expressions and equations in algebra are fundamental concepts that allow for the manipulation and solving of complex mathematical problems. When solving an equation, the goal is to [[understanding_and_manipulating_equalities | isolate]] the variable (e.g., `x`) to find its value <a class="yt-timestamp" data-t="00:00:33">[00:00:33]</a>. This process involves performing operations that transform the original equation into an equivalent one, meaning both equations have the same solution <a class="yt-timestamp" data-t="00:00:46">[00:00:46]</a>.

## Principle of Equivalence
The key principle for maintaining equivalent expressions or equations is to perform the *same operation* on *both sides* of the equation <a class="yt-timestamp" data-t="00:00:46">[00:00:46]</a>. This ensures that the equality remains true throughout the manipulation process. As long as legitimate operations are performed, the correct answer will eventually be achieved <a class="yt-timestamp" data-t="00:02:26">[00:02:26]</a>. Visualizing these operations can help understand *why* certain steps are allowed and maintain the equation's balance <a class="yt-timestamp" data-t="00:00:58">[00:00:58]</a>.

## Demonstrating Equivalence through Operations
Consider the equation: `2x + 3 = 5x - 2` <a class="yt-timestamp" data-t="00:00:15">[00:00:15]</a>. To solve this, algebraic operations are applied to create simpler, yet equivalent, equations.

### 1. Subtracting Terms
To gather the `x` terms on one side, one can subtract a term from both sides. For instance, subtracting `2x` from both sides removes `2x` from the left and reduces `5x` on the right <a class="yt-timestamp" data-t="00:02:30">[00:02:30]</a>:
*   Original: `2x + 3 = 5x - 2` <a class="yt-timestamp" data-t="00:00:03">[00:00:03]</a>
*   Subtract `2x` from both sides: `(2x + 3) - 2x = (5x - 2) - 2x` <a class="yt-timestamp" data-t="00:02:49">[00:02:49]</a>
*   Equivalent equation: `3 = 3x - 2` <a class="yt-timestamp" data-t="00:03:21">[00:03:21]</a>

### 2. Adding Terms
To further [[simplifying_expressions | isolate]] the `x` term, constant values can be moved by adding to both sides. Adding `2` to both sides eliminates the `-2` on the right:
*   Current: `3 = 3x - 2`
*   Add `2` to both sides: `3 + 2 = (3x - 2) + 2` <a class="yt-timestamp" data-t="00:03:49">[00:03:49]</a>
*   Equivalent equation: `5 = 3x` <a class="yt-timestamp" data-t="00:04:44">[00:04:44]</a>

### 3. Dividing Terms
Finally, to solve for `x` when it's multiplied by a [[applying_arithmetic_to_algebra | coefficient]], divide both sides by that coefficient <a class="yt-timestamp" data-t="00:05:31">[00:05:31]</a>. The coefficient is the number multiplying the variable <a class="yt-timestamp" data-t="00:05:51">[00:05:51]</a>.
*   Current: `5 = 3x`
*   Divide both sides by `3`: `5 / 3 = 3x / 3` <a class="yt-timestamp" data-t="00:05:43">[00:05:43]</a>
*   Equivalent equation: `5/3 = x` <a class="yt-timestamp" data-t="00:06:05">[00:06:05]</a>

This final equation, `5/3 = x`, is completely equivalent to `x = 5/3` <a class="yt-timestamp" data-t="00:06:16">[00:06:16]</a>. It can also be expressed as a mixed number: `x = 1 2/3` <a class="yt-timestamp" data-t="00:06:44">[00:06:44]</a>. Each step produced an equivalent equation, leading to the solution.