---
title: Using grouping methods to factor expressions
videoId: 7Uos1ED3KHI
---

From: [[khanacademy]] <br/> 

When dealing with [[mathematical_expressions | mathematical expressions]], particularly [[rational_expressions_with_variables | rational expressions with variables]], the ability to factor is crucial for [[simplifying_expressions | simplifying expressions]] to their lowest terms <a class="yt-timestamp" data-t="00:01:04">[00:01:04]</a>. Just as rational numbers (fractions) like 3/6 can be simplified by recognizing common factors <a class="yt-timestamp" data-t="00:00:07">[00:00:07]</a>, [[understanding_algebraic_expressions | algebraic expressions]] can also be simplified by [[factoring_numerators_and_denominators | factoring numerators and denominators]] to find common terms <a class="yt-timestamp" data-t="00:01:37">[00:01:37]</a>.

## Factoring by Grouping for Quadratic Expressions

For more complex quadratic expressions, especially those where the leading coefficient (the coefficient of the x-squared term) is not 1, [[factoring_by_grouping | factoring by grouping]] is a powerful [[strategies_for_dealing_with_complex_arithmetic_expressions | strategy]] <a class="yt-timestamp" data-t="00:07:52">[00:07:52]</a>.

### Example 1: Factoring `3x² + 3x - 18`

To factor `3x² + 3x - 18` using [[factoring_by_grouping | grouping]] <a class="yt-timestamp" data-t="00:08:01">[00:08:01]</a>:

1.  **Find two numbers (a and b):**
    *   Their product (`a * b`) must equal the product of the leading coefficient and the constant term (3 * -18 = -54) <a class="yt-timestamp" data-t="00:08:12">[00:08:12]</a>.
    *   Their sum (`a + b`) must equal the coefficient of the middle term (3) <a class="yt-timestamp" data-t="00:08:21">[00:08:21]</a>.
    *   For -54 and 3, the numbers are 9 and -6 (since 9 * -6 = -54 and 9 + (-6) = 3) <a class="yt-timestamp" data-t="00:08:41">[00:08:41]</a>.

2.  **Rewrite the middle term:** Split the `3x` into `9x - 6x` <a class="yt-timestamp" data-t="00:09:03">[00:09:03]</a>.
    *   The expression becomes `3x² + 9x - 6x - 18` <a class="yt-timestamp" data-t="00:09:03">[00:09:03]</a>.

3.  **Group the terms:** Group the first two terms and the last two terms <a class="yt-timestamp" data-t="00:09:35">[00:09:35]</a>.
    *   `(3x² + 9x) + (-6x - 18)`

4.  **Factor out common monomials from each group:**
    *   From `(3x² + 9x)`, factor out `3x`, resulting in `3x(x + 3)` <a class="yt-timestamp" data-t="00:09:56">[00:09:56]</a>.
    *   From `(-6x - 18)`, factor out `-6`, resulting in `-6(x + 3)` <a class="yt-timestamp" data-t="00:10:02">[00:10:02]</a>.

5.  **Factor out the common binomial:** Notice that both factored groups now share `(x + 3)`. Factor this out.
    *   The expression becomes `(3x - 6)(x + 3)` <a class="yt-timestamp" data-t="00:10:15">[00:10:15]</a>.

### Example 2: Factoring `2x² + 5x - 3`

To factor `2x² + 5x - 3` using [[factoring_by_grouping | grouping]] <a class="yt-timestamp" data-t="00:11:02">[00:11:02]</a>:

1.  **Find two numbers (a and b):**
    *   Their product (`a * b`) must equal (2 * -3 = -6) <a class="yt-timestamp" data-t="00:13:00">[00:13:00]</a>.
    *   Their sum (`a + b`) must equal (5) <a class="yt-timestamp" data-t="00:13:08">[00:13:08]</a>.
    *   For -6 and 5, the numbers are 6 and -1 (since 6 * -1 = -6 and 6 + (-1) = 5) <a class="yt-timestamp" data-t="00:13:12">[00:13:12]</a>.

2.  **Rewrite the middle term:** Split the `5x` into `6x - x` <a class="yt-timestamp" data-t="00:13:37">[00:13:37]</a>.
    *   The expression becomes `2x² + 6x - x - 3` <a class="yt-timestamp" data-t="00:13:37">[00:13:37]</a>.

3.  **Group the terms:** `(2x² + 6x) + (-x - 3)` <a class="yt-timestamp" data-t="00:13:53">[00:13:53]</a>.

4.  **Factor out common monomials from each group:**
    *   From `(2x² + 6x)`, factor out `2x`, resulting in `2x(x + 3)` <a class="yt-timestamp" data-t="00:13:57">[00:13:57]</a>.
    *   From `(-x - 3)`, factor out `-1`, resulting in `-1(x + 3)` <a class="yt-timestamp" data-t="00:14:02">[00:14:02]</a>.

5.  **Factor out the common binomial:**
    *   The expression becomes `(2x - 1)(x + 3)` <a class="yt-timestamp" data-t="00:14:11">[00:14:11]</a>.

## Application in Simplifying Rational Expressions

Once [[factoring_quadratic_equations | factoring quadratic equations]] or other [[mathematical_expressions | mathematical expressions]] is complete, these factored forms are used to [[simplifying_algebraic_equations_involving_fractions | simplify algebraic equations involving fractions]] by canceling common factors in the numerator and denominator <a class="yt-timestamp" data-t="00:01:04">[00:01:04]</a>.

For instance, if you have the rational expression `(3x² + 3x - 18) / (2x² + 5x - 3)`:

*   Numerator: `(3x - 6)(x + 3)` <a class="yt-timestamp" data-t="00:10:45">[00:10:45]</a>
*   Denominator: `(2x - 1)(x + 3)` <a class="yt-timestamp" data-t="00:14:37">[00:14:37]</a>

The expression becomes `(3x - 6)(x + 3) / ((2x - 1)(x + 3))` <a class="yt-timestamp" data-t="00:14:37">[00:14:37]</a>.
The common factor `(x + 3)` can be cancelled out <a class="yt-timestamp" data-t="00:14:40">[00:14:40]</a>.

### Important Consideration: Excluded Values

> [!attention] Domain Restrictions
> When [[simplifying_expressions | simplifying expressions]] by canceling common factors, it is crucial to remember the values of variables that would have made the original denominator zero, rendering the expression undefined <a class="yt-timestamp" data-t="00:03:21">[00:03:21]</a>. These values must be excluded from the domain of the simplified expression to maintain equivalence with the original <a class="yt-timestamp" data-t="00:03:28">[00:03:28]</a>.
>
> In the example above, `(x + 3)` was a common factor in the denominator. If `x = -3`, then `(x + 3)` would be `0`, making the original expression undefined <a class="yt-timestamp" data-t="00:14:47">[00:14:47]</a>. Therefore, the simplified expression `(3x - 6) / (2x - 1)` is only equivalent to the original *if* the condition `x ≠ -3` is also stated <a class="yt-timestamp" data-t="00:15:02">[00:15:02]</a>.