---
title: Working with positive and negative factors in quadratics
videoId: eF6zYNzlZKQ
---

From: [[khanacademy]] <br/> 

[[factoring_quadratic_polynomials | Factoring]] a second-degree polynomial, commonly known as a [[quadratic_equations | quadratic]] or [[understanding_quadratic_expressions | quadratic expression]], involves expressing it as the product of two binomials <a class="yt-timestamp" data-t="00:00:03">[00:00:03]</a>. A [[quadratic_equations | quadratic]] is defined as a polynomial where the variable is raised to the second power <a class="yt-timestamp" data-t="00:00:18">[00:00:18]</a>.

## The Basic Principle of Factoring Quadratics

To understand how to factor a [[quadratic_equations | quadratic expression]] like `x² + 10x + 9` <a class="yt-timestamp" data-t="00:00:30">[00:00:30]</a> into the product of two binomials, consider the general multiplication of `(x + a)` by `(x + b)` <a class="yt-timestamp" data-t="00:00:44">[00:00:44]</a>:

` (x + a)(x + b) = x² + bx + ax + ab ` <a class="yt-timestamp" data-t="00:00:57">[00:00:57]</a>
` (x + a)(x + b) = x² + (a + b)x + ab ` <a class="yt-timestamp" data-t="00:01:22">[00:01:22]</a>

From this, it can be observed that when a [[quadratic_equations | quadratic]] is in standard form (`ax² + bx + c`), the coefficient of the `x` term (the first-degree coefficient) is the sum of `a` and `b` <a class="yt-timestamp" data-t="00:01:40">[00:01:40]</a>, and the constant term is the product of `a` and `b` <a class="yt-timestamp" data-t="00:01:49">[00:01:49]</a>. This principle is applied when the leading coefficient (the coefficient of the `x²` term) is 1 <a class="yt-timestamp" data-t="00:03:22">[00:03:22]</a>.

## Factoring with Positive Factors

When both the middle term's coefficient and the constant term are positive, the factors `a` and `b` will both be positive integers <a class="yt-timestamp" data-t="00:02:27">[00:02:27]</a>.

### Example 1: `x² + 10x + 9`

To factor `x² + 10x + 9` <a class="yt-timestamp" data-t="00:00:30">[00:00:30]</a>:
*   Find two numbers `a` and `b` such that `a + b = 10` <a class="yt-timestamp" data-t="00:02:05">[00:02:05]</a>.
*   And `a × b = 9` <a class="yt-timestamp" data-t="00:02:14">[00:02:14]</a>.

Considering the factors of 9 (1, 3, 9) <a class="yt-timestamp" data-t="00:02:37">[00:02:37]</a>:
*   If `a=3, b=3`, then `3+3=6` (not 10) <a class="yt-timestamp" data-t="00:02:45">[00:02:45]</a>.
*   If `a=1, b=9`, then `1×9=9` and `1+9=10` <a class="yt-timestamp" data-t="00:02:49">[00:02:49]</a>. This works <a class="yt-timestamp" data-t="00:02:56">[00:02:56]</a>.

Therefore, `x² + 10x + 9` factors to `(x + 1)(x + 9)` <a class="yt-timestamp" data-t="00:03:04">[00:03:04]</a>.

### Example 2: `x² + 15x + 50`

To factor `x² + 15x + 50` <a class="yt-timestamp" data-t="00:04:11">[00:04:11]</a>:
*   Find two numbers `a` and `b` such that `a + b = 15` <a class="yt-timestamp" data-t="00:04:35">[00:04:35]</a>.
*   And `a × b = 50` <a class="yt-timestamp" data-t="00:04:35">[00:04:35]</a>.

Considering the factors of 50 (1, 2, 5, 10, 25, 50) <a class="yt-timestamp" data-t="00:04:47">[00:04:47]</a>:
*   `1 × 50`: `1 + 50` does not equal 15 <a class="yt-timestamp" data-t="00:05:07">[00:05:07]</a>.
*   `2 × 25`: `2 + 25` does not equal 15 <a class="yt-timestamp" data-t="00:05:12">[00:05:12]</a>.
*   `5 × 10`: `5 + 10` equals 15 <a class="yt-timestamp" data-t="00:05:16">[00:05:16]</a>. This works.

Therefore, `x² + 15x + 50` factors to `(x + 5)(x + 10)` <a class="yt-timestamp" data-t="00:05:24">[00:05:24]</a>.

## Working with Negative Factors

The presence of negative signs requires careful consideration of the signs of `a` and `b`.

### Case 1: Negative Middle Term, Positive Constant Term

If the product `a × b` is positive, then `a` and `b` must have the same sign (both positive or both negative) <a class="yt-timestamp" data-t="00:06:41">[00:06:41]</a>. If their sum `a + b` is negative, then both `a` and `b` must be negative <a class="yt-timestamp" data-t="00:07:03">[00:07:03]</a>.

### Example 3: `x² - 11x + 24`

To factor `x² - 11x + 24` <a class="yt-timestamp" data-t="00:06:11">[00:06:11]</a>:
*   Find `a` and `b` such that `a + b = -11` <a class="yt-timestamp" data-t="00:06:26">[00:06:26]</a>.
*   And `a × b = 24` <a class="yt-timestamp" data-t="00:06:30">[00:06:30]</a>.

Since the product is positive (24) and the sum is negative (-11), both `a` and `b` must be negative <a class="yt-timestamp" data-t="00:07:05">[00:07:05]</a>.
Consider factors of 24 (1, 2, 3, 4, 6, 8, 12, 24) <a class="yt-timestamp" data-t="00:07:28">[00:07:28]</a>:
*   The pair `3` and `8` are relevant because `3 + 8 = 11` <a class="yt-timestamp" data-t="00:08:15">[00:08:15]</a>.
*   If `a = -3` and `b = -8`, then `(-3) × (-8) = 24` <a class="yt-timestamp" data-t="00:08:29">[00:08:29]</a>.
*   And `(-3) + (-8) = -11` <a class="yt-timestamp" data-t="00:08:37">[00:08:37]</a>. This works.

Therefore, `x² - 11x + 24` factors to `(x - 3)(x - 8)` <a class="yt-timestamp" data-t="00:08:53">[00:08:53]</a>.

### Case 2: Positive Middle Term, Negative Constant Term

If the product `a × b` is negative, then one factor must be positive and the other must be negative <a class="yt-timestamp" data-t="00:09:29">[00:09:29]</a>. The sign of the sum `a + b` will indicate which factor (the larger or smaller absolute value) is positive or negative.

### Example 4: `x² + 5x - 14`

To factor `x² + 5x - 14` <a class="yt-timestamp" data-t="00:09:08">[00:09:08]</a>:
*   Find `a` and `b` such that `a + b = 5` <a class="yt-timestamp" data-t="00:09:33">[00:09:33]</a>.
*   And `a × b = -14` <a class="yt-timestamp" data-t="00:09:21">[00:09:21]</a>.

Since the product is negative (-14), one factor is positive and one is negative.
Consider factors of 14 (1, 2, 7, 14) <a class="yt-timestamp" data-t="00:09:41">[00:09:41]</a>:
*   The pair `2` and `7` is relevant.
*   If `a = -2` and `b = 7`, then `(-2) × 7 = -14` <a class="yt-timestamp" data-t="00:10:42">[00:10:42]</a>.
*   And `(-2) + 7 = 5` <a class="yt-timestamp" data-t="00:10:29">[00:10:29]</a>. This works.

Therefore, `x² + 5x - 14` factors to `(x - 2)(x + 7)` <a class="yt-timestamp" data-t="00:10:47">[00:10:47]</a>.

### Case 3: Negative Middle Term, Negative Constant Term

Similar to Case 2, one factor is positive and one is negative, but the larger absolute value will be negative because the sum is negative.

### Example 5: `x² - x - 56`

To factor `x² - x - 56` <a class="yt-timestamp" data-t="00:11:09">[00:11:09]</a>:
*   Find `a` and `b` such that `a + b = -1` (the coefficient of `x`) <a class="yt-timestamp" data-t="00:11:26">[00:11:26]</a>.
*   And `a × b = -56` <a class="yt-timestamp" data-t="00:11:16">[00:11:16]</a>.

Since the product is negative (-56), one factor is positive and one is negative. Since the sum is negative (-1), the number with the larger absolute value will be negative.
The factors of 56 that are close to each other are 7 and 8 <a class="yt-timestamp" data-t="00:11:33">[00:11:33]</a>.
*   If `a = -8` and `b = 7`, then `(-8) × 7 = -56` <a class="yt-timestamp" data-t="00:11:58">[00:11:58]</a>.
*   And `(-8) + 7 = -1` <a class="yt-timestamp" data-t="00:12:03">[00:12:03]</a>. This works.

Therefore, `x² - x - 56` factors to `(x - 8)(x + 7)` <a class="yt-timestamp" data-t="00:12:12">[00:12:12]</a>.

## [[factoring_quadratics_with_negative_leading_coefficients | Dealing with Negative Leading Coefficients]]

When the coefficient of the `x²` term is negative, the easiest approach is to factor out -1 from the entire expression <a class="yt-timestamp" data-t="00:13:00">[00:13:00]</a>.

### Example 6: `-x² - 5x + 24`

To factor `-x² - 5x + 24` <a class="yt-timestamp" data-t="00:12:55">[00:12:55]</a>:
1.  Factor out -1: `-1(x² + 5x - 24)` <a class="yt-timestamp" data-t="00:13:07">[00:13:07]</a>.
2.  Now factor the inner quadratic `x² + 5x - 24`:
    *   Find `a` and `b` such that `a + b = 5` <a class="yt-timestamp" data-t="00:13:41">[00:13:41]</a>.
    *   And `a × b = -24` <a class="yt-timestamp" data-t="00:13:29">[00:13:29]</a>.

    Factors of 24 (1, 2, 3, 4, 6, 8, 12, 24) <a class="yt-timestamp" data-t="00:13:43">[00:13:43]</a>.
    The pair `3` and `8` are relevant. Since the sum is positive (5), the larger number (8) should be positive.
    *   If `a = -3` and `b = 8`, then `(-3) × 8 = -24` <a class="yt-timestamp" data-t="00:14:24">[00:14:24]</a>.
    *   And `(-3) + 8 = 5` <a class="yt-timestamp" data-t="00:14:24">[00:14:24]</a>. This works.

3.  Combine with the factored-out -1: `-1(x - 3)(x + 8)` <a class="yt-timestamp" data-t="00:14:31">[00:14:31]</a>.

### Example 7: `-x² + 18x - 72`

To factor `-x² + 18x - 72` <a class="yt-timestamp" data-t="00:14:56">[00:14:56]</a>:
1.  Factor out -1: `-1(x² - 18x + 72)` <a class="yt-timestamp" data-t="00:15:09">[00:15:09]</a>.
2.  Now factor the inner quadratic `x² - 18x + 72`:
    *   Find `a` and `b` such that `a + b = -18` <a class="yt-timestamp" data-t="00:15:29">[00:15:29]</a>.
    *   And `a × b = 72` <a class="yt-timestamp" data-t="00:15:19">[00:15:19]</a>.

    Since the product is positive (72) and the sum is negative (-18), both `a` and `b` must be negative <a class="yt-timestamp" data-t="00:15:32">[00:15:32]</a>.
    Consider factors of 72. While `8` and `9` multiply to 72, `(-8) + (-9) = -17`, which is close but not -18 <a class="yt-timestamp" data-t="00:15:58">[00:15:58]</a>.
    The pair `6` and `12` are relevant.
    *   If `a = -6` and `b = -12`, then `(-6) × (-12) = 72`.
    *   And `(-6) + (-12) = -18` <a class="yt-timestamp" data-t="00:16:09">[00:16:09]</a>. This works.

3.  Combine with the factored-out -1: `-1(x - 6)(x - 12)` <a class="yt-timestamp" data-t="00:16:18">[00:16:18]</a>.

> [!NOTE] Factoring quadratics can be an "art" that requires practice with factors and signs to become second nature <a class="yt-timestamp" data-t="00:12:21">[00:12:21]</a>.